{
    "@context": {
        "gfs": "https://grundfos.com/model/",
        "gfs:ean": {
            "@type": "xsd:integer"
        },
        "gfs:level": {
            "@type": "xsd:integer"
        },
        "gfs:link": {
            "@type": "@id"
        },
        "gfs:productFamily": {
            "@type": "@id"
        },
        "gfs:typecode": {
            "@type": "xsd:string"
        },
        "rdf": "http://www.w3.org/1999/02/22-rdf-syntax-ns#",
        "rdfs": "http://www.w3.org/2000/01/rdf-schema#",
        "skos": "http://www.w3.org/2004/02/skos/core#",
        "skos:broader": {
            "@type": "@id"
        },
        "skos:narrower": {
            "@type": "@id"
        },
        "xsd": "http://www.w3.org/2001/XMLSchema#"
    },
    "@graph": [
        {
            "@id": "https://grundfos.com/concept/productFamily/DMADAPT",
            "@type": [
                "gfs:ProductFamily",
                "skos:Concept"
            ],
            "gfs:level": 2,
            "gfs:typecode": "DMADAPT",
            "rdfs:comment": "Adaptor connections for DME & DMS",
            "skos:inScheme": "https://grundfos.com/concept/productFamily",
            "skos:prefLabel": "Adapter connections DME/DMS"
        },
        {
            "@id": "https://grundfos.com/concept/productFamily/DMADAPT1",
            "@type": [
                "gfs:ProductFamily",
                "skos:Concept"
            ],
            "gfs:level": 2,
            "gfs:typecode": "DMADAPT1",
            "rdfs:comment": "Adaptor connections to connect between hoses or hose and pipe",
            "skos:inScheme": "https://grundfos.com/concept/productFamily",
            "skos:prefLabel": "Adaptors (hose-hose or hose-pipe)"
        },
        {
            "@id": "https://grundfos.com/concept/productFamily/DMADAPT2",
            "@type": [
                "gfs:ProductFamily",
                "skos:Concept"
            ],
            "gfs:level": 2,
            "gfs:typecode": "DMADAPT2",
            "rdfs:comment": "Adaptor connections to connect between different threaded connection sizes",
            "skos:inScheme": "https://grundfos.com/concept/productFamily",
            "skos:prefLabel": "Adaptors (threaded adaptors)"
        },
        {
            "@id": "https://grundfos.com/concept/productFamily/DMCATCH",
            "@type": [
                "gfs:ProductFamily",
                "skos:Concept"
            ],
            "gfs:level": 2,
            "gfs:typecode": "DMCATCH",
            "rdfs:comment": "Catchment tanks for use with cylindrical dosing tanks",
            "skos:inScheme": "https://grundfos.com/concept/productFamily",
            "skos:prefLabel": "Catchment tanks"
        },
        {
            "@id": "https://grundfos.com/concept/productFamily/DMMIX",
            "@type": [
                "gfs:ProductFamily",
                "skos:Concept"
            ],
            "gfs:level": 2,
            "gfs:typecode": "DMMIX",
            "rdfs:comment": "Electric mixers for use in dosing tanks",
            "skos:inScheme": "https://grundfos.com/concept/productFamily",
            "skos:prefLabel": "Electric mixers"
        },
        {
            "@id": "https://grundfos.com/concept/productFamily/DMFOOTV",
            "@type": [
                "gfs:ProductFamily",
                "skos:Concept"
            ],
            "gfs:level": 2,
            "gfs:typecode": "DMFOOTV",
            "rdfs:comment": "Non-return foot valves with strainer",
            "skos:inScheme": "https://grundfos.com/concept/productFamily",
            "skos:prefLabel": "Foot valves"
        },
        {
            "@id": "https://grundfos.com/concept/productFamily/DMINJEC",
            "@type": [
                "gfs:ProductFamily",
                "skos:Concept"
            ],
            "gfs:level": 2,
            "gfs:typecode": "DMINJEC",
            "rdfs:comment": "The injection units are used in conjunction with dosing pumps to inject and mix the dosing medium in pipe systems.",
            "skos:inScheme": "https://grundfos.com/concept/productFamily",
            "skos:prefLabel": "Injection units for DME from 60 l/h"
        },
        {
            "@id": "https://grundfos.com/concept/productFamily/DMINJECL",
            "@type": [
                "gfs:ProductFamily",
                "skos:Concept"
            ],
            "gfs:level": 2,
            "gfs:typecode": "DMINJECL",
            "rdfs:comment": "The injection units are used in conjunction with dosing pumps to inject and mix the dosing medium in pipe systems.",
            "skos:inScheme": "https://grundfos.com/concept/productFamily",
            "skos:prefLabel": "Injection units for pumps up to 60 l/h"
        },
        {
            "@id": "https://grundfos.com/concept/productFamily/DMINST",
            "@type": [
                "gfs:ProductFamily",
                "skos:Concept"
            ],
            "gfs:level": 2,
            "gfs:typecode": "DMINST",
            "rdfs:comment": "Installation kits",
            "skos:inScheme": "https://grundfos.com/concept/productFamily",
            "skos:prefLabel": "Installation kits"
        },
        {
            "@id": "https://grundfos.com/concept/productFamily/DMMULTI",
            "@type": [
                "gfs:ProductFamily",
                "skos:Concept"
            ],
            "gfs:level": 2,
            "gfs:typecode": "DMMULTI",
            "rdfs:comment": "Multifunction valves with counter-pressure, pressure relief, anti-siphoning and safety valve function",
            "skos:inScheme": "https://grundfos.com/concept/productFamily",
            "skos:prefLabel": "Multi function valves"
        },
        {
            "@id": "https://grundfos.com/concept/productFamily/DMPLV",
            "@type": [
                "gfs:ProductFamily",
                "skos:Concept"
            ],
            "gfs:level": 2,
            "gfs:typecode": "DMPLV",
            "rdfs:comment": "Pressure loading valves for constant pressure on the pump dischange side",
            "skos:inScheme": "https://grundfos.com/concept/productFamily",
            "skos:prefLabel": "Pressure loading valves"
        },
        {
            "@id": "https://grundfos.com/concept/productFamily/DMPRV",
            "@type": [
                "gfs:ProductFamily",
                "skos:Concept"
            ],
            "gfs:level": 2,
            "gfs:typecode": "DMPRV",
            "rdfs:comment": "Pressure relief valves open in case of too high pressure on the pump discharge side",
            "skos:inScheme": "https://grundfos.com/concept/productFamily",
            "skos:prefLabel": "Pressure relief valves"
        },
        {
            "@id": "https://grundfos.com/concept/productFamily/DMPV",
            "@type": [
                "gfs:ProductFamily",
                "skos:Concept"
            ],
            "gfs:level": 2,
            "gfs:typecode": "DMPV",
            "rdfs:comment": "Pressure valves provide a constant counterpressure of 3 bar. They are particularly required for DDA-FC or DDA-FCM pumps at very small flow rates.",
            "skos:inScheme": "https://grundfos.com/concept/productFamily",
            "skos:prefLabel": "Pressure valves"
        },
        {
            "@id": "https://grundfos.com/concept/productFamily/DMPRIM",
            "@type": [
                "gfs:ProductFamily",
                "skos:Concept"
            ],
            "gfs:level": 2,
            "gfs:typecode": "DMPRIM",
            "rdfs:comment": "Suction collectors with priming aid, gas trap and pulsation dampening function",
            "skos:inScheme": "https://grundfos.com/concept/productFamily",
            "skos:prefLabel": "Priming aids"
        },
        {
            "@id": "https://grundfos.com/concept/productFamily/DMCONN1",
            "@type": [
                "gfs:ProductFamily",
                "skos:Concept"
            ],
            "gfs:level": 2,
            "gfs:typecode": "DMCONN1",
            "rdfs:comment": "Separate pump connections",
            "skos:inScheme": "https://grundfos.com/concept/productFamily",
            "skos:prefLabel": "Pump connections for DDI/DMX"
        },
        {
            "@id": "https://grundfos.com/concept/productFamily/DMCONNE",
            "@type": [
                "gfs:ProductFamily",
                "skos:Concept"
            ],
            "gfs:level": 2,
            "gfs:typecode": "DMCONNE",
            "rdfs:comment": "Separate pump connections",
            "skos:inScheme": "https://grundfos.com/concept/productFamily",
            "skos:prefLabel": "Pump connections for DME/DMS"
        },
        {
            "@id": "https://grundfos.com/concept/productFamily/DMSUCLAN",
            "@type": [
                "gfs:ProductFamily",
                "skos:Concept"
            ],
            "gfs:level": 2,
            "gfs:typecode": "DMSUCLAN",
            "rdfs:comment": "Rigid suction lines with or without dual level switch",
            "skos:inScheme": "https://grundfos.com/concept/productFamily",
            "skos:prefLabel": "Rigid suction lances"
        },
        {
            "@id": "https://grundfos.com/concept/productFamily/DMCABLE",
            "@type": [
                "gfs:ProductFamily",
                "skos:Concept"
            ],
            "gfs:level": 2,
            "gfs:typecode": "DMCABLE",
            "rdfs:comment": "Cables and plugs for external control and level sensor connection",
            "skos:inScheme": "https://grundfos.com/concept/productFamily",
            "skos:prefLabel": "Signal cables and plugs"
        },
        {
            "@id": "https://grundfos.com/concept/productFamily/DMSTRAIN",
            "@type": [
                "gfs:ProductFamily",
                "skos:Concept"
            ],
            "gfs:level": 2,
            "gfs:typecode": "DMSTRAIN",
            "rdfs:comment": "To protect the pump from dirt",
            "skos:inScheme": "https://grundfos.com/concept/productFamily",
            "skos:prefLabel": "Strainers"
        },
        {
            "@id": "https://grundfos.com/concept/productFamily/DMTPIECE",
            "@type": [
                "gfs:ProductFamily",
                "skos:Concept"
            ],
            "gfs:level": 2,
            "gfs:typecode": "DMTPIECE",
            "rdfs:comment": "T-pieces",
            "skos:inScheme": "https://grundfos.com/concept/productFamily",
            "skos:prefLabel": "T-Pieces"
        },
        {
            "@id": "https://grundfos.com/concept/productFamily/DMTANKAC",
            "@type": [
                "gfs:ProductFamily",
                "skos:Concept"
            ],
            "gfs:level": 2,
            "gfs:typecode": "DMTANKAC",
            "rdfs:comment": "Accessories for use with dosing tanks",
            "skos:inScheme": "https://grundfos.com/concept/productFamily",
            "skos:prefLabel": "Tank accessories"
        },
        {
            "@id": "https://grundfos.com/concept/productFamily/DMTANK1",
            "@type": [
                "gfs:ProductFamily",
                "skos:Concept"
            ],
            "gfs:level": 2,
            "gfs:typecode": "DMTANK1",
            "rdfs:comment": "Chemical tanks",
            "skos:inScheme": "https://grundfos.com/concept/productFamily",
            "skos:prefLabel": "Tanks"
        },
        {
            "@id": "https://grundfos.com/concept/productFamily/DMHOSE",
            "@type": [
                "gfs:ProductFamily",
                "skos:Concept"
            ],
            "gfs:level": 2,
            "gfs:typecode": "DMHOSE",
            "rdfs:comment": "Tubing / hoses",
            "skos:inScheme": "https://grundfos.com/concept/productFamily",
            "skos:prefLabel": "Tubing / hoses"
        },
        {
            "@id": "https://grundfos.com/concept/productFamily/DMWALL",
            "@type": [
                "gfs:ProductFamily",
                "skos:Concept"
            ],
            "gfs:level": 2,
            "gfs:typecode": "DMWALL",
            "rdfs:comment": "Brackets for wall mounting of pump",
            "skos:inScheme": "https://grundfos.com/concept/productFamily",
            "skos:prefLabel": "Wall brackets"
        },
        {
            "@id": "https://grundfos.com/concept/productFamily/DMWATER",
            "@type": [
                "gfs:ProductFamily",
                "skos:Concept"
            ],
            "gfs:level": 2,
            "gfs:typecode": "DMWATER",
            "rdfs:comment": "In-line water meters with potential-free pulse signal",
            "skos:inScheme": "https://grundfos.com/concept/productFamily",
            "skos:prefLabel": "Water meters"
        },
        {
            "@id": "https://grundfos.com/concept/productFamily/DMACFAM",
            "@type": [
                "gfs:ProductFamily",
                "skos:Concept"
            ],
            "gfs:level": 1,
            "gfs:typecode": "DMACFAM",
            "rdfs:comment": "Accessories for dosing pumps",
            "skos:inScheme": "https://grundfos.com/concept/productFamily",
            "skos:narrower": [
                "https://grundfos.com/concept/productFamily/DMADAPT",
                "https://grundfos.com/concept/productFamily/DMADAPT1",
                "https://grundfos.com/concept/productFamily/DMADAPT2",
                "https://grundfos.com/concept/productFamily/DMCATCH",
                "https://grundfos.com/concept/productFamily/DMMIX",
                "https://grundfos.com/concept/productFamily/DMFOOTV",
                "https://grundfos.com/concept/productFamily/DMINJEC",
                "https://grundfos.com/concept/productFamily/DMINJECL",
                "https://grundfos.com/concept/productFamily/DMINST",
                "https://grundfos.com/concept/productFamily/DMMULTI",
                "https://grundfos.com/concept/productFamily/DMPLV",
                "https://grundfos.com/concept/productFamily/DMPRV",
                "https://grundfos.com/concept/productFamily/DMPV",
                "https://grundfos.com/concept/productFamily/DMPRIM",
                "https://grundfos.com/concept/productFamily/DMCONN1",
                "https://grundfos.com/concept/productFamily/DMCONNE",
                "https://grundfos.com/concept/productFamily/DMSUCLAN",
                "https://grundfos.com/concept/productFamily/DMCABLE",
                "https://grundfos.com/concept/productFamily/DMSTRAIN",
                "https://grundfos.com/concept/productFamily/DMTPIECE",
                "https://grundfos.com/concept/productFamily/DMTANKAC",
                "https://grundfos.com/concept/productFamily/DMTANK1",
                "https://grundfos.com/concept/productFamily/DMHOSE",
                "https://grundfos.com/concept/productFamily/DMWALL",
                "https://grundfos.com/concept/productFamily/DMWATER"
            ],
            "skos:prefLabel": "Accessories, dosing pumps"
        },
        {
            "@id": "https://grundfos.com/concept/productFamily/PCB",
            "@type": [
                "gfs:ProductFamily",
                "skos:Concept"
            ],
            "gfs:level": 2,
            "gfs:typecode": "PCB",
            "rdfs:comment": "Accessories",
            "skos:inScheme": "https://grundfos.com/concept/productFamily",
            "skos:prefLabel": "Alarm PCB"
        },
        {
            "@id": "https://grundfos.com/concept/productFamily/CABLEKIT",
            "@type": [
                "gfs:ProductFamily",
                "skos:Concept"
            ],
            "gfs:level": 2,
            "gfs:typecode": "CABLEKIT",
            "rdfs:comment": "Accessories",
            "skos:inScheme": "https://grundfos.com/concept/productFamily",
            "skos:prefLabel": "Cable termination kits"
        },
        {
            "@id": "https://grundfos.com/concept/productFamily/CAPACIT",
            "@type": [
                "gfs:ProductFamily",
                "skos:Concept"
            ],
            "gfs:level": 2,
            "gfs:typecode": "CAPACIT",
            "rdfs:comment": "Accessories",
            "skos:inScheme": "https://grundfos.com/concept/productFamily",
            "skos:prefLabel": "Capacitors"
        },
        {
            "@id": "https://grundfos.com/concept/productFamily/CONTBOX",
            "@type": [
                "gfs:ProductFamily",
                "skos:Concept"
            ],
            "gfs:level": 2,
            "gfs:typecode": "CONTBOX",
            "rdfs:comment": "Accessories",
            "skos:inScheme": "https://grundfos.com/concept/productFamily",
            "skos:prefLabel": "Control boxes"
        },
        {
            "@id": "https://grundfos.com/concept/productFamily/CU100",
            "@type": [
                "gfs:ProductFamily",
                "skos:Concept"
            ],
            "gfs:level": 2,
            "gfs:typecode": "CU100",
            "rdfs:comment": "Accessories",
            "skos:inScheme": "https://grundfos.com/concept/productFamily",
            "skos:prefLabel": "CU 100"
        },
        {
            "@id": "https://grundfos.com/concept/productFamily/CU200",
            "@type": [
                "gfs:ProductFamily",
                "skos:Concept"
            ],
            "gfs:level": 2,
            "gfs:typecode": "CU200",
            "rdfs:comment": "Accessories",
            "skos:inScheme": "https://grundfos.com/concept/productFamily",
            "skos:prefLabel": "CU 200"
        },
        {
            "@id": "https://grundfos.com/concept/productFamily/CU300",
            "@type": [
                "gfs:ProductFamily",
                "skos:Concept"
            ],
            "gfs:level": 2,
            "gfs:typecode": "CU300",
            "rdfs:comment": "CU 300 are designed for communication, monitoring and control of SQE submersible pumps in various applications.",
            "skos:inScheme": "https://grundfos.com/concept/productFamily",
            "skos:prefLabel": "CU 300"
        },
        {
            "@id": "https://grundfos.com/concept/productFamily/CU300AC",
            "@type": [
                "gfs:ProductFamily",
                "skos:Concept"
            ],
            "gfs:level": 2,
            "gfs:typecode": "CU300AC",
            "rdfs:comment": "Accessories",
            "skos:inScheme": "https://grundfos.com/concept/productFamily",
            "skos:prefLabel": "CU 300 accessories"
        },
        {
            "@id": "https://grundfos.com/concept/productFamily/CU301",
            "@type": [
                "gfs:ProductFamily",
                "skos:Concept"
            ],
            "gfs:level": 2,
            "gfs:typecode": "CU301",
            "rdfs:comment": "CU 301 are designed for communication, monitoring and control of SQE submersible pumps in constant pressure applications.",
            "skos:inScheme": "https://grundfos.com/concept/productFamily",
            "skos:prefLabel": "CU 301"
        },
        {
            "@id": "https://grundfos.com/concept/productFamily/CUEFAM",
            "@type": [
                "gfs:ProductFamily",
                "skos:Concept"
            ],
            "gfs:level": 2,
            "gfs:typecode": "CUEFAM",
            "rdfs:comment": "CUE",
            "skos:inScheme": "https://grundfos.com/concept/productFamily",
            "skos:prefLabel": "CUE"
        },
        {
            "@id": "https://grundfos.com/concept/productFamily/CUEAC",
            "@type": [
                "gfs:ProductFamily",
                "skos:Concept"
            ],
            "gfs:level": 2,
            "gfs:typecode": "CUEAC",
            "rdfs:comment": "Accessories",
            "skos:inScheme": "https://grundfos.com/concept/productFamily",
            "skos:prefLabel": "CUE accessories"
        },
        {
            "@id": "https://grundfos.com/concept/productFamily/ELCB",
            "@type": [
                "gfs:ProductFamily",
                "skos:Concept"
            ],
            "gfs:level": 2,
            "gfs:typecode": "ELCB",
            "rdfs:comment": "Accessories",
            "skos:inScheme": "https://grundfos.com/concept/productFamily",
            "skos:prefLabel": "Earth leakage circuit breakers"
        },
        {
            "@id": "https://grundfos.com/concept/productFamily/EMCFILT",
            "@type": [
                "gfs:ProductFamily",
                "skos:Concept"
            ],
            "gfs:level": 2,
            "gfs:typecode": "EMCFILT",
            "rdfs:comment": "Accessories",
            "skos:inScheme": "https://grundfos.com/concept/productFamily",
            "skos:prefLabel": "EMC-filter"
        },
        {
            "@id": "https://grundfos.com/concept/productFamily/MODUL",
            "@type": [
                "gfs:ProductFamily",
                "skos:Concept"
            ],
            "gfs:level": 2,
            "gfs:typecode": "MODUL",
            "rdfs:comment": "Accessories",
            "skos:inScheme": "https://grundfos.com/concept/productFamily",
            "skos:prefLabel": "Expansion modules"
        },
        {
            "@id": "https://grundfos.com/concept/productFamily/FACTORY",
            "@type": [
                "gfs:ProductFamily",
                "skos:Concept"
            ],
            "gfs:level": 2,
            "gfs:typecode": "FACTORY",
            "rdfs:comment": "Accessories",
            "skos:inScheme": "https://grundfos.com/concept/productFamily",
            "skos:prefLabel": "Factory-fitted for Hydro MPC or Hydro 2000"
        },
        {
            "@id": "https://grundfos.com/concept/productFamily/G10LON",
            "@type": [
                "gfs:ProductFamily",
                "skos:Concept"
            ],
            "gfs:level": 2,
            "gfs:typecode": "G10LON",
            "rdfs:comment": "Accessories",
            "skos:inScheme": "https://grundfos.com/concept/productFamily",
            "skos:prefLabel": "G10-LON"
        },
        {
            "@id": "https://grundfos.com/concept/productFamily/IO50",
            "@type": [
                "gfs:ProductFamily",
                "skos:Concept"
            ],
            "gfs:level": 2,
            "gfs:typecode": "IO50",
            "rdfs:comment": "Accessories",
            "skos:inScheme": "https://grundfos.com/concept/productFamily",
            "skos:prefLabel": "IO 50"
        },
        {
            "@id": "https://grundfos.com/concept/productFamily/IO100",
            "@type": [
                "gfs:ProductFamily",
                "skos:Concept"
            ],
            "gfs:level": 2,
            "gfs:typecode": "IO100",
            "rdfs:comment": "Accessories",
            "skos:inScheme": "https://grundfos.com/concept/productFamily",
            "skos:prefLabel": "IO 101, IO 102"
        },
        {
            "@id": "https://grundfos.com/concept/productFamily/LCACC",
            "@type": [
                "gfs:ProductFamily",
                "skos:Concept"
            ],
            "gfs:level": 2,
            "gfs:typecode": "LCACC",
            "rdfs:comment": "Accessories",
            "skos:inScheme": "https://grundfos.com/concept/productFamily",
            "skos:prefLabel": "LC, LCD accessories"
        },
        {
            "@id": "https://grundfos.com/concept/productFamily/LEVELSEN",
            "@type": [
                "gfs:ProductFamily",
                "skos:Concept"
            ],
            "gfs:level": 2,
            "gfs:typecode": "LEVELSEN",
            "rdfs:comment": "Accessories",
            "skos:inScheme": "https://grundfos.com/concept/productFamily",
            "skos:prefLabel": "Level sensor/switch"
        },
        {
            "@id": "https://grundfos.com/concept/productFamily/LIQTEC",
            "@type": [
                "gfs:ProductFamily",
                "skos:Concept"
            ],
            "gfs:level": 2,
            "gfs:typecode": "LIQTEC",
            "rdfs:comment": "Accessories",
            "skos:inScheme": "https://grundfos.com/concept/productFamily",
            "skos:prefLabel": "LiqTec"
        },
        {
            "@id": "https://grundfos.com/concept/productFamily/MGEACC",
            "@type": [
                "gfs:ProductFamily",
                "skos:Concept"
            ],
            "gfs:level": 2,
            "gfs:typecode": "MGEACC",
            "rdfs:comment": "Accessories",
            "skos:inScheme": "https://grundfos.com/concept/productFamily",
            "skos:prefLabel": "MGE, MLE accessories"
        },
        {
            "@id": "https://grundfos.com/concept/productFamily/STARTER",
            "@type": [
                "gfs:ProductFamily",
                "skos:Concept"
            ],
            "gfs:level": 2,
            "gfs:typecode": "STARTER",
            "rdfs:comment": "Accessories",
            "skos:inScheme": "https://grundfos.com/concept/productFamily",
            "skos:prefLabel": "Motor starters"
        },
        {
            "@id": "https://grundfos.com/concept/productFamily/PCTOOL",
            "@type": [
                "gfs:ProductFamily",
                "skos:Concept"
            ],
            "gfs:level": 2,
            "gfs:typecode": "PCTOOL",
            "rdfs:comment": "Accessories",
            "skos:inScheme": "https://grundfos.com/concept/productFamily",
            "skos:prefLabel": "PC-Tool"
        },
        {
            "@id": "https://grundfos.com/concept/productFamily/PLUG",
            "@type": [
                "gfs:ProductFamily",
                "skos:Concept"
            ],
            "gfs:level": 2,
            "gfs:typecode": "PLUG",
            "rdfs:comment": "Accessories",
            "skos:inScheme": "https://grundfos.com/concept/productFamily",
            "skos:prefLabel": "Plugs"
        },
        {
            "@id": "https://grundfos.com/concept/productFamily/POTENTIM",
            "@type": [
                "gfs:ProductFamily",
                "skos:Concept"
            ],
            "gfs:level": 2,
            "gfs:typecode": "POTENTIM",
            "rdfs:comment": "Accessories",
            "skos:inScheme": "https://grundfos.com/concept/productFamily",
            "skos:prefLabel": "Potentiometer"
        },
        {
            "@id": "https://grundfos.com/concept/productFamily/R100",
            "@type": [
                "gfs:ProductFamily",
                "skos:Concept"
            ],
            "gfs:level": 2,
            "gfs:typecode": "R100",
            "rdfs:comment": "Grundfos remote controls used for installation, data monitoring, fault information and configuration of Grundfos pumps and systems, by radio or IR connections.",
            "skos:inScheme": "https://grundfos.com/concept/productFamily",
            "skos:prefLabel": "Remote controls"
        },
        {
            "@id": "https://grundfos.com/concept/productFamily/RENWACC",
            "@type": [
                "gfs:ProductFamily",
                "skos:Concept"
            ],
            "gfs:level": 2,
            "gfs:typecode": "RENWACC",
            "rdfs:comment": "Accessories",
            "skos:inScheme": "https://grundfos.com/concept/productFamily",
            "skos:prefLabel": "Renewable accessories"
        },
        {
            "@id": "https://grundfos.com/concept/productFamily/RMQACC",
            "@type": [
                "gfs:ProductFamily",
                "skos:Concept"
            ],
            "gfs:level": 2,
            "gfs:typecode": "RMQACC",
            "rdfs:comment": "Accessories",
            "skos:inScheme": "https://grundfos.com/concept/productFamily",
            "skos:prefLabel": "RMQ accessories"
        },
        {
            "@id": "https://grundfos.com/concept/productFamily/SENSORS",
            "@type": [
                "gfs:ProductFamily",
                "skos:Concept"
            ],
            "gfs:level": 2,
            "gfs:typecode": "SENSORS",
            "rdfs:comment": "Accessories",
            "skos:inScheme": "https://grundfos.com/concept/productFamily",
            "skos:prefLabel": "Sensors"
        },
        {
            "@id": "https://grundfos.com/concept/productFamily/SOLARPA",
            "@type": [
                "gfs:ProductFamily",
                "skos:Concept"
            ],
            "gfs:level": 2,
            "gfs:typecode": "SOLARPA",
            "rdfs:comment": "Accessories",
            "skos:inScheme": "https://grundfos.com/concept/productFamily",
            "skos:prefLabel": "Solar panel accessories"
        },
        {
            "@id": "https://grundfos.com/concept/productFamily/DROPCAB",
            "@type": [
                "gfs:ProductFamily",
                "skos:Concept"
            ],
            "gfs:level": 2,
            "gfs:typecode": "DROPCAB",
            "rdfs:comment": "Accessories",
            "skos:inScheme": "https://grundfos.com/concept/productFamily",
            "skos:prefLabel": "Submersible drop cables"
        },
        {
            "@id": "https://grundfos.com/concept/productFamily/TERMBOX",
            "@type": [
                "gfs:ProductFamily",
                "skos:Concept"
            ],
            "gfs:level": 2,
            "gfs:typecode": "TERMBOX",
            "rdfs:comment": "Accessories",
            "skos:inScheme": "https://grundfos.com/concept/productFamily",
            "skos:prefLabel": "Terminal boxes"
        },
        {
            "@id": "https://grundfos.com/concept/productFamily/TIMER",
            "@type": [
                "gfs:ProductFamily",
                "skos:Concept"
            ],
            "gfs:level": 2,
            "gfs:typecode": "TIMER",
            "rdfs:comment": "Accessories",
            "skos:inScheme": "https://grundfos.com/concept/productFamily",
            "skos:prefLabel": "Time switches"
        },
        {
            "@id": "https://grundfos.com/concept/productFamily/WINDTURB",
            "@type": [
                "gfs:ProductFamily",
                "skos:Concept"
            ],
            "gfs:level": 2,
            "gfs:typecode": "WINDTURB",
            "rdfs:comment": "Accessories",
            "skos:inScheme": "https://grundfos.com/concept/productFamily",
            "skos:prefLabel": "Wind turbine accessories"
        },
        {
            "@id": "https://grundfos.com/concept/productFamily/ELACC",
            "@type": [
                "gfs:ProductFamily",
                "skos:Concept"
            ],
            "gfs:level": 1,
            "gfs:typecode": "ELACC",
            "rdfs:comment": "Accessories",
            "skos:inScheme": "https://grundfos.com/concept/productFamily",
            "skos:narrower": [
                "https://grundfos.com/concept/productFamily/PCB",
                "https://grundfos.com/concept/productFamily/CABLEKIT",
                "https://grundfos.com/concept/productFamily/CAPACIT",
                "https://grundfos.com/concept/productFamily/CONTBOX",
                "https://grundfos.com/concept/productFamily/CU100",
                "https://grundfos.com/concept/productFamily/CU200",
                "https://grundfos.com/concept/productFamily/CU300",
                "https://grundfos.com/concept/productFamily/CU300AC",
                "https://grundfos.com/concept/productFamily/CU301",
                "https://grundfos.com/concept/productFamily/CUEFAM",
                "https://grundfos.com/concept/productFamily/CUEAC",
                "https://grundfos.com/concept/productFamily/ELCB",
                "https://grundfos.com/concept/productFamily/EMCFILT",
                "https://grundfos.com/concept/productFamily/MODUL",
                "https://grundfos.com/concept/productFamily/FACTORY",
                "https://grundfos.com/concept/productFamily/G10LON",
                "https://grundfos.com/concept/productFamily/IO50",
                "https://grundfos.com/concept/productFamily/IO100",
                "https://grundfos.com/concept/productFamily/LCACC",
                "https://grundfos.com/concept/productFamily/LEVELSEN",
                "https://grundfos.com/concept/productFamily/LIQTEC",
                "https://grundfos.com/concept/productFamily/MGEACC",
                "https://grundfos.com/concept/productFamily/STARTER",
                "https://grundfos.com/concept/productFamily/PCTOOL",
                "https://grundfos.com/concept/productFamily/PLUG",
                "https://grundfos.com/concept/productFamily/POTENTIM",
                "https://grundfos.com/concept/productFamily/R100",
                "https://grundfos.com/concept/productFamily/RENWACC",
                "https://grundfos.com/concept/productFamily/RMQACC",
                "https://grundfos.com/concept/productFamily/SENSORS",
                "https://grundfos.com/concept/productFamily/SOLARPA",
                "https://grundfos.com/concept/productFamily/DROPCAB",
                "https://grundfos.com/concept/productFamily/TERMBOX",
                "https://grundfos.com/concept/productFamily/TIMER",
                "https://grundfos.com/concept/productFamily/WINDTURB"
            ],
            "skos:prefLabel": "Accessories, electrical"
        },
        {
            "@id": "https://grundfos.com/concept/productFamily/ANODES",
            "@type": [
                "gfs:ProductFamily",
                "skos:Concept"
            ],
            "gfs:level": 2,
            "gfs:typecode": "ANODES",
            "rdfs:comment": "Accessories",
            "skos:inScheme": "https://grundfos.com/concept/productFamily",
            "skos:prefLabel": "Anode strings"
        },
        {
            "@id": "https://grundfos.com/concept/productFamily/AUTAIR",
            "@type": [
                "gfs:ProductFamily",
                "skos:Concept"
            ],
            "gfs:level": 2,
            "gfs:typecode": "AUTAIR",
            "rdfs:comment": "Accessories",
            "skos:inScheme": "https://grundfos.com/concept/productFamily",
            "skos:prefLabel": "Automatic air control device"
        },
        {
            "@id": "https://grundfos.com/concept/productFamily/BASEPL",
            "@type": [
                "gfs:ProductFamily",
                "skos:Concept"
            ],
            "gfs:level": 2,
            "gfs:typecode": "BASEPL",
            "rdfs:comment": "Accessories",
            "skos:inScheme": "https://grundfos.com/concept/productFamily",
            "skos:prefLabel": "Base plates"
        },
        {
            "@id": "https://grundfos.com/concept/productFamily/BLANKFL",
            "@type": [
                "gfs:ProductFamily",
                "skos:Concept"
            ],
            "gfs:level": 2,
            "gfs:typecode": "BLANKFL",
            "rdfs:comment": "Accessories",
            "skos:inScheme": "https://grundfos.com/concept/productFamily",
            "skos:prefLabel": "Blanking flanges"
        },
        {
            "@id": "https://grundfos.com/concept/productFamily/BRACKET",
            "@type": [
                "gfs:ProductFamily",
                "skos:Concept"
            ],
            "gfs:level": 2,
            "gfs:typecode": "BRACKET",
            "rdfs:comment": "Accessories",
            "skos:inScheme": "https://grundfos.com/concept/productFamily",
            "skos:prefLabel": "Brackets"
        },
        {
            "@id": "https://grundfos.com/concept/productFamily/FACTOMEC",
            "@type": [
                "gfs:ProductFamily",
                "skos:Concept"
            ],
            "gfs:level": 2,
            "gfs:typecode": "FACTOMEC",
            "rdfs:comment": "Accessories",
            "skos:inScheme": "https://grundfos.com/concept/productFamily",
            "skos:prefLabel": "Factory-fitted for Hydro MPC or Hydro 2000"
        },
        {
            "@id": "https://grundfos.com/concept/productFamily/FLOWSLAC",
            "@type": [
                "gfs:ProductFamily",
                "skos:Concept"
            ],
            "gfs:level": 2,
            "gfs:typecode": "FLOWSLAC",
            "rdfs:comment": "Accessories",
            "skos:inScheme": "https://grundfos.com/concept/productFamily",
            "skos:prefLabel": "Flow sleeve accessories"
        },
        {
            "@id": "https://grundfos.com/concept/productFamily/FLOWSLE",
            "@type": [
                "gfs:ProductFamily",
                "skos:Concept"
            ],
            "gfs:level": 2,
            "gfs:typecode": "FLOWSLE",
            "rdfs:comment": "Accessories",
            "skos:inScheme": "https://grundfos.com/concept/productFamily",
            "skos:prefLabel": "Flow sleeves"
        },
        {
            "@id": "https://grundfos.com/concept/productFamily/INSULKI",
            "@type": [
                "gfs:ProductFamily",
                "skos:Concept"
            ],
            "gfs:level": 2,
            "gfs:typecode": "INSULKI",
            "rdfs:comment": "Accessories",
            "skos:inScheme": "https://grundfos.com/concept/productFamily",
            "skos:prefLabel": "Insulation kits"
        },
        {
            "@id": "https://grundfos.com/concept/productFamily/MACSHOE",
            "@type": [
                "gfs:ProductFamily",
                "skos:Concept"
            ],
            "gfs:level": 2,
            "gfs:typecode": "MACSHOE",
            "rdfs:comment": "Machine shoes reduce any vibrations from the system to the floor, allowing the system to be height-adjusted by \u00c3\u201a\u00c2\u00b1 20 mm",
            "skos:inScheme": "https://grundfos.com/concept/productFamily",
            "skos:prefLabel": "Machine shoe"
        },
        {
            "@id": "https://grundfos.com/concept/productFamily/PIPECON",
            "@type": [
                "gfs:ProductFamily",
                "skos:Concept"
            ],
            "gfs:level": 2,
            "gfs:typecode": "PIPECON",
            "rdfs:comment": "Accessories",
            "skos:inScheme": "https://grundfos.com/concept/productFamily",
            "skos:prefLabel": "Pipe connections"
        },
        {
            "@id": "https://grundfos.com/concept/productFamily/PRESCON",
            "@type": [
                "gfs:ProductFamily",
                "skos:Concept"
            ],
            "gfs:level": 2,
            "gfs:typecode": "PRESCON",
            "rdfs:comment": "Accessories",
            "skos:inScheme": "https://grundfos.com/concept/productFamily",
            "skos:prefLabel": "Pressure control units"
        },
        {
            "@id": "https://grundfos.com/concept/productFamily/PREEXCH",
            "@type": [
                "gfs:ProductFamily",
                "skos:Concept"
            ],
            "gfs:level": 2,
            "gfs:typecode": "PREEXCH",
            "rdfs:comment": "Pressure exchanger for BMSX systems",
            "skos:inScheme": "https://grundfos.com/concept/productFamily",
            "skos:prefLabel": "Pressure exchanger"
        },
        {
            "@id": "https://grundfos.com/concept/productFamily/PREGAUG",
            "@type": [
                "gfs:ProductFamily",
                "skos:Concept"
            ],
            "gfs:level": 2,
            "gfs:typecode": "PREGAUG",
            "rdfs:comment": "Accessories",
            "skos:inScheme": "https://grundfos.com/concept/productFamily",
            "skos:prefLabel": "Pressure gauges"
        },
        {
            "@id": "https://grundfos.com/concept/productFamily/SHRIMS",
            "@type": [
                "gfs:ProductFamily",
                "skos:Concept"
            ],
            "gfs:level": 2,
            "gfs:typecode": "SHRIMS",
            "rdfs:comment": "Accessories",
            "skos:inScheme": "https://grundfos.com/concept/productFamily",
            "skos:prefLabel": "Shims"
        },
        {
            "@id": "https://grundfos.com/concept/productFamily/FLOWJET",
            "@type": [
                "gfs:ProductFamily",
                "skos:Concept"
            ],
            "gfs:level": 2,
            "gfs:typecode": "FLOWJET",
            "rdfs:comment": "Accessories",
            "skos:inScheme": "https://grundfos.com/concept/productFamily",
            "skos:prefLabel": "Shut-off and evacuation fitting"
        },
        {
            "@id": "https://grundfos.com/concept/productFamily/VIBDAMP",
            "@type": [
                "gfs:ProductFamily",
                "skos:Concept"
            ],
            "gfs:level": 2,
            "gfs:typecode": "VIBDAMP",
            "rdfs:comment": "Accessories",
            "skos:inScheme": "https://grundfos.com/concept/productFamily",
            "skos:prefLabel": "Vibration dampers"
        },
        {
            "@id": "https://grundfos.com/concept/productFamily/WATERLEV",
            "@type": [
                "gfs:ProductFamily",
                "skos:Concept"
            ],
            "gfs:level": 2,
            "gfs:typecode": "WATERLEV",
            "rdfs:comment": "Accessories",
            "skos:inScheme": "https://grundfos.com/concept/productFamily",
            "skos:prefLabel": "Water level indicators"
        },
        {
            "@id": "https://grundfos.com/concept/productFamily/WIRE",
            "@type": [
                "gfs:ProductFamily",
                "skos:Concept"
            ],
            "gfs:level": 2,
            "gfs:typecode": "WIRE",
            "rdfs:comment": "Accessories",
            "skos:inScheme": "https://grundfos.com/concept/productFamily",
            "skos:prefLabel": "Wires and chains"
        },
        {
            "@id": "https://grundfos.com/concept/productFamily/MECACC",
            "@type": [
                "gfs:ProductFamily",
                "skos:Concept"
            ],
            "gfs:level": 1,
            "gfs:typecode": "MECACC",
            "rdfs:comment": "Accessories",
            "skos:inScheme": "https://grundfos.com/concept/productFamily",
            "skos:narrower": [
                "https://grundfos.com/concept/productFamily/ANODES",
                "https://grundfos.com/concept/productFamily/AUTAIR",
                "https://grundfos.com/concept/productFamily/BASEPL",
                "https://grundfos.com/concept/productFamily/BLANKFL",
                "https://grundfos.com/concept/productFamily/BRACKET",
                "https://grundfos.com/concept/productFamily/FACTOMEC",
                "https://grundfos.com/concept/productFamily/FLOWSLAC",
                "https://grundfos.com/concept/productFamily/FLOWSLE",
                "https://grundfos.com/concept/productFamily/INSULKI",
                "https://grundfos.com/concept/productFamily/MACSHOE",
                "https://grundfos.com/concept/productFamily/PIPECON",
                "https://grundfos.com/concept/productFamily/PRESCON",
                "https://grundfos.com/concept/productFamily/PREEXCH",
                "https://grundfos.com/concept/productFamily/PREGAUG",
                "https://grundfos.com/concept/productFamily/SHRIMS",
                "https://grundfos.com/concept/productFamily/FLOWJET",
                "https://grundfos.com/concept/productFamily/VIBDAMP",
                "https://grundfos.com/concept/productFamily/WATERLEV",
                "https://grundfos.com/concept/productFamily/WIRE"
            ],
            "skos:prefLabel": "Accessories, mechanical"
        },
        {
            "@id": "https://grundfos.com/concept/productFamily/LIFTACC",
            "@type": [
                "gfs:ProductFamily",
                "skos:Concept"
            ],
            "gfs:level": 2,
            "gfs:typecode": "LIFTACC",
            "rdfs:comment": "Grundfos LIFTAWAY are collecting tanks designed to be equipped with UNILIFT KP or AP12 to create a lifting station for grey wastewater from floor drains, wash-basins, washing machines, dishwashers, etc. that cannot be connected directly to the sewer.",
            "skos:inScheme": "https://grundfos.com/concept/productFamily",
            "skos:prefLabel": "Liftaway"
        },
        {
            "@id": "https://grundfos.com/concept/productFamily/LIPEACC",
            "@type": [
                "gfs:ProductFamily",
                "skos:Concept"
            ],
            "gfs:level": 2,
            "gfs:typecode": "LIPEACC",
            "rdfs:comment": "Accessories",
            "skos:inScheme": "https://grundfos.com/concept/productFamily",
            "skos:prefLabel": "Lifting station PE"
        },
        {
            "@id": "https://grundfos.com/concept/productFamily/PEFLACC",
            "@type": [
                "gfs:ProductFamily",
                "skos:Concept"
            ],
            "gfs:level": 2,
            "gfs:typecode": "PEFLACC",
            "rdfs:comment": "Accessories",
            "skos:inScheme": "https://grundfos.com/concept/productFamily",
            "skos:prefLabel": "Lifting- and pumping stations accessories"
        },
        {
            "@id": "https://grundfos.com/concept/productFamily/UNIT",
            "@type": [
                "gfs:ProductFamily",
                "skos:Concept"
            ],
            "gfs:level": 2,
            "gfs:typecode": "UNIT",
            "rdfs:comment": "Accessories",
            "skos:inScheme": "https://grundfos.com/concept/productFamily",
            "skos:prefLabel": "Neutralisation Unit"
        },
        {
            "@id": "https://grundfos.com/concept/productFamily/PITACC",
            "@type": [
                "gfs:ProductFamily",
                "skos:Concept"
            ],
            "gfs:level": 1,
            "gfs:typecode": "PITACC",
            "rdfs:comment": "Accessories",
            "skos:inScheme": "https://grundfos.com/concept/productFamily",
            "skos:narrower": [
                "https://grundfos.com/concept/productFamily/LIFTACC",
                "https://grundfos.com/concept/productFamily/LIPEACC",
                "https://grundfos.com/concept/productFamily/PEFLACC",
                "https://grundfos.com/concept/productFamily/UNIT"
            ],
            "skos:prefLabel": "Accessories, prefabricated pumping systems"
        },
        {
            "@id": "https://grundfos.com/concept/productFamily/GAMACC",
            "@type": [
                "gfs:ProductFamily",
                "skos:Concept"
            ],
            "gfs:level": 2,
            "gfs:typecode": "GAMACC",
            "rdfs:comment": "Accessories",
            "skos:inScheme": "https://grundfos.com/concept/productFamily",
            "skos:prefLabel": "Accessories, AMD, AMG, AFG, SRP, SMG, SFG, SRG"
        },
        {
            "@id": "https://grundfos.com/concept/productFamily/AXIACC",
            "@type": [
                "gfs:ProductFamily",
                "skos:Concept"
            ],
            "gfs:level": 2,
            "gfs:typecode": "AXIACC",
            "rdfs:comment": "Accessories designed for axial flow pumps",
            "skos:inScheme": "https://grundfos.com/concept/productFamily",
            "skos:prefLabel": "Accessories, axial flow pumps"
        },
        {
            "@id": "https://grundfos.com/concept/productFamily/UNILACC",
            "@type": [
                "gfs:ProductFamily",
                "skos:Concept"
            ],
            "gfs:level": 2,
            "gfs:typecode": "UNILACC",
            "rdfs:comment": "Accessories",
            "skos:inScheme": "https://grundfos.com/concept/productFamily",
            "skos:prefLabel": "Accessories, Drainage and Lifting Stations"
        },
        {
            "@id": "https://grundfos.com/concept/productFamily/MLIFTACC",
            "@type": [
                "gfs:ProductFamily",
                "skos:Concept"
            ],
            "gfs:level": 2,
            "gfs:typecode": "MLIFTACC",
            "rdfs:comment": "Accessories",
            "skos:inScheme": "https://grundfos.com/concept/productFamily",
            "skos:prefLabel": "Accessories, MSS/M/MOG/MD/MLD/MDG/MD1/MDV"
        },
        {
            "@id": "https://grundfos.com/concept/productFamily/CHAACC",
            "@type": [
                "gfs:ProductFamily",
                "skos:Concept"
            ],
            "gfs:level": 2,
            "gfs:typecode": "CHAACC",
            "rdfs:comment": "Lifting chains are designed to lift and lower the pumps into water and wastewater segments.",
            "skos:inScheme": "https://grundfos.com/concept/productFamily",
            "skos:prefLabel": "Chains"
        },
        {
            "@id": "https://grundfos.com/concept/productFamily/FLATAPER",
            "@type": [
                "gfs:ProductFamily",
                "skos:Concept"
            ],
            "gfs:level": 2,
            "gfs:typecode": "FLATAPER",
            "rdfs:comment": "Flanged taper is used as an expansion cone to bridge gaps in pipelines for water and wastewater segments.",
            "skos:inScheme": "https://grundfos.com/concept/productFamily",
            "skos:prefLabel": "Flanged taper"
        },
        {
            "@id": "https://grundfos.com/concept/productFamily/DIAACC",
            "@type": [
                "gfs:ProductFamily",
                "skos:Concept"
            ],
            "gfs:level": 2,
            "gfs:typecode": "DIAACC",
            "rdfs:comment": "Accessories",
            "skos:inScheme": "https://grundfos.com/concept/productFamily",
            "skos:prefLabel": "Manual diaphram pumps"
        },
        {
            "@id": "https://grundfos.com/concept/productFamily/PUMACC",
            "@type": [
                "gfs:ProductFamily",
                "skos:Concept"
            ],
            "gfs:level": 2,
            "gfs:typecode": "PUMACC",
            "rdfs:comment": "Dry installation vertical, Dry installation horizontal, Submersible pump with autocoupling system",
            "skos:inScheme": "https://grundfos.com/concept/productFamily",
            "skos:prefLabel": "Pump accessories"
        },
        {
            "@id": "https://grundfos.com/concept/productFamily/WASACC",
            "@type": [
                "gfs:ProductFamily",
                "skos:Concept"
            ],
            "gfs:level": 1,
            "gfs:typecode": "WASACC",
            "rdfs:comment": "Accessories designed for wastewater solutions.",
            "skos:inScheme": "https://grundfos.com/concept/productFamily",
            "skos:narrower": [
                "https://grundfos.com/concept/productFamily/GAMACC",
                "https://grundfos.com/concept/productFamily/AXIACC",
                "https://grundfos.com/concept/productFamily/UNILACC",
                "https://grundfos.com/concept/productFamily/MLIFTACC",
                "https://grundfos.com/concept/productFamily/CHAACC",
                "https://grundfos.com/concept/productFamily/FLATAPER",
                "https://grundfos.com/concept/productFamily/DIAACC",
                "https://grundfos.com/concept/productFamily/PUMACC"
            ],
            "skos:prefLabel": "Accessories, Waste Water"
        },
        {
            "@id": "https://grundfos.com/concept/productFamily/AFG00",
            "@type": [
                "gfs:ProductFamily",
                "skos:Concept"
            ],
            "gfs:level": 2,
            "gfs:typecode": "AFG00",
            "rdfs:comment": "The Grundfos range of horizontal, planetary gear drive AFG flowmakers are designed for flowmaking, i.e. keeping liquids moving in low/medium viscosity liquids. Fitted with motors of 1.5-7.5 kW.",
            "skos:inScheme": "https://grundfos.com/concept/productFamily",
            "skos:prefLabel": "AFG"
        },
        {
            "@id": "https://grundfos.com/concept/productFamily/AMD07",
            "@type": [
                "gfs:ProductFamily",
                "skos:Concept"
            ],
            "gfs:level": 2,
            "gfs:typecode": "AMD07",
            "rdfs:comment": "Grundfos submersible, direct driven AMD mixers are designed for mixing, i.e. homogenisation and suspension of low/medium viscosity liquids in small tanks and pumping stations.",
            "skos:inScheme": "https://grundfos.com/concept/productFamily",
            "skos:prefLabel": "AMD"
        },
        {
            "@id": "https://grundfos.com/concept/productFamily/AMG00",
            "@type": [
                "gfs:ProductFamily",
                "skos:Concept"
            ],
            "gfs:level": 2,
            "gfs:typecode": "AMG00",
            "rdfs:comment": "The Grundfos range of horizontal, planetary gear drive AMG mixers are designed for mixing, i.e. homogenisation and suspension of low/ medium viscosity liquids. Fitted with motors of 0.75-18.5 kW.",
            "skos:inScheme": "https://grundfos.com/concept/productFamily",
            "skos:prefLabel": "AMG"
        },
        {
            "@id": "https://grundfos.com/concept/productFamily/SFG00",
            "@type": [
                "gfs:ProductFamily",
                "skos:Concept"
            ],
            "gfs:level": 2,
            "gfs:typecode": "SFG00",
            "rdfs:comment": "The Grundfos range of horizontal, planetary gear drive SFG flowmakers are designed for flowmaking, i.e. keeping liquids moving in low/medium viscosity liquids. Suitable for use in large volumes. Fitted with motors of 0.7-8.0 kW.",
            "skos:inScheme": "https://grundfos.com/concept/productFamily",
            "skos:prefLabel": "SFG"
        },
        {
            "@id": "https://grundfos.com/concept/productFamily/SMD00",
            "@type": [
                "gfs:ProductFamily",
                "skos:Concept"
            ],
            "gfs:level": 2,
            "gfs:typecode": "SMD00",
            "rdfs:comment": "The Grundfos range of horizontal, direct drive SMD mixers are designed for mixing, i.e. homogenisation and suspension of low/medium viscosity liquids. Fitted with motors of 0.9-3.5 kW.",
            "skos:inScheme": "https://grundfos.com/concept/productFamily",
            "skos:prefLabel": "SMD"
        },
        {
            "@id": "https://grundfos.com/concept/productFamily/SMG00",
            "@type": [
                "gfs:ProductFamily",
                "skos:Concept"
            ],
            "gfs:level": 2,
            "gfs:typecode": "SMG00",
            "rdfs:comment": "The Grundfos range of horizontal, planetary gear drive SMG mixers are designed for mixing, i.e. homogenisation and suspension of low/medium viscosity liquids. Fitted with motors of 0.9-18.0 kW.",
            "skos:inScheme": "https://grundfos.com/concept/productFamily",
            "skos:prefLabel": "SMG"
        },
        {
            "@id": "https://grundfos.com/concept/productFamily/SRG00",
            "@type": [
                "gfs:ProductFamily",
                "skos:Concept"
            ],
            "gfs:level": 2,
            "gfs:typecode": "SRG00",
            "rdfs:comment": "Grundfos SRG recirculation pumps are designed for the pumping of sludge from one tank to another in sewage treatment plants and for other pump applications involving a high flow rate and low head.",
            "skos:inScheme": "https://grundfos.com/concept/productFamily",
            "skos:prefLabel": "SRG"
        },
        {
            "@id": "https://grundfos.com/concept/productFamily/AGIFAM",
            "@type": [
                "gfs:ProductFamily",
                "skos:Concept"
            ],
            "gfs:level": 1,
            "gfs:typecode": "AGIFAM",
            "rdfs:comment": "Mixers and flowmakers for mixing and keeping media in suspension",
            "skos:inScheme": "https://grundfos.com/concept/productFamily",
            "skos:narrower": [
                "https://grundfos.com/concept/productFamily/AFG00",
                "https://grundfos.com/concept/productFamily/AMD07",
                "https://grundfos.com/concept/productFamily/AMG00",
                "https://grundfos.com/concept/productFamily/SFG00",
                "https://grundfos.com/concept/productFamily/SMD00",
                "https://grundfos.com/concept/productFamily/SMG00",
                "https://grundfos.com/concept/productFamily/SRG00"
            ],
            "skos:prefLabel": "Agitators"
        },
        {
            "@id": "https://grundfos.com/concept/productFamily/ALPSOL",
            "@type": [
                "gfs:ProductFamily",
                "skos:Concept"
            ],
            "gfs:level": 2,
            "gfs:typecode": "ALPSOL",
            "rdfs:comment": "Grundfos ALPHA SOLAR pumps are high-efficiency circulators designed to be integrated in all types of thermal solar systems.",
            "skos:inScheme": "https://grundfos.com/concept/productFamily",
            "skos:prefLabel": "ALPHA SOLAR"
        },
        {
            "@id": "https://grundfos.com/concept/productFamily/ALPHA1",
            "@type": [
                "gfs:ProductFamily",
                "skos:Concept"
            ],
            "gfs:level": 2,
            "gfs:typecode": "ALPHA1",
            "rdfs:comment": "Grundfos ALPHA1 pumps are high-efficiency circulators, designed for heating systems. The ideal choice for basic functionality needs.",
            "skos:inScheme": "https://grundfos.com/concept/productFamily",
            "skos:prefLabel": "ALPHA1"
        },
        {
            "@id": "https://grundfos.com/concept/productFamily/ALPHA1L",
            "@type": [
                "gfs:ProductFamily",
                "skos:Concept"
            ],
            "gfs:level": 2,
            "gfs:typecode": "ALPHA1L",
            "rdfs:comment": "Grundfos ALPHA1 L pumps are high-efficiency circulators, designed for heating systems. Applicable as a universal upgrade and replacement pump.",
            "skos:inScheme": "https://grundfos.com/concept/productFamily",
            "skos:prefLabel": "ALPHA1 L"
        },
        {
            "@id": "https://grundfos.com/concept/productFamily/ALPHA1N",
            "@type": [
                "gfs:ProductFamily",
                "skos:Concept"
            ],
            "gfs:level": 2,
            "gfs:typecode": "ALPHA1N",
            "rdfs:comment": "Grundfos ALPHA1 N pumps are high-efficiency circulators with stainless-steel pump housing, designed for heating systems. And suitable for domestic hot water systems. The ideal choice for basic functionality needs.",
            "skos:inScheme": "https://grundfos.com/concept/productFamily",
            "skos:prefLabel": "ALPHA1 N"
        },
        {
            "@id": "https://grundfos.com/concept/productFamily/ALPHA2",
            "@type": [
                "gfs:ProductFamily",
                "skos:Concept"
            ],
            "gfs:level": 2,
            "gfs:typecode": "ALPHA2",
            "rdfs:comment": "Grundfos ALPHA2 pumps are high-efficiency circulators, designed for heating and air-conditioning systems. The pump features AUTOADAPT which automatically adjusts the pump to system demands for optimal comfort and the lowest energy consumption as well as simple commissioning.",
            "skos:inScheme": "https://grundfos.com/concept/productFamily",
            "skos:prefLabel": "ALPHA2"
        },
        {
            "@id": "https://grundfos.com/concept/productFamily/ALPHA2N",
            "@type": [
                "gfs:ProductFamily",
                "skos:Concept"
            ],
            "gfs:level": 2,
            "gfs:typecode": "ALPHA2N",
            "rdfs:comment": "Grundfos ALPHA2 N pumps are high-efficiency circulators with stainless-steel pump housing, designed for heating, air-conditioning and domestic hot water systems. The pump features AUTOADAPT which automatically adjusts the pump to system demands for optimal comfort and the lowest energy consumption as well as simple commissioning.",
            "skos:inScheme": "https://grundfos.com/concept/productFamily",
            "skos:prefLabel": "ALPHA2 N"
        },
        {
            "@id": "https://grundfos.com/concept/productFamily/ALPHA3",
            "@type": [
                "gfs:ProductFamily",
                "skos:Concept"
            ],
            "gfs:level": 2,
            "gfs:typecode": "ALPHA3",
            "rdfs:comment": "Grundfos ALPHA3 pumps are high-efficiency circulators, designed for heating systems. The pump features AUTOADAPT which automatically adjusts the pump to system demands for optimal comfort and the lowest energy consumption as well as simple commissioning. Features connectivity to smart devices via Grundfos Apps.",
            "skos:inScheme": "https://grundfos.com/concept/productFamily",
            "skos:prefLabel": "ALPHA3"
        },
        {
            "@id": "https://grundfos.com/concept/productFamily/ALPFAM",
            "@type": [
                "gfs:ProductFamily",
                "skos:Concept"
            ],
            "gfs:level": 1,
            "gfs:typecode": "ALPFAM",
            "rdfs:comment": "Electronically controlled circulator pumps for domestic building",
            "skos:inScheme": "https://grundfos.com/concept/productFamily",
            "skos:narrower": [
                "https://grundfos.com/concept/productFamily/ALPSOL",
                "https://grundfos.com/concept/productFamily/ALPHA1",
                "https://grundfos.com/concept/productFamily/ALPHA1L",
                "https://grundfos.com/concept/productFamily/ALPHA1N",
                "https://grundfos.com/concept/productFamily/ALPHA2",
                "https://grundfos.com/concept/productFamily/ALPHA2N",
                "https://grundfos.com/concept/productFamily/ALPHA3"
            ],
            "skos:prefLabel": "ALPHA"
        },
        {
            "@id": "https://grundfos.com/concept/productFamily/APG00",
            "@type": [
                "gfs:ProductFamily",
                "skos:Concept"
            ],
            "gfs:level": 2,
            "gfs:typecode": "APG00",
            "rdfs:comment": "Grundfos APG pumps are designed for pumping wastewater, sludge-containing water, groundwater, and sewage. Equipped with a cutter system which cuts all destructible solids into small pieces.",
            "skos:inScheme": "https://grundfos.com/concept/productFamily",
            "skos:prefLabel": "APG"
        },
        {
            "@id": "https://grundfos.com/concept/productFamily/APFAM",
            "@type": [
                "gfs:ProductFamily",
                "skos:Concept"
            ],
            "gfs:level": 1,
            "gfs:typecode": "APFAM",
            "rdfs:comment": "APG pumps are designed for pumping wastewater, sludge-containing water, groundwater and sewage. Equipped with a cutter system which cuts all destructible solids into small pieces",
            "skos:inScheme": "https://grundfos.com/concept/productFamily",
            "skos:narrower": [
                "https://grundfos.com/concept/productFamily/APG00"
            ],
            "skos:prefLabel": "AP"
        },
        {
            "@id": "https://grundfos.com/concept/productFamily/AQPACC",
            "@type": [
                "gfs:ProductFamily",
                "skos:Concept"
            ],
            "gfs:level": 2,
            "gfs:typecode": "AQPACC",
            "rdfs:comment": "AQpure is a pre-fabricated, automated and modular water treatment plant that provides reliable and affordable water supply, even in remote areas.",
            "skos:inScheme": "https://grundfos.com/concept/productFamily",
            "skos:prefLabel": "AQpure accessories"
        },
        {
            "@id": "https://grundfos.com/concept/productFamily/AQPURE",
            "@type": [
                "gfs:ProductFamily",
                "skos:Concept"
            ],
            "gfs:level": 2,
            "gfs:typecode": "AQPURE",
            "rdfs:comment": "AQpure is a pre-fabricated, automated and modular water treatment plant that provides reliable and affordable water supply, even in remote areas.",
            "skos:inScheme": "https://grundfos.com/concept/productFamily",
            "skos:prefLabel": "AQpure UF"
        },
        {
            "@id": "https://grundfos.com/concept/productFamily/AQPFAM",
            "@type": [
                "gfs:ProductFamily",
                "skos:Concept"
            ],
            "gfs:level": 1,
            "gfs:typecode": "AQPFAM",
            "rdfs:comment": "AQpure is a pre-fabricated, automated and modular water treatment plant that provides reliable and affordable water supply, even in remote areas.",
            "skos:inScheme": "https://grundfos.com/concept/productFamily",
            "skos:narrower": [
                "https://grundfos.com/concept/productFamily/AQPACC",
                "https://grundfos.com/concept/productFamily/AQPURE"
            ],
            "skos:prefLabel": "AQpure"
        },
        {
            "@id": "https://grundfos.com/concept/productFamily/AQTAP",
            "@type": [
                "gfs:ProductFamily",
                "skos:Concept"
            ],
            "gfs:level": 1,
            "gfs:typecode": "AQTAP",
            "rdfs:comment": "AQtap is an intelligent water dispenser with integrated revenue collection platform for viable and accountable water supply",
            "skos:inScheme": "https://grundfos.com/concept/productFamily",
            "skos:narrower": [],
            "skos:prefLabel": "AQtap"
        },
        {
            "@id": "https://grundfos.com/concept/productFamily/BIOFAM",
            "@type": [
                "gfs:ProductFamily",
                "skos:Concept"
            ],
            "gfs:level": 1,
            "gfs:typecode": "BIOFAM",
            "rdfs:comment": "Grundfos BioBooster is a scalable decentralised wastewater treatment plant built up around stand-alone modules. Based on a membrane biological reactor process and rotating ceramic ultrafiltration membranes, BioBooster plants ensure superior effluent quality for water reuse or safe discharge. Benefits include robustness, reliability, high automation and low operating costs",
            "skos:inScheme": "https://grundfos.com/concept/productFamily",
            "skos:narrower": [],
            "skos:prefLabel": "BioBooster"
        },
        {
            "@id": "https://grundfos.com/concept/productFamily/BM004",
            "@type": [
                "gfs:ProductFamily",
                "skos:Concept"
            ],
            "gfs:level": 2,
            "gfs:typecode": "BM004",
            "rdfs:comment": "Booster modules",
            "skos:inScheme": "https://grundfos.com/concept/productFamily",
            "skos:prefLabel": "BM 4\""
        },
        {
            "@id": "https://grundfos.com/concept/productFamily/BM006",
            "@type": [
                "gfs:ProductFamily",
                "skos:Concept"
            ],
            "gfs:level": 2,
            "gfs:typecode": "BM006",
            "rdfs:comment": "Booster modules",
            "skos:inScheme": "https://grundfos.com/concept/productFamily",
            "skos:prefLabel": "BM 6\""
        },
        {
            "@id": "https://grundfos.com/concept/productFamily/BM008",
            "@type": [
                "gfs:ProductFamily",
                "skos:Concept"
            ],
            "gfs:level": 2,
            "gfs:typecode": "BM008",
            "rdfs:comment": "Booster modules",
            "skos:inScheme": "https://grundfos.com/concept/productFamily",
            "skos:prefLabel": "BM 8\""
        },
        {
            "@id": "https://grundfos.com/concept/productFamily/BMFAM",
            "@type": [
                "gfs:ProductFamily",
                "skos:Concept"
            ],
            "gfs:level": 1,
            "gfs:typecode": "BMFAM",
            "rdfs:comment": "Booster modules",
            "skos:inScheme": "https://grundfos.com/concept/productFamily",
            "skos:narrower": [
                "https://grundfos.com/concept/productFamily/BM004",
                "https://grundfos.com/concept/productFamily/BM006",
                "https://grundfos.com/concept/productFamily/BM008"
            ],
            "skos:prefLabel": "BM"
        },
        {
            "@id": "https://grundfos.com/concept/productFamily/BMHP17",
            "@type": [
                "gfs:ProductFamily",
                "skos:Concept"
            ],
            "gfs:level": 2,
            "gfs:typecode": "BMHP17",
            "rdfs:comment": "Booster modules",
            "skos:inScheme": "https://grundfos.com/concept/productFamily",
            "skos:prefLabel": "BM hp 17"
        },
        {
            "@id": "https://grundfos.com/concept/productFamily/BMHP30",
            "@type": [
                "gfs:ProductFamily",
                "skos:Concept"
            ],
            "gfs:level": 2,
            "gfs:typecode": "BMHP30",
            "rdfs:comment": "Booster modules",
            "skos:inScheme": "https://grundfos.com/concept/productFamily",
            "skos:prefLabel": "BM hp 30"
        },
        {
            "@id": "https://grundfos.com/concept/productFamily/BMHP46",
            "@type": [
                "gfs:ProductFamily",
                "skos:Concept"
            ],
            "gfs:level": 2,
            "gfs:typecode": "BMHP46",
            "rdfs:comment": "Booster modules",
            "skos:inScheme": "https://grundfos.com/concept/productFamily",
            "skos:prefLabel": "BM hp 46"
        },
        {
            "@id": "https://grundfos.com/concept/productFamily/BMHP60",
            "@type": [
                "gfs:ProductFamily",
                "skos:Concept"
            ],
            "gfs:level": 2,
            "gfs:typecode": "BMHP60",
            "rdfs:comment": "Booster modules",
            "skos:inScheme": "https://grundfos.com/concept/productFamily",
            "skos:prefLabel": "BM hp 60"
        },
        {
            "@id": "https://grundfos.com/concept/productFamily/BMHP77",
            "@type": [
                "gfs:ProductFamily",
                "skos:Concept"
            ],
            "gfs:level": 2,
            "gfs:typecode": "BMHP77",
            "rdfs:comment": "Booster modules",
            "skos:inScheme": "https://grundfos.com/concept/productFamily",
            "skos:prefLabel": "BM hp 77"
        },
        {
            "@id": "https://grundfos.com/concept/productFamily/BMHP95",
            "@type": [
                "gfs:ProductFamily",
                "skos:Concept"
            ],
            "gfs:level": 2,
            "gfs:typecode": "BMHP95",
            "rdfs:comment": "Booster modules",
            "skos:inScheme": "https://grundfos.com/concept/productFamily",
            "skos:prefLabel": "BM hp 95"
        },
        {
            "@id": "https://grundfos.com/concept/productFamily/BMHP125",
            "@type": [
                "gfs:ProductFamily",
                "skos:Concept"
            ],
            "gfs:level": 2,
            "gfs:typecode": "BMHP125",
            "rdfs:comment": "Booster modules",
            "skos:inScheme": "https://grundfos.com/concept/productFamily",
            "skos:prefLabel": "BM hp 125"
        },
        {
            "@id": "https://grundfos.com/concept/productFamily/BMHP160",
            "@type": [
                "gfs:ProductFamily",
                "skos:Concept"
            ],
            "gfs:level": 2,
            "gfs:typecode": "BMHP160",
            "rdfs:comment": "Booster modules",
            "skos:inScheme": "https://grundfos.com/concept/productFamily",
            "skos:prefLabel": "BM hp 160"
        },
        {
            "@id": "https://grundfos.com/concept/productFamily/BMHP215",
            "@type": [
                "gfs:ProductFamily",
                "skos:Concept"
            ],
            "gfs:level": 2,
            "gfs:typecode": "BMHP215",
            "rdfs:comment": "Booster modules",
            "skos:inScheme": "https://grundfos.com/concept/productFamily",
            "skos:prefLabel": "BM hp 215"
        },
        {
            "@id": "https://grundfos.com/concept/productFamily/BMHP00",
            "@type": [
                "gfs:ProductFamily",
                "skos:Concept"
            ],
            "gfs:level": 1,
            "gfs:typecode": "BMHP00",
            "rdfs:comment": "Booster modules",
            "skos:inScheme": "https://grundfos.com/concept/productFamily",
            "skos:narrower": [
                "https://grundfos.com/concept/productFamily/BMHP17",
                "https://grundfos.com/concept/productFamily/BMHP30",
                "https://grundfos.com/concept/productFamily/BMHP46",
                "https://grundfos.com/concept/productFamily/BMHP60",
                "https://grundfos.com/concept/productFamily/BMHP77",
                "https://grundfos.com/concept/productFamily/BMHP95",
                "https://grundfos.com/concept/productFamily/BMHP125",
                "https://grundfos.com/concept/productFamily/BMHP160",
                "https://grundfos.com/concept/productFamily/BMHP215"
            ],
            "skos:prefLabel": "BM hp"
        },
        {
            "@id": "https://grundfos.com/concept/productFamily/BMPFAM",
            "@type": [
                "gfs:ProductFamily",
                "skos:Concept"
            ],
            "gfs:level": 1,
            "gfs:typecode": "BMPFAM",
            "rdfs:comment": "Booster modules",
            "skos:inScheme": "https://grundfos.com/concept/productFamily",
            "skos:narrower": [],
            "skos:prefLabel": "BMP"
        },
        {
            "@id": "https://grundfos.com/concept/productFamily/BMSHPMG",
            "@type": [
                "gfs:ProductFamily",
                "skos:Concept"
            ],
            "gfs:level": 2,
            "gfs:typecode": "BMSHPMG",
            "rdfs:comment": "The BMShp booster module is suitable for industrial and water supply applications where the inlet pressure is up to 80 bar. The booster modules are used to increase the system pressure.",
            "skos:inScheme": "https://grundfos.com/concept/productFamily",
            "skos:prefLabel": "BMS hp MG"
        },
        {
            "@id": "https://grundfos.com/concept/productFamily/BMSHP",
            "@type": [
                "gfs:ProductFamily",
                "skos:Concept"
            ],
            "gfs:level": 2,
            "gfs:typecode": "BMSHP",
            "rdfs:comment": "The BMShp booster module is suitable for industrial and water supply applications where the inlet pressure is up to 80 bar. The booster modules are used to increase the system pressure.",
            "skos:inScheme": "https://grundfos.com/concept/productFamily",
            "skos:prefLabel": "BMS hp MGE"
        },
        {
            "@id": "https://grundfos.com/concept/productFamily/BMSHSAC",
            "@type": [
                "gfs:ProductFamily",
                "skos:Concept"
            ],
            "gfs:level": 2,
            "gfs:typecode": "BMSHSAC",
            "rdfs:comment": "High Pressure pumps for reverse osmosis and filtration applications, driven by an asynchronous motor.",
            "skos:inScheme": "https://grundfos.com/concept/productFamily",
            "skos:prefLabel": "BMS hs AC"
        },
        {
            "@id": "https://grundfos.com/concept/productFamily/BMSHS",
            "@type": [
                "gfs:ProductFamily",
                "skos:Concept"
            ],
            "gfs:level": 2,
            "gfs:typecode": "BMSHS",
            "rdfs:comment": "High Pressure pumps for reverse osmosis and filtration applications, driven by a permanent magnet motor and VFD included.",
            "skos:inScheme": "https://grundfos.com/concept/productFamily",
            "skos:prefLabel": "BMS hs PM"
        },
        {
            "@id": "https://grundfos.com/concept/productFamily/BMSFAM",
            "@type": [
                "gfs:ProductFamily",
                "skos:Concept"
            ],
            "gfs:level": 1,
            "gfs:typecode": "BMSFAM",
            "rdfs:comment": "Booster modules",
            "skos:inScheme": "https://grundfos.com/concept/productFamily",
            "skos:narrower": [
                "https://grundfos.com/concept/productFamily/BMSHPMG",
                "https://grundfos.com/concept/productFamily/BMSHP",
                "https://grundfos.com/concept/productFamily/BMSHSAC",
                "https://grundfos.com/concept/productFamily/BMSHS"
            ],
            "skos:prefLabel": "BMS"
        },
        {
            "@id": "https://grundfos.com/concept/productFamily/CMBASIS",
            "@type": [
                "gfs:ProductFamily",
                "skos:Concept"
            ],
            "gfs:level": 2,
            "gfs:typecode": "CMBASIS",
            "rdfs:comment": "CM are reliable, quiet and compact horizontal end-suction pumps. The modular pump design makes it easy to make customised solutions. The CM pumps are available in cast iron and stainless steel",
            "skos:inScheme": "https://grundfos.com/concept/productFamily",
            "skos:prefLabel": "CM"
        },
        {
            "@id": "https://grundfos.com/concept/productFamily/CML00",
            "@type": [
                "gfs:ProductFamily",
                "skos:Concept"
            ],
            "gfs:level": 2,
            "gfs:typecode": "CML00",
            "rdfs:comment": "CM Leakage-free are reliable, quiet and compact horizontal end-suction pumps with canned-rotor motors. This means no shaft-seal is needed, so leakage is eliminated.",
            "skos:inScheme": "https://grundfos.com/concept/productFamily",
            "skos:prefLabel": "CM Leakage free"
        },
        {
            "@id": "https://grundfos.com/concept/productFamily/CMSP0",
            "@type": [
                "gfs:ProductFamily",
                "skos:Concept"
            ],
            "gfs:level": 2,
            "gfs:typecode": "CMSP0",
            "rdfs:comment": "CM self-priming pumps are reliable, quiet and compact horizontal end-suction pumps. The modular pump design makes customised solutions easy. The CM self-priming pumps are available in stainless steel",
            "skos:inScheme": "https://grundfos.com/concept/productFamily",
            "skos:prefLabel": "CM Self-priming"
        },
        {
            "@id": "https://grundfos.com/concept/productFamily/CMEBASIS",
            "@type": [
                "gfs:ProductFamily",
                "skos:Concept"
            ],
            "gfs:level": 2,
            "gfs:typecode": "CMEBASIS",
            "rdfs:comment": "CME are reliable, quiet and compact horizontal end-suction pumps. The modular pump design makes it easy to make customised solutions. The CME pumps are available in cast iron and stainless steel",
            "skos:inScheme": "https://grundfos.com/concept/productFamily",
            "skos:prefLabel": "CME"
        },
        {
            "@id": "https://grundfos.com/concept/productFamily/CMFAM",
            "@type": [
                "gfs:ProductFamily",
                "skos:Concept"
            ],
            "gfs:level": 1,
            "gfs:typecode": "CMFAM",
            "rdfs:comment": "CM/CME are reliable, quiet and compact horizontal end-suction pumps. The modular pump design makes it easy to make customised solutions. The CM/CME pumps are available in cast iron and stainless steel",
            "skos:inScheme": "https://grundfos.com/concept/productFamily",
            "skos:narrower": [
                "https://grundfos.com/concept/productFamily/CMBASIS",
                "https://grundfos.com/concept/productFamily/CML00",
                "https://grundfos.com/concept/productFamily/CMSP0",
                "https://grundfos.com/concept/productFamily/CMEBASIS"
            ],
            "skos:prefLabel": "CM, CME"
        },
        {
            "@id": "https://grundfos.com/concept/productFamily/CMB00",
            "@type": [
                "gfs:ProductFamily",
                "skos:Concept"
            ],
            "gfs:level": 2,
            "gfs:typecode": "CMB00",
            "rdfs:comment": "Compact booster set for water supply in domestic and light commercial applications",
            "skos:inScheme": "https://grundfos.com/concept/productFamily",
            "skos:prefLabel": "CMB PM"
        },
        {
            "@id": "https://grundfos.com/concept/productFamily/CMBPTPS",
            "@type": [
                "gfs:ProductFamily",
                "skos:Concept"
            ],
            "gfs:level": 2,
            "gfs:typecode": "CMBPTPS",
            "rdfs:comment": "Grundfos CM Booster PT and PS is a compact booster set with pressure switch for water supply in domestic light commercial applications.",
            "skos:inScheme": "https://grundfos.com/concept/productFamily",
            "skos:prefLabel": "CMB PT and CMB PS"
        },
        {
            "@id": "https://grundfos.com/concept/productFamily/CMBSP",
            "@type": [
                "gfs:ProductFamily",
                "skos:Concept"
            ],
            "gfs:level": 2,
            "gfs:typecode": "CMBSP",
            "rdfs:comment": "Compact booster solution with pressure manager for water supply in domestic and light commercial applications. It can create suction lift of up to 8 m. Wetted parts are in stainless steel (EN 1.4301)",
            "skos:inScheme": "https://grundfos.com/concept/productFamily",
            "skos:prefLabel": "CMB-SP PM"
        },
        {
            "@id": "https://grundfos.com/concept/productFamily/CMEB00",
            "@type": [
                "gfs:ProductFamily",
                "skos:Concept"
            ],
            "gfs:level": 2,
            "gfs:typecode": "CMEB00",
            "rdfs:comment": "Compact booster set for water supply in light commercial applications. Pump materials in contact with the liquid are in stainless steel (EN 1.4301)",
            "skos:inScheme": "https://grundfos.com/concept/productFamily",
            "skos:prefLabel": "CMBE"
        },
        {
            "@id": "https://grundfos.com/concept/productFamily/CMBETWIN",
            "@type": [
                "gfs:ProductFamily",
                "skos:Concept"
            ],
            "gfs:level": 2,
            "gfs:typecode": "CMBETWIN",
            "rdfs:comment": "The CMBE TWIN booster systems consist of two to four Grundfos CMBE booster connected in parallel, designed for the transfer and pressure boosting of clean water.",
            "skos:inScheme": "https://grundfos.com/concept/productFamily",
            "skos:prefLabel": "CMBE TWIN"
        },
        {
            "@id": "https://grundfos.com/concept/productFamily/CMBFAM",
            "@type": [
                "gfs:ProductFamily",
                "skos:Concept"
            ],
            "gfs:level": 1,
            "gfs:typecode": "CMBFAM",
            "rdfs:comment": "Compact booster set for water supply in domestic and light commercial applications",
            "skos:inScheme": "https://grundfos.com/concept/productFamily",
            "skos:narrower": [
                "https://grundfos.com/concept/productFamily/CMB00",
                "https://grundfos.com/concept/productFamily/CMBPTPS",
                "https://grundfos.com/concept/productFamily/CMBSP",
                "https://grundfos.com/concept/productFamily/CMEB00",
                "https://grundfos.com/concept/productFamily/CMBETWIN"
            ],
            "skos:prefLabel": "CMB, CMBE"
        },
        {
            "@id": "https://grundfos.com/concept/productFamily/COMB1",
            "@type": [
                "gfs:ProductFamily",
                "skos:Concept"
            ],
            "gfs:level": 1,
            "gfs:typecode": "COMB1",
            "rdfs:comment": "Domestic hot water pumps",
            "skos:inScheme": "https://grundfos.com/concept/productFamily",
            "skos:narrower": [],
            "skos:prefLabel": "COMFORT"
        },
        {
            "@id": "https://grundfos.com/concept/productFamily/CONLIF",
            "@type": [
                "gfs:ProductFamily",
                "skos:Concept"
            ],
            "gfs:level": 2,
            "gfs:typecode": "CONLIF",
            "rdfs:comment": "Condensate lifting station",
            "skos:inScheme": "https://grundfos.com/concept/productFamily",
            "skos:prefLabel": "Conlift"
        },
        {
            "@id": "https://grundfos.com/concept/productFamily/CONLIFT",
            "@type": [
                "gfs:ProductFamily",
                "skos:Concept"
            ],
            "gfs:level": 1,
            "gfs:typecode": "CONLIFT",
            "rdfs:comment": "Grundfos CONLIFT are condensate removal pump solutions suitable for the pumping of condensate that is collected below sewer level or which cannot flow to the buildings sewage system or drain by means of a natural downward slope.",
            "skos:inScheme": "https://grundfos.com/concept/productFamily",
            "skos:narrower": [
                "https://grundfos.com/concept/productFamily/CONLIF"
            ],
            "skos:prefLabel": "Conlift"
        },
        {
            "@id": "https://grundfos.com/concept/productFamily/ALPREAD",
            "@type": [
                "gfs:ProductFamily",
                "skos:Concept"
            ],
            "gfs:level": 2,
            "gfs:typecode": "ALPREAD",
            "rdfs:comment": "Mobile product for hydronic balancing of radiators in combination with an ALPHA3 and a smart phone via Bluetooth with Go Balance-app (iOS and Android devices).",
            "skos:inScheme": "https://grundfos.com/concept/productFamily",
            "skos:prefLabel": "ALPHA READER"
        },
        {
            "@id": "https://grundfos.com/concept/productFamily/CIMCIU",
            "@type": [
                "gfs:ProductFamily",
                "skos:Concept"
            ],
            "gfs:level": 2,
            "gfs:typecode": "CIMCIU",
            "rdfs:comment": "Communication Interfaces",
            "skos:inScheme": "https://grundfos.com/concept/productFamily",
            "skos:prefLabel": "CIM/CIU"
        },
        {
            "@id": "https://grundfos.com/concept/productFamily/CONTCUE",
            "@type": [
                "gfs:ProductFamily",
                "skos:Concept"
            ],
            "gfs:level": 2,
            "gfs:typecode": "CONTCUE",
            "rdfs:comment": "Accessories",
            "skos:inScheme": "https://grundfos.com/concept/productFamily",
            "skos:prefLabel": "Control CUE"
        },
        {
            "@id": "https://grundfos.com/concept/productFamily/DEDICONT",
            "@type": [
                "gfs:ProductFamily",
                "skos:Concept"
            ],
            "gfs:level": 2,
            "gfs:typecode": "DEDICONT",
            "rdfs:comment": "Grundfos Control DC is a control system designed for installation in municipal wastewater transportation installations, commercial buildings or network pumping stations with up to six wastewater pumps. Advanced control and data communication are also possible with the Grundfos Control DC.",
            "skos:inScheme": "https://grundfos.com/concept/productFamily",
            "skos:prefLabel": "Control DC"
        },
        {
            "@id": "https://grundfos.com/concept/productFamily/CONTDDD",
            "@type": [
                "gfs:ProductFamily",
                "skos:Concept"
            ],
            "gfs:level": 2,
            "gfs:typecode": "CONTDDD",
            "rdfs:comment": "Demand Driven Distribution, offers the next level in water distribution with critical point measurement and advanced flow adoption. Up to six pumps.",
            "skos:inScheme": "https://grundfos.com/concept/productFamily",
            "skos:prefLabel": "Control DDD"
        },
        {
            "@id": "https://grundfos.com/concept/productFamily/CONT204",
            "@type": [
                "gfs:ProductFamily",
                "skos:Concept"
            ],
            "gfs:level": 2,
            "gfs:typecode": "CONT204",
            "rdfs:comment": "Pump controler system designed for water utility marked. Complete protection of one pump.",
            "skos:inScheme": "https://grundfos.com/concept/productFamily",
            "skos:prefLabel": "Control MP 204"
        },
        {
            "@id": "https://grundfos.com/concept/productFamily/COMPC",
            "@type": [
                "gfs:ProductFamily",
                "skos:Concept"
            ],
            "gfs:level": 2,
            "gfs:typecode": "COMPC",
            "rdfs:comment": "Grundfos Multi Pump Controller for control and monitoring of up to six identical pumps. Control MPC offers perfect solutions to building services, water utilities and industry applications.",
            "skos:inScheme": "https://grundfos.com/concept/productFamily",
            "skos:prefLabel": "Control MPC"
        },
        {
            "@id": "https://grundfos.com/concept/productFamily/CU241",
            "@type": [
                "gfs:ProductFamily",
                "skos:Concept"
            ],
            "gfs:level": 2,
            "gfs:typecode": "CU241",
            "rdfs:comment": "CU 241 control unit are designed for level control, monitoring and protection of waste water pumping systems one pumps or two pumps in combination with IO 242 module and as option IO 241 module. CU 241 control unit is designed to fit into the front of a control panel.",
            "skos:inScheme": "https://grundfos.com/concept/productFamily",
            "skos:prefLabel": "CU 241"
        },
        {
            "@id": "https://grundfos.com/concept/productFamily/CU242",
            "@type": [
                "gfs:ProductFamily",
                "skos:Concept"
            ],
            "gfs:level": 2,
            "gfs:typecode": "CU242",
            "rdfs:comment": "CU 242 control unit are designed for level control, monitoring and protection of groundwater installation with one or two pumps in combination with IO 242 module and as option IO 241 module. CU 242 control unit is designed to fit into the front of a control panel.",
            "skos:inScheme": "https://grundfos.com/concept/productFamily",
            "skos:prefLabel": "CU 242"
        },
        {
            "@id": "https://grundfos.com/concept/productFamily/CU362",
            "@type": [
                "gfs:ProductFamily",
                "skos:Concept"
            ],
            "gfs:level": 2,
            "gfs:typecode": "CU362",
            "rdfs:comment": "Accessories",
            "skos:inScheme": "https://grundfos.com/concept/productFamily",
            "skos:prefLabel": "CU 362"
        },
        {
            "@id": "https://grundfos.com/concept/productFamily/DCACC",
            "@type": [
                "gfs:ProductFamily",
                "skos:Concept"
            ],
            "gfs:level": 2,
            "gfs:typecode": "DCACC",
            "rdfs:comment": "Accessories",
            "skos:inScheme": "https://grundfos.com/concept/productFamily",
            "skos:prefLabel": "Dedicated Controls accessories"
        },
        {
            "@id": "https://grundfos.com/concept/productFamily/IO113",
            "@type": [
                "gfs:ProductFamily",
                "skos:Concept"
            ],
            "gfs:level": 2,
            "gfs:typecode": "IO113",
            "rdfs:comment": "Input Module IO 113 designed to interface with pump sensors. One without communication as standard variant and one with communication for interface to Sensor Module SM 113",
            "skos:inScheme": "https://grundfos.com/concept/productFamily",
            "skos:prefLabel": "IO 113"
        },
        {
            "@id": "https://grundfos.com/concept/productFamily/IO241",
            "@type": [
                "gfs:ProductFamily",
                "skos:Concept"
            ],
            "gfs:level": 2,
            "gfs:typecode": "IO241",
            "rdfs:comment": "The IO 241 module is an optional module for gaining extra input and output signals. It\u00c3\u00a2\u00e2\u201a\u00ac\u00e2\u201e\u00a2s designed to fit into a DIN rail, and for use in control panels. It can be connected to the IO 242 pump module and control unit CU 241.",
            "skos:inScheme": "https://grundfos.com/concept/productFamily",
            "skos:prefLabel": "IO 241"
        },
        {
            "@id": "https://grundfos.com/concept/productFamily/IO242",
            "@type": [
                "gfs:ProductFamily",
                "skos:Concept"
            ],
            "gfs:level": 2,
            "gfs:typecode": "IO242",
            "rdfs:comment": "IO 242 provides analog and digital input signals for CU 241, and designed to fit into a DIN rail, and for use in control panels. The IO 242 pump module is used together with Grundfos controllers and modules.",
            "skos:inScheme": "https://grundfos.com/concept/productFamily",
            "skos:prefLabel": "IO 242"
        },
        {
            "@id": "https://grundfos.com/concept/productFamily/IO351B",
            "@type": [
                "gfs:ProductFamily",
                "skos:Concept"
            ],
            "gfs:level": 2,
            "gfs:typecode": "IO351B",
            "rdfs:comment": "Accessories",
            "skos:inScheme": "https://grundfos.com/concept/productFamily",
            "skos:prefLabel": "IO 351B"
        },
        {
            "@id": "https://grundfos.com/concept/productFamily/LC231",
            "@type": [
                "gfs:ProductFamily",
                "skos:Concept"
            ],
            "gfs:level": 2,
            "gfs:typecode": "LC231",
            "rdfs:comment": "LC 231 pump controllers are designed for level control, monitoring and protection of pumping systems, one or two pumps starting DOL up to 12 Amp. The LC 231 has a built-in motor protection and current measurement.",
            "skos:inScheme": "https://grundfos.com/concept/productFamily",
            "skos:prefLabel": "LC 231"
        },
        {
            "@id": "https://grundfos.com/concept/productFamily/LC241",
            "@type": [
                "gfs:ProductFamily",
                "skos:Concept"
            ],
            "gfs:level": 2,
            "gfs:typecode": "LC241",
            "rdfs:comment": "LC 241 level controllers offer a comprehensive range of features for waste water pumping systems, monitoring and control of one or two pumps, up to 72 Amp. The LC 241 is a metal or plastic cabinet solution offering modularity and customization according to your needs.",
            "skos:inScheme": "https://grundfos.com/concept/productFamily",
            "skos:prefLabel": "LC 241"
        },
        {
            "@id": "https://grundfos.com/concept/productFamily/LC242",
            "@type": [
                "gfs:ProductFamily",
                "skos:Concept"
            ],
            "gfs:level": 2,
            "gfs:typecode": "LC242",
            "rdfs:comment": "LC 242 level controllers offer a comprehensive range of features for groundwater installation, monitoring and control of one or two pumps, up to 72 Amp. The LC 242 is a metal or plastic cabinet solution offering modularity and customization according to your needs.",
            "skos:inScheme": "https://grundfos.com/concept/productFamily",
            "skos:prefLabel": "LC 242"
        },
        {
            "@id": "https://grundfos.com/concept/productFamily/MP0204",
            "@type": [
                "gfs:ProductFamily",
                "skos:Concept"
            ],
            "gfs:level": 2,
            "gfs:typecode": "MP0204",
            "rdfs:comment": "MP 204 is a motor protection that protects the motor primarily by measuring the motor current by means of a true RMS measurement. The MP 204 disconnects the contactor if, for example, the current exceeds the preset value. It can be used as a stand-alone or as incorporated in a for example Control DC.",
            "skos:inScheme": "https://grundfos.com/concept/productFamily",
            "skos:prefLabel": "MP 204"
        },
        {
            "@id": "https://grundfos.com/concept/productFamily/MP0204AC",
            "@type": [
                "gfs:ProductFamily",
                "skos:Concept"
            ],
            "gfs:level": 2,
            "gfs:typecode": "MP0204AC",
            "rdfs:comment": "Accessories",
            "skos:inScheme": "https://grundfos.com/concept/productFamily",
            "skos:prefLabel": "MP 204 accessories"
        },
        {
            "@id": "https://grundfos.com/concept/productFamily/SM113",
            "@type": [
                "gfs:ProductFamily",
                "skos:Concept"
            ],
            "gfs:level": 2,
            "gfs:typecode": "SM113",
            "rdfs:comment": "Sensor Module SM113 designed to interface with pump sensors and communicate via powerline to IO 113 with communication.",
            "skos:inScheme": "https://grundfos.com/concept/productFamily",
            "skos:prefLabel": "SM 113"
        },
        {
            "@id": "https://grundfos.com/concept/productFamily/CONTROL",
            "@type": [
                "gfs:ProductFamily",
                "skos:Concept"
            ],
            "gfs:level": 1,
            "gfs:typecode": "CONTROL",
            "rdfs:comment": "Control units for pumps",
            "skos:inScheme": "https://grundfos.com/concept/productFamily",
            "skos:narrower": [
                "https://grundfos.com/concept/productFamily/ALPREAD",
                "https://grundfos.com/concept/productFamily/CIMCIU",
                "https://grundfos.com/concept/productFamily/CONTCUE",
                "https://grundfos.com/concept/productFamily/DEDICONT",
                "https://grundfos.com/concept/productFamily/CONTDDD",
                "https://grundfos.com/concept/productFamily/CONT204",
                "https://grundfos.com/concept/productFamily/COMPC",
                "https://grundfos.com/concept/productFamily/CU241",
                "https://grundfos.com/concept/productFamily/CU242",
                "https://grundfos.com/concept/productFamily/CU362",
                "https://grundfos.com/concept/productFamily/DCACC",
                "https://grundfos.com/concept/productFamily/IO113",
                "https://grundfos.com/concept/productFamily/IO241",
                "https://grundfos.com/concept/productFamily/IO242",
                "https://grundfos.com/concept/productFamily/IO351B",
                "https://grundfos.com/concept/productFamily/LC231",
                "https://grundfos.com/concept/productFamily/LC241",
                "https://grundfos.com/concept/productFamily/LC242",
                "https://grundfos.com/concept/productFamily/MP0204",
                "https://grundfos.com/concept/productFamily/MP0204AC",
                "https://grundfos.com/concept/productFamily/SM113"
            ],
            "skos:prefLabel": "Controls and Monitoring"
        },
        {
            "@id": "https://grundfos.com/concept/productFamily/CRFAM",
            "@type": [
                "gfs:ProductFamily",
                "skos:Concept"
            ],
            "gfs:level": 2,
            "gfs:typecode": "CRFAM",
            "rdfs:comment": "Vertical, multistage centrifugal pump with suction and discharge ports on the same level. The pump head and base are in cast iron - all other wetted parts are in stainless steel (EN 1.4301)",
            "skos:inScheme": "https://grundfos.com/concept/productFamily",
            "skos:prefLabel": "CR"
        },
        {
            "@id": "https://grundfos.com/concept/productFamily/CREFAM",
            "@type": [
                "gfs:ProductFamily",
                "skos:Concept"
            ],
            "gfs:level": 2,
            "gfs:typecode": "CREFAM",
            "rdfs:comment": "Vertical, multistage centrifugal pump with integrated frequency converter. The pump head and base are in cast iron - all other wetted parts are in stainless steel (EN 1.4301)",
            "skos:inScheme": "https://grundfos.com/concept/productFamily",
            "skos:prefLabel": "CRE"
        },
        {
            "@id": "https://grundfos.com/concept/productFamily/CRIFAM",
            "@type": [
                "gfs:ProductFamily",
                "skos:Concept"
            ],
            "gfs:level": 2,
            "gfs:typecode": "CRIFAM",
            "rdfs:comment": "Vertical, multistage centrifugal pump with suction and discharge ports on same the level. Pump materials in contact with the liquid are in stainless steel (EN 1.4301)",
            "skos:inScheme": "https://grundfos.com/concept/productFamily",
            "skos:prefLabel": "CRI"
        },
        {
            "@id": "https://grundfos.com/concept/productFamily/CRIEFAM",
            "@type": [
                "gfs:ProductFamily",
                "skos:Concept"
            ],
            "gfs:level": 2,
            "gfs:typecode": "CRIEFAM",
            "rdfs:comment": "Vertical, multistage centrifugal pump with integrated frequency converter. Pump materials in contact with the liquid are in stainless steel (EN 1.4301)",
            "skos:inScheme": "https://grundfos.com/concept/productFamily",
            "skos:prefLabel": "CRIE"
        },
        {
            "@id": "https://grundfos.com/concept/productFamily/CRNFAM",
            "@type": [
                "gfs:ProductFamily",
                "skos:Concept"
            ],
            "gfs:level": 2,
            "gfs:typecode": "CRNFAM",
            "rdfs:comment": "Vertical, multistage centrifugal pump with suction and discharge ports on the same level. Pump materials in contact with the liquid are in high-grade stainless steel (EN 1.4401)",
            "skos:inScheme": "https://grundfos.com/concept/productFamily",
            "skos:prefLabel": "CRN"
        },
        {
            "@id": "https://grundfos.com/concept/productFamily/CRNEFAM",
            "@type": [
                "gfs:ProductFamily",
                "skos:Concept"
            ],
            "gfs:level": 2,
            "gfs:typecode": "CRNEFAM",
            "rdfs:comment": "Vertical, multistage centrifugal pump with integrated frequency converter. Pump materials in contact with the liquid are in high-grade stainless steel (EN 1.4401)",
            "skos:inScheme": "https://grundfos.com/concept/productFamily",
            "skos:prefLabel": "CRNE"
        },
        {
            "@id": "https://grundfos.com/concept/productFamily/CRNEHSSF",
            "@type": [
                "gfs:ProductFamily",
                "skos:Concept"
            ],
            "gfs:level": 2,
            "gfs:typecode": "CRNEHSSF",
            "rdfs:comment": "Vertical, multistage centrifugal pump with suction and discharge ports on the same level. Pump materials in contact with the liquid are in high-grade stainless steel (EN 1.4401)",
            "skos:inScheme": "https://grundfos.com/concept/productFamily",
            "skos:prefLabel": "CRNE-HS, CRN-SF"
        },
        {
            "@id": "https://grundfos.com/concept/productFamily/CRTFAM",
            "@type": [
                "gfs:ProductFamily",
                "skos:Concept"
            ],
            "gfs:level": 2,
            "gfs:typecode": "CRTFAM",
            "rdfs:comment": "Vertical, multistage centrifugal pump with suction and discharge ports on same the level. Materials in contact with the liquid are in Titanium. Titanium has an exceptional resistance to a wide range of acids, alkalis, seawater and industrial chemicals",
            "skos:inScheme": "https://grundfos.com/concept/productFamily",
            "skos:prefLabel": "CRT"
        },
        {
            "@id": "https://grundfos.com/concept/productFamily/CRTEFAM",
            "@type": [
                "gfs:ProductFamily",
                "skos:Concept"
            ],
            "gfs:level": 2,
            "gfs:typecode": "CRTEFAM",
            "rdfs:comment": "Vertical, multistage centrifugal pump with integrated frequency converter. Materials in contact with the liquid are in Titanium has an exceptional resistance to a wide range of acids, alkalis, seawater and industrial chemicals",
            "skos:inScheme": "https://grundfos.com/concept/productFamily",
            "skos:prefLabel": "CRTE"
        },
        {
            "@id": "https://grundfos.com/concept/productFamily/CRRANGE",
            "@type": [
                "gfs:ProductFamily",
                "skos:Concept"
            ],
            "gfs:level": 1,
            "gfs:typecode": "CRRANGE",
            "rdfs:comment": "Vertical, multistage centrifugal pump with suction and discharge ports on the same level.",
            "skos:inScheme": "https://grundfos.com/concept/productFamily",
            "skos:narrower": [
                "https://grundfos.com/concept/productFamily/CRFAM",
                "https://grundfos.com/concept/productFamily/CREFAM",
                "https://grundfos.com/concept/productFamily/CRIFAM",
                "https://grundfos.com/concept/productFamily/CRIEFAM",
                "https://grundfos.com/concept/productFamily/CRNFAM",
                "https://grundfos.com/concept/productFamily/CRNEFAM",
                "https://grundfos.com/concept/productFamily/CRNEHSSF",
                "https://grundfos.com/concept/productFamily/CRTFAM",
                "https://grundfos.com/concept/productFamily/CRTEFAM"
            ],
            "skos:prefLabel": "CR, CRE, CRI, CRIE, CRN, CRNE, CRT, CRTE"
        },
        {
            "@id": "https://grundfos.com/concept/productFamily/CRFLEX",
            "@type": [
                "gfs:ProductFamily",
                "skos:Concept"
            ],
            "gfs:level": 1,
            "gfs:typecode": "CRFLEX",
            "rdfs:comment": "Vertical multistage pumps with Renewable MGFlex motor for solar, wind and AC powersource. Runs on both AC and DC voltage",
            "skos:inScheme": "https://grundfos.com/concept/productFamily",
            "skos:narrower": [],
            "skos:prefLabel": "CRFlex"
        },
        {
            "@id": "https://grundfos.com/concept/productFamily/DDDFAM",
            "@type": [
                "gfs:ProductFamily",
                "skos:Concept"
            ],
            "gfs:level": 1,
            "gfs:typecode": "DDDFAM",
            "rdfs:comment": "Many distribution networks struggle with excessive water waste, high operational costs and high energy consumption. Demand Driven Distribution is a unique pressure management system, to adjust the pressure in the system. As a water leakage solution, the results are minimised water losses, reduced energy consumption and minimised operational costs \u00c3\u00a2\u00e2\u201a\u00ac\u00e2\u20ac\u0153 without reducing comfort at the end user.",
            "skos:inScheme": "https://grundfos.com/concept/productFamily",
            "skos:narrower": [],
            "skos:prefLabel": "Demand driven distribution"
        },
        {
            "@id": "https://grundfos.com/concept/productFamily/GRUNDFGO",
            "@type": [
                "gfs:ProductFamily",
                "skos:Concept"
            ],
            "gfs:level": 2,
            "gfs:typecode": "GRUNDFGO",
            "rdfs:comment": "Our intuitive tool box for mobile pump control that provides you with instant pump data, designed to save you time and effort.",
            "skos:inScheme": "https://grundfos.com/concept/productFamily",
            "skos:prefLabel": "Grundfos Go"
        },
        {
            "@id": "https://grundfos.com/concept/productFamily/GRUNDFIC",
            "@type": [
                "gfs:ProductFamily",
                "skos:Concept"
            ],
            "gfs:level": 2,
            "gfs:typecode": "GRUNDFIC",
            "rdfs:comment": "This is our platform for developing digital service solutions where specialised applications software can optimise your systems.",
            "skos:inScheme": "https://grundfos.com/concept/productFamily",
            "skos:prefLabel": "Grundfos iSolution cloud"
        },
        {
            "@id": "https://grundfos.com/concept/productFamily/GIM000",
            "@type": [
                "gfs:ProductFamily",
                "skos:Concept"
            ],
            "gfs:level": 2,
            "gfs:typecode": "GIM000",
            "rdfs:comment": "A single smart sensor improving your peace of mind by constantly monitoring pump health and process errors that can damage pumps.",
            "skos:inScheme": "https://grundfos.com/concept/productFamily",
            "skos:prefLabel": "Grundfos iSolution monitor"
        },
        {
            "@id": "https://grundfos.com/concept/productFamily/GRM000",
            "@type": [
                "gfs:ProductFamily",
                "skos:Concept"
            ],
            "gfs:level": 2,
            "gfs:typecode": "GRM000",
            "rdfs:comment": "Internet-based system that gives you an efficient and cost-effective alternative to more costly systems.",
            "skos:inScheme": "https://grundfos.com/concept/productFamily",
            "skos:prefLabel": "Grundfos Remote Management"
        },
        {
            "@id": "https://grundfos.com/concept/productFamily/WWNETCON",
            "@type": [
                "gfs:ProductFamily",
                "skos:Concept"
            ],
            "gfs:level": 2,
            "gfs:typecode": "WWNETCON",
            "rdfs:comment": "Cloud-based solution to optimise operation and ease expansion or repair of your wastewater network.",
            "skos:inScheme": "https://grundfos.com/concept/productFamily",
            "skos:prefLabel": "Waste water network connect"
        },
        {
            "@id": "https://grundfos.com/concept/productFamily/DIGSERVI",
            "@type": [
                "gfs:ProductFamily",
                "skos:Concept"
            ],
            "gfs:level": 1,
            "gfs:typecode": "DIGSERVI",
            "rdfs:comment": "Connected pumps open up a world of opportunities for true data-based optimisation taking pump performance to a new level.",
            "skos:inScheme": "https://grundfos.com/concept/productFamily",
            "skos:narrower": [
                "https://grundfos.com/concept/productFamily/GRUNDFGO",
                "https://grundfos.com/concept/productFamily/GRUNDFIC",
                "https://grundfos.com/concept/productFamily/GIM000",
                "https://grundfos.com/concept/productFamily/GRM000",
                "https://grundfos.com/concept/productFamily/WWNETCON"
            ],
            "skos:prefLabel": "Digital services"
        },
        {
            "@id": "https://grundfos.com/concept/productFamily/OCD162",
            "@type": [
                "gfs:ProductFamily",
                "skos:Concept"
            ],
            "gfs:level": 2,
            "gfs:typecode": "OCD162",
            "rdfs:comment": "OCD, OCC and ISIA chlorine dioxide preparing and dosing system.",
            "skos:inScheme": "https://grundfos.com/concept/productFamily",
            "skos:prefLabel": "Oxiperm"
        },
        {
            "@id": "https://grundfos.com/concept/productFamily/SES",
            "@type": [
                "gfs:ProductFamily",
                "skos:Concept"
            ],
            "gfs:level": 2,
            "gfs:typecode": "SES",
            "rdfs:comment": "SES electro-chlorinator produces hypochlorite solution from a solution of common salt using electricty",
            "skos:inScheme": "https://grundfos.com/concept/productFamily",
            "skos:prefLabel": "Selcoperm"
        },
        {
            "@id": "https://grundfos.com/concept/productFamily/VGFAM",
            "@type": [
                "gfs:ProductFamily",
                "skos:Concept"
            ],
            "gfs:level": 2,
            "gfs:typecode": "VGFAM",
            "rdfs:comment": "VGA, VGB and VGS chlorine gas dosing systems.",
            "skos:inScheme": "https://grundfos.com/concept/productFamily",
            "skos:prefLabel": "Vaccuperm"
        },
        {
            "@id": "https://grundfos.com/concept/productFamily/DISINFEC",
            "@type": [
                "gfs:ProductFamily",
                "skos:Concept"
            ],
            "gfs:level": 2,
            "gfs:typecode": "DISINFEC",
            "rdfs:comment": "Accessories",
            "skos:inScheme": "https://grundfos.com/concept/productFamily",
            "skos:prefLabel": "Vaccuperm Accessories"
        },
        {
            "@id": "https://grundfos.com/concept/productFamily/DISINFAM",
            "@type": [
                "gfs:ProductFamily",
                "skos:Concept"
            ],
            "gfs:level": 1,
            "gfs:typecode": "DISINFAM",
            "rdfs:comment": "Chlorine, Chlorine Dioxide, Electrochlorination",
            "skos:inScheme": "https://grundfos.com/concept/productFamily",
            "skos:narrower": [
                "https://grundfos.com/concept/productFamily/OCD162",
                "https://grundfos.com/concept/productFamily/SES",
                "https://grundfos.com/concept/productFamily/VGFAM",
                "https://grundfos.com/concept/productFamily/DISINFEC"
            ],
            "skos:prefLabel": "Disinfection Systems"
        },
        {
            "@id": "https://grundfos.com/concept/productFamily/DISTPUMP",
            "@type": [
                "gfs:ProductFamily",
                "skos:Concept"
            ],
            "gfs:level": 1,
            "gfs:typecode": "DISTPUMP",
            "rdfs:comment": "Grundfos Distributed Pumping makes it easy to balance chilled water systems and enhancing comfort in buildings. The solution replaces traditional balance and control valves with intelligent pumps. This improves Delta T and reduces pump energy in commercial buildings.",
            "skos:inScheme": "https://grundfos.com/concept/productFamily",
            "skos:narrower": [],
            "skos:prefLabel": "Distributed pumping"
        },
        {
            "@id": "https://grundfos.com/concept/productFamily/DDAFAM",
            "@type": [
                "gfs:ProductFamily",
                "skos:Concept"
            ],
            "gfs:level": 2,
            "gfs:typecode": "DDAFAM",
            "rdfs:comment": "SMART Digital diaphragm dosing pump with internal brushless motor drive. High-end solution for complex and demanding applications (Digital Dosing Advanced).",
            "skos:inScheme": "https://grundfos.com/concept/productFamily",
            "skos:prefLabel": "DDA"
        },
        {
            "@id": "https://grundfos.com/concept/productFamily/DDCFAM",
            "@type": [
                "gfs:ProductFamily",
                "skos:Concept"
            ],
            "gfs:level": 2,
            "gfs:typecode": "DDCFAM",
            "rdfs:comment": "SMART Digital diaphragm dosing pump with internal stepper motor drive. User-friendly at optimum price-performance-ratio (Digital Dosing Convenience).",
            "skos:inScheme": "https://grundfos.com/concept/productFamily",
            "skos:prefLabel": "DDC"
        },
        {
            "@id": "https://grundfos.com/concept/productFamily/DDEFAM",
            "@type": [
                "gfs:ProductFamily",
                "skos:Concept"
            ],
            "gfs:level": 2,
            "gfs:typecode": "DDEFAM",
            "rdfs:comment": "SMART Digital diaphragm dosing pump with internal stepper motor drive. Economic Digital Dosing even for basic dosing applications (Digital Dosing Essential).",
            "skos:inScheme": "https://grundfos.com/concept/productFamily",
            "skos:prefLabel": "DDE"
        },
        {
            "@id": "https://grundfos.com/concept/productFamily/DDIFAM",
            "@type": [
                "gfs:ProductFamily",
                "skos:Concept"
            ],
            "gfs:level": 2,
            "gfs:typecode": "DDIFAM",
            "rdfs:comment": "Digital diaphragm dosing pumps with internal step motor drive",
            "skos:inScheme": "https://grundfos.com/concept/productFamily",
            "skos:prefLabel": "DDI"
        },
        {
            "@id": "https://grundfos.com/concept/productFamily/DME01",
            "@type": [
                "gfs:ProductFamily",
                "skos:Concept"
            ],
            "gfs:level": 2,
            "gfs:typecode": "DME01",
            "rdfs:comment": "Digital diaphragm dosing pumps with internal step motor drive",
            "skos:inScheme": "https://grundfos.com/concept/productFamily",
            "skos:prefLabel": "DME"
        },
        {
            "@id": "https://grundfos.com/concept/productFamily/DMHFAM",
            "@type": [
                "gfs:ProductFamily",
                "skos:Concept"
            ],
            "gfs:level": 2,
            "gfs:typecode": "DMHFAM",
            "rdfs:comment": "Hydraulically driven diaphragm dosing pumps with external motor",
            "skos:inScheme": "https://grundfos.com/concept/productFamily",
            "skos:prefLabel": "DMH"
        },
        {
            "@id": "https://grundfos.com/concept/productFamily/DMXFAM",
            "@type": [
                "gfs:ProductFamily",
                "skos:Concept"
            ],
            "gfs:level": 2,
            "gfs:typecode": "DMXFAM",
            "rdfs:comment": "Diaphragm dosing pumps with external motor",
            "skos:inScheme": "https://grundfos.com/concept/productFamily",
            "skos:prefLabel": "DMX"
        },
        {
            "@id": "https://grundfos.com/concept/productFamily/DOSFAM",
            "@type": [
                "gfs:ProductFamily",
                "skos:Concept"
            ],
            "gfs:level": 1,
            "gfs:typecode": "DOSFAM",
            "rdfs:comment": "Mechanical and digital dosing pumps",
            "skos:inScheme": "https://grundfos.com/concept/productFamily",
            "skos:narrower": [
                "https://grundfos.com/concept/productFamily/DDAFAM",
                "https://grundfos.com/concept/productFamily/DDCFAM",
                "https://grundfos.com/concept/productFamily/DDEFAM",
                "https://grundfos.com/concept/productFamily/DDIFAM",
                "https://grundfos.com/concept/productFamily/DME01",
                "https://grundfos.com/concept/productFamily/DMHFAM",
                "https://grundfos.com/concept/productFamily/DMXFAM"
            ],
            "skos:prefLabel": "Dosing pumps"
        },
        {
            "@id": "https://grundfos.com/concept/productFamily/DPFAM",
            "@type": [
                "gfs:ProductFamily",
                "skos:Concept"
            ],
            "gfs:level": 1,
            "gfs:typecode": "DPFAM",
            "rdfs:comment": "Submersible Grundfos Drainage Pumps (DP) cover a motor range of 0.9-2.6 kW. The pumps are fitted with a semi-open multi-vane impeller capable of handling solids up to 10 mm in size.",
            "skos:inScheme": "https://grundfos.com/concept/productFamily",
            "skos:narrower": [],
            "skos:prefLabel": "DP"
        },
        {
            "@id": "https://grundfos.com/concept/productFamily/DPK000",
            "@type": [
                "gfs:ProductFamily",
                "skos:Concept"
            ],
            "gfs:level": 1,
            "gfs:typecode": "DPK000",
            "rdfs:comment": "Grundfos DPK drainage pumps are designed with an enclosed, semi-open or SuperVortex, free-flow impeller for use in many building and industrial applications. Range is 0.75-22 kW.",
            "skos:inScheme": "https://grundfos.com/concept/productFamily",
            "skos:narrower": [],
            "skos:prefLabel": "DPK"
        },
        {
            "@id": "https://grundfos.com/concept/productFamily/DWK000",
            "@type": [
                "gfs:ProductFamily",
                "skos:Concept"
            ],
            "gfs:level": 1,
            "gfs:typecode": "DWK000",
            "rdfs:comment": "Grundfos DWK dewatering pumps are designed with an enclosed, semi-open or SuperVortex, free-flow impeller for use in a wide range of building and industrial applications. Range is 0.75-90 kW.",
            "skos:inScheme": "https://grundfos.com/concept/productFamily",
            "skos:narrower": [],
            "skos:prefLabel": "DWK"
        },
        {
            "@id": "https://grundfos.com/concept/productFamily/EFFAM",
            "@type": [
                "gfs:ProductFamily",
                "skos:Concept"
            ],
            "gfs:level": 1,
            "gfs:typecode": "EFFAM",
            "rdfs:comment": "Grundfos EF pumps have a single-vane, semi-open impeller for 30 mm free passage, designed for pumping effluent and other liquids such as drainage and surface water with fibres and small impurities.",
            "skos:inScheme": "https://grundfos.com/concept/productFamily",
            "skos:narrower": [],
            "skos:prefLabel": "EF"
        },
        {
            "@id": "https://grundfos.com/concept/productFamily/FIRECRF",
            "@type": [
                "gfs:ProductFamily",
                "skos:Concept"
            ],
            "gfs:level": 1,
            "gfs:typecode": "FIRECRF",
            "rdfs:comment": "Grundfos fire systems",
            "skos:inScheme": "https://grundfos.com/concept/productFamily",
            "skos:narrower": [],
            "skos:prefLabel": "Fire, CRF"
        },
        {
            "@id": "https://grundfos.com/concept/productFamily/FIREDBI",
            "@type": [
                "gfs:ProductFamily",
                "skos:Concept"
            ],
            "gfs:level": 1,
            "gfs:typecode": "FIREDBI",
            "rdfs:comment": "Grundfos fire systems",
            "skos:inScheme": "https://grundfos.com/concept/productFamily",
            "skos:narrower": [],
            "skos:prefLabel": "Fire, DBI"
        },
        {
            "@id": "https://grundfos.com/concept/productFamily/FIREEN",
            "@type": [
                "gfs:ProductFamily",
                "skos:Concept"
            ],
            "gfs:level": 1,
            "gfs:typecode": "FIREEN",
            "rdfs:comment": "Grundfos fire systems",
            "skos:inScheme": "https://grundfos.com/concept/productFamily",
            "skos:narrower": [],
            "skos:prefLabel": "Fire, EN"
        },
        {
            "@id": "https://grundfos.com/concept/productFamily/FIREFMUL",
            "@type": [
                "gfs:ProductFamily",
                "skos:Concept"
            ],
            "gfs:level": 1,
            "gfs:typecode": "FIREFMUL",
            "rdfs:comment": "Grundfos fire systems",
            "skos:inScheme": "https://grundfos.com/concept/productFamily",
            "skos:narrower": [],
            "skos:prefLabel": "Fire, FM/UL"
        },
        {
            "@id": "https://grundfos.com/concept/productFamily/FIREPSB",
            "@type": [
                "gfs:ProductFamily",
                "skos:Concept"
            ],
            "gfs:level": 1,
            "gfs:typecode": "FIREPSB",
            "rdfs:comment": "Grundfos fire systems",
            "skos:inScheme": "https://grundfos.com/concept/productFamily",
            "skos:narrower": [],
            "skos:prefLabel": "Fire, PSB"
        },
        {
            "@id": "https://grundfos.com/concept/productFamily/FIREUNI",
            "@type": [
                "gfs:ProductFamily",
                "skos:Concept"
            ],
            "gfs:level": 1,
            "gfs:typecode": "FIREUNI",
            "rdfs:comment": "Grundfos fire systems",
            "skos:inScheme": "https://grundfos.com/concept/productFamily",
            "skos:narrower": [],
            "skos:prefLabel": "Fire, UNI"
        },
        {
            "@id": "https://grundfos.com/concept/productFamily/FIREVDS",
            "@type": [
                "gfs:ProductFamily",
                "skos:Concept"
            ],
            "gfs:level": 1,
            "gfs:typecode": "FIREVDS",
            "rdfs:comment": "Grundfos fire systems",
            "skos:inScheme": "https://grundfos.com/concept/productFamily",
            "skos:narrower": [],
            "skos:prefLabel": "Fire, VdS"
        },
        {
            "@id": "https://grundfos.com/concept/productFamily/FIREVTF",
            "@type": [
                "gfs:ProductFamily",
                "skos:Concept"
            ],
            "gfs:level": 1,
            "gfs:typecode": "FIREVTF",
            "rdfs:comment": "Grundfos fire systems",
            "skos:inScheme": "https://grundfos.com/concept/productFamily",
            "skos:narrower": [],
            "skos:prefLabel": "Fire, VTF"
        },
        {
            "@id": "https://grundfos.com/concept/productFamily/HSP000",
            "@type": [
                "gfs:ProductFamily",
                "skos:Concept"
            ],
            "gfs:level": 2,
            "gfs:typecode": "HSP000",
            "rdfs:comment": "Horizontal split case pumps",
            "skos:inScheme": "https://grundfos.com/concept/productFamily",
            "skos:prefLabel": "HS version 5"
        },
        {
            "@id": "https://grundfos.com/concept/productFamily/HSPFAM",
            "@type": [
                "gfs:ProductFamily",
                "skos:Concept"
            ],
            "gfs:level": 1,
            "gfs:typecode": "HSPFAM",
            "rdfs:comment": "Horizontal split case pumps",
            "skos:inScheme": "https://grundfos.com/concept/productFamily",
            "skos:narrower": [
                "https://grundfos.com/concept/productFamily/HSP000"
            ],
            "skos:prefLabel": "HS"
        },
        {
            "@id": "https://grundfos.com/concept/productFamily/HY100",
            "@type": [
                "gfs:ProductFamily",
                "skos:Concept"
            ],
            "gfs:level": 1,
            "gfs:typecode": "HY100",
            "rdfs:comment": "Turnkey booster systems",
            "skos:inScheme": "https://grundfos.com/concept/productFamily",
            "skos:narrower": [],
            "skos:prefLabel": "Hydro 1000"
        },
        {
            "@id": "https://grundfos.com/concept/productFamily/HYMPCE",
            "@type": [
                "gfs:ProductFamily",
                "skos:Concept"
            ],
            "gfs:level": 2,
            "gfs:typecode": "HYMPCE",
            "rdfs:comment": "Booster systems with frequency-controlled pumps",
            "skos:inScheme": "https://grundfos.com/concept/productFamily",
            "skos:prefLabel": "Hydro MPC-E"
        },
        {
            "@id": "https://grundfos.com/concept/productFamily/HYMPCF",
            "@type": [
                "gfs:ProductFamily",
                "skos:Concept"
            ],
            "gfs:level": 2,
            "gfs:typecode": "HYMPCF",
            "rdfs:comment": "Booster systems with frequency converter control",
            "skos:inScheme": "https://grundfos.com/concept/productFamily",
            "skos:prefLabel": "Hydro MPC-F"
        },
        {
            "@id": "https://grundfos.com/concept/productFamily/HYMPCS",
            "@type": [
                "gfs:ProductFamily",
                "skos:Concept"
            ],
            "gfs:level": 2,
            "gfs:typecode": "HYMPCS",
            "rdfs:comment": "Booster systems with ON/OFF control",
            "skos:inScheme": "https://grundfos.com/concept/productFamily",
            "skos:prefLabel": "Hydro MPC-S"
        },
        {
            "@id": "https://grundfos.com/concept/productFamily/HYMPC",
            "@type": [
                "gfs:ProductFamily",
                "skos:Concept"
            ],
            "gfs:level": 1,
            "gfs:typecode": "HYMPC",
            "rdfs:comment": "Advanced and energy efficient pressure boosting system for boosting of clean water.  Available with 2-6 parallel connected pumps, Integrated advanced controller and all necessary fittings",
            "skos:inScheme": "https://grundfos.com/concept/productFamily",
            "skos:narrower": [
                "https://grundfos.com/concept/productFamily/HYMPCE",
                "https://grundfos.com/concept/productFamily/HYMPCF",
                "https://grundfos.com/concept/productFamily/HYMPCS"
            ],
            "skos:prefLabel": "Hydro MPC"
        },
        {
            "@id": "https://grundfos.com/concept/productFamily/HYMULE",
            "@type": [
                "gfs:ProductFamily",
                "skos:Concept"
            ],
            "gfs:level": 1,
            "gfs:typecode": "HYMULE",
            "rdfs:comment": "Energy efficient pressure boosting system for boosting of clean water.  Available with 2-4 parallel connected   frequency controlled pumps, Integrated advanced controller and all necessary fittings",
            "skos:inScheme": "https://grundfos.com/concept/productFamily",
            "skos:narrower": [],
            "skos:prefLabel": "Hydro Multi-E"
        },
        {
            "@id": "https://grundfos.com/concept/productFamily/HYMULS",
            "@type": [
                "gfs:ProductFamily",
                "skos:Concept"
            ],
            "gfs:level": 1,
            "gfs:typecode": "HYMULS",
            "rdfs:comment": "Turn Key Pressure boosting system for boosting of water in flats, hotels etc. Available with 2-3 parallel connected pumps, with an integrated controller and all necessary fittings",
            "skos:inScheme": "https://grundfos.com/concept/productFamily",
            "skos:narrower": [],
            "skos:prefLabel": "Hydro Multi-S"
        },
        {
            "@id": "https://grundfos.com/concept/productFamily/HMONOE",
            "@type": [
                "gfs:ProductFamily",
                "skos:Concept"
            ],
            "gfs:level": 1,
            "gfs:typecode": "HMONOE",
            "rdfs:comment": "Grundfos Hydro Solo-E booster set is a fully-optimized booster system with constant pressure control, flow estimation and plug-and-pump installation.",
            "skos:inScheme": "https://grundfos.com/concept/productFamily",
            "skos:narrower": [],
            "skos:prefLabel": "Hydro Solo-E"
        },
        {
            "@id": "https://grundfos.com/concept/productFamily/HYDGEN",
            "@type": [
                "gfs:ProductFamily",
                "skos:Concept"
            ],
            "gfs:level": 1,
            "gfs:typecode": "HYDGEN",
            "rdfs:comment": "Hydrogen sulphide causes odour and corrosion in sewer systems, and it can pose a serious health hazard to operating staff. Grundfos Hydrogen Sulphide Solution automatically monitors actual measures all H2S occurrences in sewers and manholes. Based on these measurements, the optimal dosage is found and used in the wastewater over the subsequent days.",
            "skos:inScheme": "https://grundfos.com/concept/productFamily",
            "skos:narrower": [],
            "skos:prefLabel": "Hydrogen sulphide solution"
        },
        {
            "@id": "https://grundfos.com/concept/productFamily/IGRID",
            "@type": [
                "gfs:ProductFamily",
                "skos:Concept"
            ],
            "gfs:level": 1,
            "gfs:typecode": "IGRID",
            "rdfs:comment": "Grundfos iGRID solutions enables optimisation of distribution in even the largest district heating networks by dividing them into low-temperature zones with uniform building masses. Within each zone, iGRID ensures optimum operation by means of standardized mixing loops in wells or cabinets and control via real-time data, enabling us to deliver exactly the temperature and energy needed.",
            "skos:inScheme": "https://grundfos.com/concept/productFamily",
            "skos:narrower": [],
            "skos:prefLabel": "iGRID"
        },
        {
            "@id": "https://grundfos.com/concept/productFamily/JPPMBO",
            "@type": [
                "gfs:ProductFamily",
                "skos:Concept"
            ],
            "gfs:level": 2,
            "gfs:typecode": "JPPMBO",
            "rdfs:comment": "JP PM are boosters that consist of a pressure manager and a self-priming, single-stage centrifugal pump. Designed for a wide range of garden and domestic applications, including water supply and transfer duties in the home.",
            "skos:inScheme": "https://grundfos.com/concept/productFamily",
            "skos:prefLabel": "JP PM boosters"
        },
        {
            "@id": "https://grundfos.com/concept/productFamily/JPPTHB",
            "@type": [
                "gfs:ProductFamily",
                "skos:Concept"
            ],
            "gfs:level": 2,
            "gfs:typecode": "JPPTHB",
            "rdfs:comment": "JP PT-H are boosters that consist of a horizontal pressure tank and a self-priming, single-stage centrifugal pump with stainless-steel pump housings. Designed for a wide range of garden and domestic applications, including water supply and transfer duties in the home.",
            "skos:inScheme": "https://grundfos.com/concept/productFamily",
            "skos:prefLabel": "JP PT-H boosters"
        },
        {
            "@id": "https://grundfos.com/concept/productFamily/JPPTVB",
            "@type": [
                "gfs:ProductFamily",
                "skos:Concept"
            ],
            "gfs:level": 2,
            "gfs:typecode": "JPPTVB",
            "rdfs:comment": "JP PT-V are boosters that consist of a vertical pressure tank and a self-priming, single-stage centrifugal pump with stainless-steel pump housings. Designed for a wide range of garden and domestic applications, including water supply and transfer duties in the home.",
            "skos:inScheme": "https://grundfos.com/concept/productFamily",
            "skos:prefLabel": "JP PT-V boosters"
        },
        {
            "@id": "https://grundfos.com/concept/productFamily/JPDB0",
            "@type": [
                "gfs:ProductFamily",
                "skos:Concept"
            ],
            "gfs:level": 2,
            "gfs:typecode": "JPDB0",
            "rdfs:comment": "JPD are boosters consist of a pressure tank and a self-priming, single-stage centrifugal pump with cast iron pump housings. Designed for deep-well applications.",
            "skos:inScheme": "https://grundfos.com/concept/productFamily",
            "skos:prefLabel": "JPD boosters"
        },
        {
            "@id": "https://grundfos.com/concept/productFamily/JPB00",
            "@type": [
                "gfs:ProductFamily",
                "skos:Concept"
            ],
            "gfs:level": 1,
            "gfs:typecode": "JPB00",
            "rdfs:comment": "Grundfos Jet boosters consist of a pressure tank and a self-priming, single-stage centrifugal pump. Designed for a wide range of garden and domestic applications, including water supply and transfer duties in the home. JPD are suitable for deep-well applications.",
            "skos:inScheme": "https://grundfos.com/concept/productFamily",
            "skos:narrower": [
                "https://grundfos.com/concept/productFamily/JPPMBO",
                "https://grundfos.com/concept/productFamily/JPPTHB",
                "https://grundfos.com/concept/productFamily/JPPTVB",
                "https://grundfos.com/concept/productFamily/JPDB0"
            ],
            "skos:prefLabel": "Jet boosters"
        },
        {
            "@id": "https://grundfos.com/concept/productFamily/JP100",
            "@type": [
                "gfs:ProductFamily",
                "skos:Concept"
            ],
            "gfs:level": 2,
            "gfs:typecode": "JP100",
            "rdfs:comment": "Grundfos JP are self-priming, single-stage centrifugal pumps with stainless-steel pump housings, designed for a wide range of garden and domestic applications, including water supply and transfer duties in the home.",
            "skos:inScheme": "https://grundfos.com/concept/productFamily",
            "skos:prefLabel": "JP"
        },
        {
            "@id": "https://grundfos.com/concept/productFamily/JPFAM",
            "@type": [
                "gfs:ProductFamily",
                "skos:Concept"
            ],
            "gfs:level": 1,
            "gfs:typecode": "JPFAM",
            "rdfs:comment": "Grundfos Jet Pumps are self-priming single-stage centrifugal pumps, designed for a wide range of domestic applications, including water supply and transfer duties in home, and garden applications.",
            "skos:inScheme": "https://grundfos.com/concept/productFamily",
            "skos:narrower": [
                "https://grundfos.com/concept/productFamily/JP100"
            ],
            "skos:prefLabel": "Jet pumps"
        },
        {
            "@id": "https://grundfos.com/concept/productFamily/KPC00",
            "@type": [
                "gfs:ProductFamily",
                "skos:Concept"
            ],
            "gfs:level": 1,
            "gfs:typecode": "KPC00",
            "rdfs:comment": "Submersible Grundfos Drainage Pumps (DP) cover a motor range of 0.9-2.6 kW. The pumps are fitted with a semi-open multi-vane impeller capable of handling solids up to 10 mm size.",
            "skos:inScheme": "https://grundfos.com/concept/productFamily",
            "skos:narrower": [],
            "skos:prefLabel": "KPC"
        },
        {
            "@id": "https://grundfos.com/concept/productFamily/KPGFAM",
            "@type": [
                "gfs:ProductFamily",
                "skos:Concept"
            ],
            "gfs:level": 1,
            "gfs:typecode": "KPGFAM",
            "rdfs:comment": "The KPG axial-flow propeller pump is designed for flood and storm water transportation in pump gate installations",
            "skos:inScheme": "https://grundfos.com/concept/productFamily",
            "skos:narrower": [],
            "skos:prefLabel": "KPG"
        },
        {
            "@id": "https://grundfos.com/concept/productFamily/KPLFAM",
            "@type": [
                "gfs:ProductFamily",
                "skos:Concept"
            ],
            "gfs:level": 1,
            "gfs:typecode": "KPLFAM",
            "rdfs:comment": "The KPL axial-flow propeller pump is designed for high flow at low head.",
            "skos:inScheme": "https://grundfos.com/concept/productFamily",
            "skos:narrower": [],
            "skos:prefLabel": "KPL"
        },
        {
            "@id": "https://grundfos.com/concept/productFamily/KWMFAM",
            "@type": [
                "gfs:ProductFamily",
                "skos:Concept"
            ],
            "gfs:level": 1,
            "gfs:typecode": "KWMFAM",
            "rdfs:comment": "The KWM mixed-flow pump is designed for high flow at medium head.",
            "skos:inScheme": "https://grundfos.com/concept/productFamily",
            "skos:narrower": [],
            "skos:prefLabel": "KWM"
        },
        {
            "@id": "https://grundfos.com/concept/productFamily/LSSM",
            "@type": [
                "gfs:ProductFamily",
                "skos:Concept"
            ],
            "gfs:level": 2,
            "gfs:typecode": "LSSM",
            "rdfs:comment": "The horizontal split case, double suction, double volute LS pump is designed for high flow, low NPSH and high efficient application.",
            "skos:inScheme": "https://grundfos.com/concept/productFamily",
            "skos:prefLabel": "LS"
        },
        {
            "@id": "https://grundfos.com/concept/productFamily/LSFAM",
            "@type": [
                "gfs:ProductFamily",
                "skos:Concept"
            ],
            "gfs:level": 1,
            "gfs:typecode": "LSFAM",
            "rdfs:comment": "The horizontal split case, double suction, double volute LS pump is designed for high flow, low NPSH and high efficient application.",
            "skos:inScheme": "https://grundfos.com/concept/productFamily",
            "skos:narrower": [
                "https://grundfos.com/concept/productFamily/LSSM"
            ],
            "skos:prefLabel": "LS"
        },
        {
            "@id": "https://grundfos.com/concept/productFamily/MAGNA1",
            "@type": [
                "gfs:ProductFamily",
                "skos:Concept"
            ],
            "gfs:level": 2,
            "gfs:typecode": "MAGNA1",
            "rdfs:comment": "The simple option for a job well done. The product has an intuitive user interface, which is especially fit for replacement of older circulators. The ideal choice for basic functionality needs",
            "skos:inScheme": "https://grundfos.com/concept/productFamily",
            "skos:prefLabel": "MAGNA1"
        },
        {
            "@id": "https://grundfos.com/concept/productFamily/MAGNA1D",
            "@type": [
                "gfs:ProductFamily",
                "skos:Concept"
            ],
            "gfs:level": 2,
            "gfs:typecode": "MAGNA1D",
            "rdfs:comment": "Double the pump performance or enjoy reduced downtime in service by having redundancy from the twin pump (manual change over). The basic product which can be operated from an intuitive user interface.",
            "skos:inScheme": "https://grundfos.com/concept/productFamily",
            "skos:prefLabel": "MAGNA1 D"
        },
        {
            "@id": "https://grundfos.com/concept/productFamily/MAGNA1N",
            "@type": [
                "gfs:ProductFamily",
                "skos:Concept"
            ],
            "gfs:level": 2,
            "gfs:typecode": "MAGNA1N",
            "rdfs:comment": "MAGNA1 N is the stainless steel variant for applications where the media requires this (e.g. domestic hot water). With MAGNA1, the job is done in an intuitive and efficient way.",
            "skos:inScheme": "https://grundfos.com/concept/productFamily",
            "skos:prefLabel": "MAGNA1 N"
        },
        {
            "@id": "https://grundfos.com/concept/productFamily/MAGNA3",
            "@type": [
                "gfs:ProductFamily",
                "skos:Concept"
            ],
            "gfs:level": 2,
            "gfs:typecode": "MAGNA3",
            "rdfs:comment": "The premium choice when system control and monitoring is key. The MAGNA3 supports fieldbus by optional CIM modules and has a TFT display for intuitive configuration of the intelligent features.",
            "skos:inScheme": "https://grundfos.com/concept/productFamily",
            "skos:prefLabel": "MAGNA3"
        },
        {
            "@id": "https://grundfos.com/concept/productFamily/MAGNA3D",
            "@type": [
                "gfs:ProductFamily",
                "skos:Concept"
            ],
            "gfs:level": 2,
            "gfs:typecode": "MAGNA3D",
            "rdfs:comment": "Double the performance or enjoy reduced downtime in service by having redundancy from the twin pump which operates wirelessly. The intelligence in the MAGNA3 caters for all application needs.",
            "skos:inScheme": "https://grundfos.com/concept/productFamily",
            "skos:prefLabel": "MAGNA3 D"
        },
        {
            "@id": "https://grundfos.com/concept/productFamily/MAGNA3N",
            "@type": [
                "gfs:ProductFamily",
                "skos:Concept"
            ],
            "gfs:level": 2,
            "gfs:typecode": "MAGNA3N",
            "rdfs:comment": "Get all of the premium features and the best in class efficiency of MAGNA3 in a stainless steel variant if the media requires this (e.g. domestic hot water).",
            "skos:inScheme": "https://grundfos.com/concept/productFamily",
            "skos:prefLabel": "MAGNA3 N"
        },
        {
            "@id": "https://grundfos.com/concept/productFamily/UPEFAM",
            "@type": [
                "gfs:ProductFamily",
                "skos:Concept"
            ],
            "gfs:level": 1,
            "gfs:typecode": "UPEFAM",
            "rdfs:comment": "Electronically controlled and high efficiency circulator pumps for commercial building",
            "skos:inScheme": "https://grundfos.com/concept/productFamily",
            "skos:narrower": [
                "https://grundfos.com/concept/productFamily/MAGNA1",
                "https://grundfos.com/concept/productFamily/MAGNA1D",
                "https://grundfos.com/concept/productFamily/MAGNA1N",
                "https://grundfos.com/concept/productFamily/MAGNA3",
                "https://grundfos.com/concept/productFamily/MAGNA3D",
                "https://grundfos.com/concept/productFamily/MAGNA3N"
            ],
            "skos:prefLabel": "MAGNA"
        },
        {
            "@id": "https://grundfos.com/concept/productFamily/ACCPART",
            "@type": [
                "gfs:ProductFamily",
                "skos:Concept"
            ],
            "gfs:level": 2,
            "gfs:typecode": "ACCPART",
            "rdfs:comment": "Accessories",
            "skos:inScheme": "https://grundfos.com/concept/productFamily",
            "skos:prefLabel": "Accessories and spare parts"
        },
        {
            "@id": "https://grundfos.com/concept/productFamily/DIA00",
            "@type": [
                "gfs:ProductFamily",
                "skos:Concept"
            ],
            "gfs:level": 2,
            "gfs:typecode": "DIA00",
            "rdfs:comment": "Controllers for water quality, 1 or 2 parameters",
            "skos:inScheme": "https://grundfos.com/concept/productFamily",
            "skos:prefLabel": "Conex DIA"
        },
        {
            "@id": "https://grundfos.com/concept/productFamily/DIA-G1",
            "@type": [
                "gfs:ProductFamily",
                "skos:Concept"
            ],
            "gfs:level": 2,
            "gfs:typecode": "DIA-G1",
            "rdfs:comment": "Gas warning unit for gas detection",
            "skos:inScheme": "https://grundfos.com/concept/productFamily",
            "skos:prefLabel": "Conex DIA-G and DIS-G"
        },
        {
            "@id": "https://grundfos.com/concept/productFamily/DIA-G",
            "@type": [
                "gfs:ProductFamily",
                "skos:Concept"
            ],
            "gfs:level": 2,
            "gfs:typecode": "DIA-G",
            "rdfs:comment": "Gas warning unit for gas detection",
            "skos:inScheme": "https://grundfos.com/concept/productFamily",
            "skos:prefLabel": "Conex DIA-G-P and DIS-G-P"
        },
        {
            "@id": "https://grundfos.com/concept/productFamily/DIS00",
            "@type": [
                "gfs:ProductFamily",
                "skos:Concept"
            ],
            "gfs:level": 2,
            "gfs:typecode": "DIS00",
            "rdfs:comment": "Controllers for water quality (1 parameter)",
            "skos:inScheme": "https://grundfos.com/concept/productFamily",
            "skos:prefLabel": "Conex DIS-D and DIS-PR"
        },
        {
            "@id": "https://grundfos.com/concept/productFamily/DID00",
            "@type": [
                "gfs:ProductFamily",
                "skos:Concept"
            ],
            "gfs:level": 2,
            "gfs:typecode": "DID00",
            "rdfs:comment": "Testing in addition to the standard performance and hydrostatic testing required by UL, FM, and NFPA 20",
            "skos:inScheme": "https://grundfos.com/concept/productFamily",
            "skos:prefLabel": "DID"
        },
        {
            "@id": "https://grundfos.com/concept/productFamily/MEASSEN",
            "@type": [
                "gfs:ProductFamily",
                "skos:Concept"
            ],
            "gfs:level": 2,
            "gfs:typecode": "MEASSEN",
            "rdfs:comment": "Measuring cells & sensors for water and gas",
            "skos:inScheme": "https://grundfos.com/concept/productFamily",
            "skos:prefLabel": "Measuring cells & Sensors"
        },
        {
            "@id": "https://grundfos.com/concept/productFamily/PHOTOM",
            "@type": [
                "gfs:ProductFamily",
                "skos:Concept"
            ],
            "gfs:level": 2,
            "gfs:typecode": "PHOTOM",
            "rdfs:comment": "Hand photometer for water analysis and calibration",
            "skos:inScheme": "https://grundfos.com/concept/productFamily",
            "skos:prefLabel": "Photometers"
        },
        {
            "@id": "https://grundfos.com/concept/productFamily/MEASCONT",
            "@type": [
                "gfs:ProductFamily",
                "skos:Concept"
            ],
            "gfs:level": 1,
            "gfs:typecode": "MEASCONT",
            "rdfs:comment": "Measuring amplifiers and controllers for dosing processes",
            "skos:inScheme": "https://grundfos.com/concept/productFamily",
            "skos:narrower": [
                "https://grundfos.com/concept/productFamily/ACCPART",
                "https://grundfos.com/concept/productFamily/DIA00",
                "https://grundfos.com/concept/productFamily/DIA-G1",
                "https://grundfos.com/concept/productFamily/DIA-G",
                "https://grundfos.com/concept/productFamily/DIS00",
                "https://grundfos.com/concept/productFamily/DID00",
                "https://grundfos.com/concept/productFamily/MEASSEN",
                "https://grundfos.com/concept/productFamily/PHOTOM"
            ],
            "skos:prefLabel": "Measurement & Control"
        },
        {
            "@id": "https://grundfos.com/concept/productFamily/MG071",
            "@type": [
                "gfs:ProductFamily",
                "skos:Concept"
            ],
            "gfs:level": 2,
            "gfs:typecode": "MG071",
            "rdfs:comment": "Standard motors",
            "skos:inScheme": "https://grundfos.com/concept/productFamily",
            "skos:prefLabel": "MG, ML 71"
        },
        {
            "@id": "https://grundfos.com/concept/productFamily/MG080",
            "@type": [
                "gfs:ProductFamily",
                "skos:Concept"
            ],
            "gfs:level": 2,
            "gfs:typecode": "MG080",
            "rdfs:comment": "Standard motors",
            "skos:inScheme": "https://grundfos.com/concept/productFamily",
            "skos:prefLabel": "MG, ML 80"
        },
        {
            "@id": "https://grundfos.com/concept/productFamily/MG090",
            "@type": [
                "gfs:ProductFamily",
                "skos:Concept"
            ],
            "gfs:level": 2,
            "gfs:typecode": "MG090",
            "rdfs:comment": "Standard motors",
            "skos:inScheme": "https://grundfos.com/concept/productFamily",
            "skos:prefLabel": "MG, ML 90"
        },
        {
            "@id": "https://grundfos.com/concept/productFamily/MG100",
            "@type": [
                "gfs:ProductFamily",
                "skos:Concept"
            ],
            "gfs:level": 2,
            "gfs:typecode": "MG100",
            "rdfs:comment": "Standard motors",
            "skos:inScheme": "https://grundfos.com/concept/productFamily",
            "skos:prefLabel": "MG, ML 100"
        },
        {
            "@id": "https://grundfos.com/concept/productFamily/MG112",
            "@type": [
                "gfs:ProductFamily",
                "skos:Concept"
            ],
            "gfs:level": 2,
            "gfs:typecode": "MG112",
            "rdfs:comment": "Standard motors",
            "skos:inScheme": "https://grundfos.com/concept/productFamily",
            "skos:prefLabel": "MG, ML 112"
        },
        {
            "@id": "https://grundfos.com/concept/productFamily/MG132",
            "@type": [
                "gfs:ProductFamily",
                "skos:Concept"
            ],
            "gfs:level": 2,
            "gfs:typecode": "MG132",
            "rdfs:comment": "Standard motors",
            "skos:inScheme": "https://grundfos.com/concept/productFamily",
            "skos:prefLabel": "MG, ML 132"
        },
        {
            "@id": "https://grundfos.com/concept/productFamily/MG160",
            "@type": [
                "gfs:ProductFamily",
                "skos:Concept"
            ],
            "gfs:level": 2,
            "gfs:typecode": "MG160",
            "rdfs:comment": "Standard motors",
            "skos:inScheme": "https://grundfos.com/concept/productFamily",
            "skos:prefLabel": "MG, ML 160"
        },
        {
            "@id": "https://grundfos.com/concept/productFamily/MG180",
            "@type": [
                "gfs:ProductFamily",
                "skos:Concept"
            ],
            "gfs:level": 2,
            "gfs:typecode": "MG180",
            "rdfs:comment": "Standard motors",
            "skos:inScheme": "https://grundfos.com/concept/productFamily",
            "skos:prefLabel": "MG, ML 180"
        },
        {
            "@id": "https://grundfos.com/concept/productFamily/MGFAM",
            "@type": [
                "gfs:ProductFamily",
                "skos:Concept"
            ],
            "gfs:level": 1,
            "gfs:typecode": "MGFAM",
            "rdfs:comment": "Standard norm motors",
            "skos:inScheme": "https://grundfos.com/concept/productFamily",
            "skos:narrower": [
                "https://grundfos.com/concept/productFamily/MG071",
                "https://grundfos.com/concept/productFamily/MG080",
                "https://grundfos.com/concept/productFamily/MG090",
                "https://grundfos.com/concept/productFamily/MG100",
                "https://grundfos.com/concept/productFamily/MG112",
                "https://grundfos.com/concept/productFamily/MG132",
                "https://grundfos.com/concept/productFamily/MG160",
                "https://grundfos.com/concept/productFamily/MG180"
            ],
            "skos:prefLabel": "MG, ML"
        },
        {
            "@id": "https://grundfos.com/concept/productFamily/MGE071",
            "@type": [
                "gfs:ProductFamily",
                "skos:Concept"
            ],
            "gfs:level": 2,
            "gfs:typecode": "MGE071",
            "rdfs:comment": "Standard norm motors with speed control",
            "skos:inScheme": "https://grundfos.com/concept/productFamily",
            "skos:prefLabel": "MGE, MLE 71"
        },
        {
            "@id": "https://grundfos.com/concept/productFamily/MGE080",
            "@type": [
                "gfs:ProductFamily",
                "skos:Concept"
            ],
            "gfs:level": 2,
            "gfs:typecode": "MGE080",
            "rdfs:comment": "Standard norm motors with speed control",
            "skos:inScheme": "https://grundfos.com/concept/productFamily",
            "skos:prefLabel": "MGE, MLE 80"
        },
        {
            "@id": "https://grundfos.com/concept/productFamily/MGE090",
            "@type": [
                "gfs:ProductFamily",
                "skos:Concept"
            ],
            "gfs:level": 2,
            "gfs:typecode": "MGE090",
            "rdfs:comment": "Standard norm motors with speed control",
            "skos:inScheme": "https://grundfos.com/concept/productFamily",
            "skos:prefLabel": "MGE, MLE 90"
        },
        {
            "@id": "https://grundfos.com/concept/productFamily/MGE100",
            "@type": [
                "gfs:ProductFamily",
                "skos:Concept"
            ],
            "gfs:level": 2,
            "gfs:typecode": "MGE100",
            "rdfs:comment": "Standard norm motors with speed control",
            "skos:inScheme": "https://grundfos.com/concept/productFamily",
            "skos:prefLabel": "MGE, MLE 100"
        },
        {
            "@id": "https://grundfos.com/concept/productFamily/MGE112",
            "@type": [
                "gfs:ProductFamily",
                "skos:Concept"
            ],
            "gfs:level": 2,
            "gfs:typecode": "MGE112",
            "rdfs:comment": "Standard norm motors with speed control",
            "skos:inScheme": "https://grundfos.com/concept/productFamily",
            "skos:prefLabel": "MGE, MLE 112"
        },
        {
            "@id": "https://grundfos.com/concept/productFamily/MGE132",
            "@type": [
                "gfs:ProductFamily",
                "skos:Concept"
            ],
            "gfs:level": 2,
            "gfs:typecode": "MGE132",
            "rdfs:comment": "Standard norm motors with speed control",
            "skos:inScheme": "https://grundfos.com/concept/productFamily",
            "skos:prefLabel": "MGE, MLE 132"
        },
        {
            "@id": "https://grundfos.com/concept/productFamily/MGE160",
            "@type": [
                "gfs:ProductFamily",
                "skos:Concept"
            ],
            "gfs:level": 2,
            "gfs:typecode": "MGE160",
            "rdfs:comment": "Standard norm motors with speed control",
            "skos:inScheme": "https://grundfos.com/concept/productFamily",
            "skos:prefLabel": "MGE, MLE 160"
        },
        {
            "@id": "https://grundfos.com/concept/productFamily/MGE180",
            "@type": [
                "gfs:ProductFamily",
                "skos:Concept"
            ],
            "gfs:level": 2,
            "gfs:typecode": "MGE180",
            "rdfs:comment": "Standard norm motors with speed control",
            "skos:inScheme": "https://grundfos.com/concept/productFamily",
            "skos:prefLabel": "MGE, MLE 180"
        },
        {
            "@id": "https://grundfos.com/concept/productFamily/MGEFAM",
            "@type": [
                "gfs:ProductFamily",
                "skos:Concept"
            ],
            "gfs:level": 1,
            "gfs:typecode": "MGEFAM",
            "rdfs:comment": "Standard norm motors with speed control",
            "skos:inScheme": "https://grundfos.com/concept/productFamily",
            "skos:narrower": [
                "https://grundfos.com/concept/productFamily/MGE071",
                "https://grundfos.com/concept/productFamily/MGE080",
                "https://grundfos.com/concept/productFamily/MGE090",
                "https://grundfos.com/concept/productFamily/MGE100",
                "https://grundfos.com/concept/productFamily/MGE112",
                "https://grundfos.com/concept/productFamily/MGE132",
                "https://grundfos.com/concept/productFamily/MGE160",
                "https://grundfos.com/concept/productFamily/MGE180"
            ],
            "skos:prefLabel": "MGE, MLE"
        },
        {
            "@id": "https://grundfos.com/concept/productFamily/MGEFLEX",
            "@type": [
                "gfs:ProductFamily",
                "skos:Concept"
            ],
            "gfs:level": 1,
            "gfs:typecode": "MGEFLEX",
            "rdfs:comment": "Renewable norm motor with speed control",
            "skos:inScheme": "https://grundfos.com/concept/productFamily",
            "skos:narrower": [],
            "skos:prefLabel": "MGFlex"
        },
        {
            "@id": "https://grundfos.com/concept/productFamily/MMG063",
            "@type": [
                "gfs:ProductFamily",
                "skos:Concept"
            ],
            "gfs:level": 2,
            "gfs:typecode": "MMG063",
            "rdfs:comment": "Standard motors",
            "skos:inScheme": "https://grundfos.com/concept/productFamily",
            "skos:prefLabel": "MMG 63"
        },
        {
            "@id": "https://grundfos.com/concept/productFamily/MMG071",
            "@type": [
                "gfs:ProductFamily",
                "skos:Concept"
            ],
            "gfs:level": 2,
            "gfs:typecode": "MMG071",
            "rdfs:comment": "Standard motors",
            "skos:inScheme": "https://grundfos.com/concept/productFamily",
            "skos:prefLabel": "MMG 71"
        },
        {
            "@id": "https://grundfos.com/concept/productFamily/MMG080",
            "@type": [
                "gfs:ProductFamily",
                "skos:Concept"
            ],
            "gfs:level": 2,
            "gfs:typecode": "MMG080",
            "rdfs:comment": "Standard motors",
            "skos:inScheme": "https://grundfos.com/concept/productFamily",
            "skos:prefLabel": "MMG 80"
        },
        {
            "@id": "https://grundfos.com/concept/productFamily/MMG090",
            "@type": [
                "gfs:ProductFamily",
                "skos:Concept"
            ],
            "gfs:level": 2,
            "gfs:typecode": "MMG090",
            "rdfs:comment": "Standard motors",
            "skos:inScheme": "https://grundfos.com/concept/productFamily",
            "skos:prefLabel": "MMG 90"
        },
        {
            "@id": "https://grundfos.com/concept/productFamily/MMG100",
            "@type": [
                "gfs:ProductFamily",
                "skos:Concept"
            ],
            "gfs:level": 2,
            "gfs:typecode": "MMG100",
            "rdfs:comment": "Standard motors",
            "skos:inScheme": "https://grundfos.com/concept/productFamily",
            "skos:prefLabel": "MMG 100"
        },
        {
            "@id": "https://grundfos.com/concept/productFamily/MMG112",
            "@type": [
                "gfs:ProductFamily",
                "skos:Concept"
            ],
            "gfs:level": 2,
            "gfs:typecode": "MMG112",
            "rdfs:comment": "Standard motors",
            "skos:inScheme": "https://grundfos.com/concept/productFamily",
            "skos:prefLabel": "MMG 112"
        },
        {
            "@id": "https://grundfos.com/concept/productFamily/MMG132",
            "@type": [
                "gfs:ProductFamily",
                "skos:Concept"
            ],
            "gfs:level": 2,
            "gfs:typecode": "MMG132",
            "rdfs:comment": "Standard motors",
            "skos:inScheme": "https://grundfos.com/concept/productFamily",
            "skos:prefLabel": "MMG 132"
        },
        {
            "@id": "https://grundfos.com/concept/productFamily/MMG160",
            "@type": [
                "gfs:ProductFamily",
                "skos:Concept"
            ],
            "gfs:level": 2,
            "gfs:typecode": "MMG160",
            "rdfs:comment": "Standard motors",
            "skos:inScheme": "https://grundfos.com/concept/productFamily",
            "skos:prefLabel": "MMG 160"
        },
        {
            "@id": "https://grundfos.com/concept/productFamily/MMG180",
            "@type": [
                "gfs:ProductFamily",
                "skos:Concept"
            ],
            "gfs:level": 2,
            "gfs:typecode": "MMG180",
            "rdfs:comment": "Standard motors",
            "skos:inScheme": "https://grundfos.com/concept/productFamily",
            "skos:prefLabel": "MMG 180"
        },
        {
            "@id": "https://grundfos.com/concept/productFamily/MMG200",
            "@type": [
                "gfs:ProductFamily",
                "skos:Concept"
            ],
            "gfs:level": 2,
            "gfs:typecode": "MMG200",
            "rdfs:comment": "Standard motors",
            "skos:inScheme": "https://grundfos.com/concept/productFamily",
            "skos:prefLabel": "MMG 200"
        },
        {
            "@id": "https://grundfos.com/concept/productFamily/MMG225",
            "@type": [
                "gfs:ProductFamily",
                "skos:Concept"
            ],
            "gfs:level": 2,
            "gfs:typecode": "MMG225",
            "rdfs:comment": "Standard motors",
            "skos:inScheme": "https://grundfos.com/concept/productFamily",
            "skos:prefLabel": "MMG 225"
        },
        {
            "@id": "https://grundfos.com/concept/productFamily/MMG250",
            "@type": [
                "gfs:ProductFamily",
                "skos:Concept"
            ],
            "gfs:level": 2,
            "gfs:typecode": "MMG250",
            "rdfs:comment": "Standard motors",
            "skos:inScheme": "https://grundfos.com/concept/productFamily",
            "skos:prefLabel": "MMG 250"
        },
        {
            "@id": "https://grundfos.com/concept/productFamily/MMG280",
            "@type": [
                "gfs:ProductFamily",
                "skos:Concept"
            ],
            "gfs:level": 2,
            "gfs:typecode": "MMG280",
            "rdfs:comment": "Standard motors",
            "skos:inScheme": "https://grundfos.com/concept/productFamily",
            "skos:prefLabel": "MMG 280"
        },
        {
            "@id": "https://grundfos.com/concept/productFamily/MMG315",
            "@type": [
                "gfs:ProductFamily",
                "skos:Concept"
            ],
            "gfs:level": 2,
            "gfs:typecode": "MMG315",
            "rdfs:comment": "Standard motors",
            "skos:inScheme": "https://grundfos.com/concept/productFamily",
            "skos:prefLabel": "MMG 315"
        },
        {
            "@id": "https://grundfos.com/concept/productFamily/MMG355",
            "@type": [
                "gfs:ProductFamily",
                "skos:Concept"
            ],
            "gfs:level": 2,
            "gfs:typecode": "MMG355",
            "rdfs:comment": "Standard motors",
            "skos:inScheme": "https://grundfos.com/concept/productFamily",
            "skos:prefLabel": "MMG 355"
        },
        {
            "@id": "https://grundfos.com/concept/productFamily/MMG400",
            "@type": [
                "gfs:ProductFamily",
                "skos:Concept"
            ],
            "gfs:level": 2,
            "gfs:typecode": "MMG400",
            "rdfs:comment": "Standard motors",
            "skos:inScheme": "https://grundfos.com/concept/productFamily",
            "skos:prefLabel": "MMG 400"
        },
        {
            "@id": "https://grundfos.com/concept/productFamily/MMG450",
            "@type": [
                "gfs:ProductFamily",
                "skos:Concept"
            ],
            "gfs:level": 2,
            "gfs:typecode": "MMG450",
            "rdfs:comment": "Standard motors",
            "skos:inScheme": "https://grundfos.com/concept/productFamily",
            "skos:prefLabel": "MMG 450"
        },
        {
            "@id": "https://grundfos.com/concept/productFamily/MMG500",
            "@type": [
                "gfs:ProductFamily",
                "skos:Concept"
            ],
            "gfs:level": 2,
            "gfs:typecode": "MMG500",
            "rdfs:comment": "Standard motors",
            "skos:inScheme": "https://grundfos.com/concept/productFamily",
            "skos:prefLabel": "MMG 500"
        },
        {
            "@id": "https://grundfos.com/concept/productFamily/MMG560",
            "@type": [
                "gfs:ProductFamily",
                "skos:Concept"
            ],
            "gfs:level": 2,
            "gfs:typecode": "MMG560",
            "rdfs:comment": "Standard motors",
            "skos:inScheme": "https://grundfos.com/concept/productFamily",
            "skos:prefLabel": "MMG 560"
        },
        {
            "@id": "https://grundfos.com/concept/productFamily/MMG630",
            "@type": [
                "gfs:ProductFamily",
                "skos:Concept"
            ],
            "gfs:level": 2,
            "gfs:typecode": "MMG630",
            "rdfs:comment": "Standard motors",
            "skos:inScheme": "https://grundfos.com/concept/productFamily",
            "skos:prefLabel": "MMG 630"
        },
        {
            "@id": "https://grundfos.com/concept/productFamily/MMGFAM",
            "@type": [
                "gfs:ProductFamily",
                "skos:Concept"
            ],
            "gfs:level": 1,
            "gfs:typecode": "MMGFAM",
            "rdfs:comment": "Standard norm sourced motors",
            "skos:inScheme": "https://grundfos.com/concept/productFamily",
            "skos:narrower": [
                "https://grundfos.com/concept/productFamily/MMG063",
                "https://grundfos.com/concept/productFamily/MMG071",
                "https://grundfos.com/concept/productFamily/MMG080",
                "https://grundfos.com/concept/productFamily/MMG090",
                "https://grundfos.com/concept/productFamily/MMG100",
                "https://grundfos.com/concept/productFamily/MMG112",
                "https://grundfos.com/concept/productFamily/MMG132",
                "https://grundfos.com/concept/productFamily/MMG160",
                "https://grundfos.com/concept/productFamily/MMG180",
                "https://grundfos.com/concept/productFamily/MMG200",
                "https://grundfos.com/concept/productFamily/MMG225",
                "https://grundfos.com/concept/productFamily/MMG250",
                "https://grundfos.com/concept/productFamily/MMG280",
                "https://grundfos.com/concept/productFamily/MMG315",
                "https://grundfos.com/concept/productFamily/MMG355",
                "https://grundfos.com/concept/productFamily/MMG400",
                "https://grundfos.com/concept/productFamily/MMG450",
                "https://grundfos.com/concept/productFamily/MMG500",
                "https://grundfos.com/concept/productFamily/MMG560",
                "https://grundfos.com/concept/productFamily/MMG630"
            ],
            "skos:prefLabel": "MMG"
        },
        {
            "@id": "https://grundfos.com/concept/productFamily/MMS08",
            "@type": [
                "gfs:ProductFamily",
                "skos:Concept"
            ],
            "gfs:level": 2,
            "gfs:typecode": "MMS08",
            "rdfs:comment": "Submersible motors",
            "skos:inScheme": "https://grundfos.com/concept/productFamily",
            "skos:prefLabel": "MMS 8000"
        },
        {
            "@id": "https://grundfos.com/concept/productFamily/MMS10",
            "@type": [
                "gfs:ProductFamily",
                "skos:Concept"
            ],
            "gfs:level": 2,
            "gfs:typecode": "MMS10",
            "rdfs:comment": "Submersible motors",
            "skos:inScheme": "https://grundfos.com/concept/productFamily",
            "skos:prefLabel": "MMS 10000"
        },
        {
            "@id": "https://grundfos.com/concept/productFamily/MMS12",
            "@type": [
                "gfs:ProductFamily",
                "skos:Concept"
            ],
            "gfs:level": 2,
            "gfs:typecode": "MMS12",
            "rdfs:comment": "Submersible motors",
            "skos:inScheme": "https://grundfos.com/concept/productFamily",
            "skos:prefLabel": "MMS 12000"
        },
        {
            "@id": "https://grundfos.com/concept/productFamily/MMS6FUMO",
            "@type": [
                "gfs:ProductFamily",
                "skos:Concept"
            ],
            "gfs:level": 2,
            "gfs:typecode": "MMS6FUMO",
            "rdfs:comment": "Submersible motors",
            "skos:inScheme": "https://grundfos.com/concept/productFamily",
            "skos:prefLabel": "MMS6"
        },
        {
            "@id": "https://grundfos.com/concept/productFamily/MMSFAM",
            "@type": [
                "gfs:ProductFamily",
                "skos:Concept"
            ],
            "gfs:level": 1,
            "gfs:typecode": "MMSFAM",
            "rdfs:comment": "Submersible motors",
            "skos:inScheme": "https://grundfos.com/concept/productFamily",
            "skos:narrower": [
                "https://grundfos.com/concept/productFamily/MMS08",
                "https://grundfos.com/concept/productFamily/MMS10",
                "https://grundfos.com/concept/productFamily/MMS12",
                "https://grundfos.com/concept/productFamily/MMS6FUMO"
            ],
            "skos:prefLabel": "MMS"
        },
        {
            "@id": "https://grundfos.com/concept/productFamily/MQFAM",
            "@type": [
                "gfs:ProductFamily",
                "skos:Concept"
            ],
            "gfs:level": 1,
            "gfs:typecode": "MQFAM",
            "rdfs:comment": "Grundfos MQ booster are an all-in-one unit, designed for pumping clean water from break tanks and shallow wells, and for general pressure-boosting in private homes, farms, and irrigation. The boosters are suitable for both indoor and outdoor use.",
            "skos:inScheme": "https://grundfos.com/concept/productFamily",
            "skos:narrower": [],
            "skos:prefLabel": "MQ"
        },
        {
            "@id": "https://grundfos.com/concept/productFamily/MS402",
            "@type": [
                "gfs:ProductFamily",
                "skos:Concept"
            ],
            "gfs:level": 2,
            "gfs:typecode": "MS402",
            "rdfs:comment": "Submersible motors",
            "skos:inScheme": "https://grundfos.com/concept/productFamily",
            "skos:prefLabel": "MS 402"
        },
        {
            "@id": "https://grundfos.com/concept/productFamily/MS4000",
            "@type": [
                "gfs:ProductFamily",
                "skos:Concept"
            ],
            "gfs:level": 2,
            "gfs:typecode": "MS4000",
            "rdfs:comment": "Submersible motors",
            "skos:inScheme": "https://grundfos.com/concept/productFamily",
            "skos:prefLabel": "MS 4000"
        },
        {
            "@id": "https://grundfos.com/concept/productFamily/MS6000",
            "@type": [
                "gfs:ProductFamily",
                "skos:Concept"
            ],
            "gfs:level": 2,
            "gfs:typecode": "MS6000",
            "rdfs:comment": "Submersible motors",
            "skos:inScheme": "https://grundfos.com/concept/productFamily",
            "skos:prefLabel": "MS6000"
        },
        {
            "@id": "https://grundfos.com/concept/productFamily/MSFAM",
            "@type": [
                "gfs:ProductFamily",
                "skos:Concept"
            ],
            "gfs:level": 1,
            "gfs:typecode": "MSFAM",
            "rdfs:comment": "Submersible motors",
            "skos:inScheme": "https://grundfos.com/concept/productFamily",
            "skos:narrower": [
                "https://grundfos.com/concept/productFamily/MS402",
                "https://grundfos.com/concept/productFamily/MS4000",
                "https://grundfos.com/concept/productFamily/MS6000"
            ],
            "skos:prefLabel": "MS"
        },
        {
            "@id": "https://grundfos.com/concept/productFamily/MS300",
            "@type": [
                "gfs:ProductFamily",
                "skos:Concept"
            ],
            "gfs:level": 1,
            "gfs:typecode": "MS300",
            "rdfs:comment": "Submersible motors for SQ pumps",
            "skos:inScheme": "https://grundfos.com/concept/productFamily",
            "skos:narrower": [],
            "skos:prefLabel": "MS 3"
        },
        {
            "@id": "https://grundfos.com/concept/productFamily/MSF3",
            "@type": [
                "gfs:ProductFamily",
                "skos:Concept"
            ],
            "gfs:level": 1,
            "gfs:typecode": "MSF3",
            "rdfs:comment": "Submersible motors for SQFlex pumps",
            "skos:inScheme": "https://grundfos.com/concept/productFamily",
            "skos:narrower": [],
            "skos:prefLabel": "MSF 3"
        },
        {
            "@id": "https://grundfos.com/concept/productFamily/CRKFAM",
            "@type": [
                "gfs:ProductFamily",
                "skos:Concept"
            ],
            "gfs:level": 2,
            "gfs:typecode": "CRKFAM",
            "rdfs:comment": "Vertical, multistage centrifugal pump for tank top mounting",
            "skos:inScheme": "https://grundfos.com/concept/productFamily",
            "skos:prefLabel": "CRK"
        },
        {
            "@id": "https://grundfos.com/concept/productFamily/MTAFAM",
            "@type": [
                "gfs:ProductFamily",
                "skos:Concept"
            ],
            "gfs:level": 2,
            "gfs:typecode": "MTAFAM",
            "rdfs:comment": "Single stage coolant pump for tank top mounting",
            "skos:inScheme": "https://grundfos.com/concept/productFamily",
            "skos:prefLabel": "MTA"
        },
        {
            "@id": "https://grundfos.com/concept/productFamily/MTDFAM",
            "@type": [
                "gfs:ProductFamily",
                "skos:Concept"
            ],
            "gfs:level": 2,
            "gfs:typecode": "MTDFAM",
            "rdfs:comment": "Vertical, multistage centrifugal pump with semi-open impeller for tank top mounting.",
            "skos:inScheme": "https://grundfos.com/concept/productFamily",
            "skos:prefLabel": "MTD"
        },
        {
            "@id": "https://grundfos.com/concept/productFamily/MTHFAM",
            "@type": [
                "gfs:ProductFamily",
                "skos:Concept"
            ],
            "gfs:level": 2,
            "gfs:typecode": "MTHFAM",
            "rdfs:comment": "Compact, vertical, multistage centrifugal pump for tank top mounting",
            "skos:inScheme": "https://grundfos.com/concept/productFamily",
            "skos:prefLabel": "MTH"
        },
        {
            "@id": "https://grundfos.com/concept/productFamily/MTRFAM",
            "@type": [
                "gfs:ProductFamily",
                "skos:Concept"
            ],
            "gfs:level": 2,
            "gfs:typecode": "MTRFAM",
            "rdfs:comment": "Vertical, multistage centrifugal pump for tank top mounting",
            "skos:inScheme": "https://grundfos.com/concept/productFamily",
            "skos:prefLabel": "MTR"
        },
        {
            "@id": "https://grundfos.com/concept/productFamily/MTREFAM",
            "@type": [
                "gfs:ProductFamily",
                "skos:Concept"
            ],
            "gfs:level": 2,
            "gfs:typecode": "MTREFAM",
            "rdfs:comment": "Vertical, multistage centrifugal pump for tank top mounting with intergrated frquency converter",
            "skos:inScheme": "https://grundfos.com/concept/productFamily",
            "skos:prefLabel": "MTRE"
        },
        {
            "@id": "https://grundfos.com/concept/productFamily/MTSFAM",
            "@type": [
                "gfs:ProductFamily",
                "skos:Concept"
            ],
            "gfs:level": 2,
            "gfs:typecode": "MTSFAM",
            "rdfs:comment": "Screw spindle pump for coolant and cutting oil",
            "skos:inScheme": "https://grundfos.com/concept/productFamily",
            "skos:prefLabel": "MTS"
        },
        {
            "@id": "https://grundfos.com/concept/productFamily/MTSEFAM",
            "@type": [
                "gfs:ProductFamily",
                "skos:Concept"
            ],
            "gfs:level": 2,
            "gfs:typecode": "MTSEFAM",
            "rdfs:comment": "Screw spindle pump for coolant and cutting oil with intergrated frquency converter",
            "skos:inScheme": "https://grundfos.com/concept/productFamily",
            "skos:prefLabel": "MTSE"
        },
        {
            "@id": "https://grundfos.com/concept/productFamily/SPKFAM",
            "@type": [
                "gfs:ProductFamily",
                "skos:Concept"
            ],
            "gfs:level": 2,
            "gfs:typecode": "SPKFAM",
            "rdfs:comment": "Vertical, multistage centrifugal pump for tank top mounting",
            "skos:inScheme": "https://grundfos.com/concept/productFamily",
            "skos:prefLabel": "SPK"
        },
        {
            "@id": "https://grundfos.com/concept/productFamily/MTRANGE",
            "@type": [
                "gfs:ProductFamily",
                "skos:Concept"
            ],
            "gfs:level": 1,
            "gfs:typecode": "MTRANGE",
            "rdfs:comment": "Vertical, multistage centrifugal and screw pumps, for mounting in tanks",
            "skos:inScheme": "https://grundfos.com/concept/productFamily",
            "skos:narrower": [
                "https://grundfos.com/concept/productFamily/CRKFAM",
                "https://grundfos.com/concept/productFamily/MTAFAM",
                "https://grundfos.com/concept/productFamily/MTDFAM",
                "https://grundfos.com/concept/productFamily/MTHFAM",
                "https://grundfos.com/concept/productFamily/MTRFAM",
                "https://grundfos.com/concept/productFamily/MTREFAM",
                "https://grundfos.com/concept/productFamily/MTSFAM",
                "https://grundfos.com/concept/productFamily/MTSEFAM",
                "https://grundfos.com/concept/productFamily/SPKFAM"
            ],
            "skos:prefLabel": "MT, tank mounted pumps"
        },
        {
            "@id": "https://grundfos.com/concept/productFamily/MTB000",
            "@type": [
                "gfs:ProductFamily",
                "skos:Concept"
            ],
            "gfs:level": 2,
            "gfs:typecode": "MTB000",
            "rdfs:comment": "Close coupled End Suction pump with semi-open Wortex impeller.",
            "skos:inScheme": "https://grundfos.com/concept/productFamily",
            "skos:prefLabel": "MTB"
        },
        {
            "@id": "https://grundfos.com/concept/productFamily/MTBE00",
            "@type": [
                "gfs:ProductFamily",
                "skos:Concept"
            ],
            "gfs:level": 2,
            "gfs:typecode": "MTBE00",
            "rdfs:comment": "Close coupled End Suction pump with semi-open Vortex impeller with MGE motor",
            "skos:inScheme": "https://grundfos.com/concept/productFamily",
            "skos:prefLabel": "MTBE"
        },
        {
            "@id": "https://grundfos.com/concept/productFamily/MTBFAM",
            "@type": [
                "gfs:ProductFamily",
                "skos:Concept"
            ],
            "gfs:level": 1,
            "gfs:typecode": "MTBFAM",
            "rdfs:comment": "Close coupled End Suction pump with semi-open Wortex impeller.",
            "skos:inScheme": "https://grundfos.com/concept/productFamily",
            "skos:narrower": [
                "https://grundfos.com/concept/productFamily/MTB000",
                "https://grundfos.com/concept/productFamily/MTBE00"
            ],
            "skos:prefLabel": "MTB, MTBE"
        },
        {
            "@id": "https://grundfos.com/concept/productFamily/MULDOUB",
            "@type": [
                "gfs:ProductFamily",
                "skos:Concept"
            ],
            "gfs:level": 2,
            "gfs:typecode": "MULDOUB",
            "rdfs:comment": "Lifting stations",
            "skos:inScheme": "https://grundfos.com/concept/productFamily",
            "skos:prefLabel": "Double pump units"
        },
        {
            "@id": "https://grundfos.com/concept/productFamily/MULSING",
            "@type": [
                "gfs:ProductFamily",
                "skos:Concept"
            ],
            "gfs:level": 2,
            "gfs:typecode": "MULSING",
            "rdfs:comment": "Lifting stations",
            "skos:inScheme": "https://grundfos.com/concept/productFamily",
            "skos:prefLabel": "Single pump units"
        },
        {
            "@id": "https://grundfos.com/concept/productFamily/LIFFAM",
            "@type": [
                "gfs:ProductFamily",
                "skos:Concept"
            ],
            "gfs:level": 1,
            "gfs:typecode": "LIFFAM",
            "rdfs:comment": "Lifting stations for collecting and removing wastewater of inside buildings",
            "skos:inScheme": "https://grundfos.com/concept/productFamily",
            "skos:narrower": [
                "https://grundfos.com/concept/productFamily/MULDOUB",
                "https://grundfos.com/concept/productFamily/MULSING"
            ],
            "skos:prefLabel": "Multilift"
        },
        {
            "@id": "https://grundfos.com/concept/productFamily/NB000",
            "@type": [
                "gfs:ProductFamily",
                "skos:Concept"
            ],
            "gfs:level": 2,
            "gfs:typecode": "NB000",
            "rdfs:comment": "End-suction close-coupled pumps according to EN 733",
            "skos:inScheme": "https://grundfos.com/concept/productFamily",
            "skos:prefLabel": "NB"
        },
        {
            "@id": "https://grundfos.com/concept/productFamily/NBE00",
            "@type": [
                "gfs:ProductFamily",
                "skos:Concept"
            ],
            "gfs:level": 2,
            "gfs:typecode": "NBE00",
            "rdfs:comment": "End-suction close-coupled pumps according to EN 733 with MGE motor",
            "skos:inScheme": "https://grundfos.com/concept/productFamily",
            "skos:prefLabel": "NBE"
        },
        {
            "@id": "https://grundfos.com/concept/productFamily/NBE0S2",
            "@type": [
                "gfs:ProductFamily",
                "skos:Concept"
            ],
            "gfs:level": 2,
            "gfs:typecode": "NBE0S2",
            "rdfs:comment": "End-suction close-coupled pumps according to EN 733 with MGE motor",
            "skos:inScheme": "https://grundfos.com/concept/productFamily",
            "skos:prefLabel": "NBE Series 2000"
        },
        {
            "@id": "https://grundfos.com/concept/productFamily/NBFAM",
            "@type": [
                "gfs:ProductFamily",
                "skos:Concept"
            ],
            "gfs:level": 1,
            "gfs:typecode": "NBFAM",
            "rdfs:comment": "End-suction close-coupled pumps according to EN 733",
            "skos:inScheme": "https://grundfos.com/concept/productFamily",
            "skos:narrower": [
                "https://grundfos.com/concept/productFamily/NB000",
                "https://grundfos.com/concept/productFamily/NBE00",
                "https://grundfos.com/concept/productFamily/NBE0S2"
            ],
            "skos:prefLabel": "NB, NBE, NBE Series 2000"
        },
        {
            "@id": "https://grundfos.com/concept/productFamily/NBG00",
            "@type": [
                "gfs:ProductFamily",
                "skos:Concept"
            ],
            "gfs:level": 2,
            "gfs:typecode": "NBG00",
            "rdfs:comment": "Close-coupled pumps according to ISO 2858",
            "skos:inScheme": "https://grundfos.com/concept/productFamily",
            "skos:prefLabel": "NBG"
        },
        {
            "@id": "https://grundfos.com/concept/productFamily/NBGE0",
            "@type": [
                "gfs:ProductFamily",
                "skos:Concept"
            ],
            "gfs:level": 2,
            "gfs:typecode": "NBGE0",
            "rdfs:comment": "Close-coupled pumps according to ISO 2858 with MGE motor",
            "skos:inScheme": "https://grundfos.com/concept/productFamily",
            "skos:prefLabel": "NBGE"
        },
        {
            "@id": "https://grundfos.com/concept/productFamily/NBGFAM",
            "@type": [
                "gfs:ProductFamily",
                "skos:Concept"
            ],
            "gfs:level": 1,
            "gfs:typecode": "NBGFAM",
            "rdfs:comment": "End-suction close-coupled pumps according to ISO 2858",
            "skos:inScheme": "https://grundfos.com/concept/productFamily",
            "skos:narrower": [
                "https://grundfos.com/concept/productFamily/NBG00",
                "https://grundfos.com/concept/productFamily/NBGE0"
            ],
            "skos:prefLabel": "NBG, NBGE"
        },
        {
            "@id": "https://grundfos.com/concept/productFamily/NKBASIS",
            "@type": [
                "gfs:ProductFamily",
                "skos:Concept"
            ],
            "gfs:level": 2,
            "gfs:typecode": "NKBASIS",
            "rdfs:comment": "Standard pumps according to EN 733",
            "skos:inScheme": "https://grundfos.com/concept/productFamily",
            "skos:prefLabel": "NK"
        },
        {
            "@id": "https://grundfos.com/concept/productFamily/NKBARE",
            "@type": [
                "gfs:ProductFamily",
                "skos:Concept"
            ],
            "gfs:level": 2,
            "gfs:typecode": "NKBARE",
            "rdfs:comment": "Bare shaft pumps according to EN 733",
            "skos:inScheme": "https://grundfos.com/concept/productFamily",
            "skos:prefLabel": "NK Bare shaft"
        },
        {
            "@id": "https://grundfos.com/concept/productFamily/NKEBASIS",
            "@type": [
                "gfs:ProductFamily",
                "skos:Concept"
            ],
            "gfs:level": 2,
            "gfs:typecode": "NKEBASIS",
            "rdfs:comment": "Standard pumps according to EN 733 with MGE motor",
            "skos:inScheme": "https://grundfos.com/concept/productFamily",
            "skos:prefLabel": "NKE"
        },
        {
            "@id": "https://grundfos.com/concept/productFamily/NKE0S2",
            "@type": [
                "gfs:ProductFamily",
                "skos:Concept"
            ],
            "gfs:level": 2,
            "gfs:typecode": "NKE0S2",
            "rdfs:comment": "Standard pumps according to EN 733 with MGE motor",
            "skos:inScheme": "https://grundfos.com/concept/productFamily",
            "skos:prefLabel": "NKE Series 2000"
        },
        {
            "@id": "https://grundfos.com/concept/productFamily/NKFAM",
            "@type": [
                "gfs:ProductFamily",
                "skos:Concept"
            ],
            "gfs:level": 1,
            "gfs:typecode": "NKFAM",
            "rdfs:comment": "End-suction long-coupled pumps according to EN 733",
            "skos:inScheme": "https://grundfos.com/concept/productFamily",
            "skos:narrower": [
                "https://grundfos.com/concept/productFamily/NKBASIS",
                "https://grundfos.com/concept/productFamily/NKBARE",
                "https://grundfos.com/concept/productFamily/NKEBASIS",
                "https://grundfos.com/concept/productFamily/NKE0S2"
            ],
            "skos:prefLabel": "NK, NKE, NKE Series 2000, NK Bare shaft"
        },
        {
            "@id": "https://grundfos.com/concept/productFamily/NKG00",
            "@type": [
                "gfs:ProductFamily",
                "skos:Concept"
            ],
            "gfs:level": 2,
            "gfs:typecode": "NKG00",
            "rdfs:comment": "Standard pumps according to ISO 2858",
            "skos:inScheme": "https://grundfos.com/concept/productFamily",
            "skos:prefLabel": "NKG"
        },
        {
            "@id": "https://grundfos.com/concept/productFamily/NKGBARE",
            "@type": [
                "gfs:ProductFamily",
                "skos:Concept"
            ],
            "gfs:level": 2,
            "gfs:typecode": "NKGBARE",
            "rdfs:comment": "Bare shaft pumps according to ISO 2858",
            "skos:inScheme": "https://grundfos.com/concept/productFamily",
            "skos:prefLabel": "NKG Bare shaft"
        },
        {
            "@id": "https://grundfos.com/concept/productFamily/NKGE0",
            "@type": [
                "gfs:ProductFamily",
                "skos:Concept"
            ],
            "gfs:level": 2,
            "gfs:typecode": "NKGE0",
            "rdfs:comment": "Standard pumps according to ISO 2858 with MGE motor",
            "skos:inScheme": "https://grundfos.com/concept/productFamily",
            "skos:prefLabel": "NKGE"
        },
        {
            "@id": "https://grundfos.com/concept/productFamily/NKGFAM",
            "@type": [
                "gfs:ProductFamily",
                "skos:Concept"
            ],
            "gfs:level": 1,
            "gfs:typecode": "NKGFAM",
            "rdfs:comment": "End-suction long-coupled pumps according to ISO 2858",
            "skos:inScheme": "https://grundfos.com/concept/productFamily",
            "skos:narrower": [
                "https://grundfos.com/concept/productFamily/NKG00",
                "https://grundfos.com/concept/productFamily/NKGBARE",
                "https://grundfos.com/concept/productFamily/NKGE0"
            ],
            "skos:prefLabel": "NKG, NKGE, NKG Bare shaft"
        },
        {
            "@id": "https://grundfos.com/concept/productFamily/NSFAM",
            "@type": [
                "gfs:ProductFamily",
                "skos:Concept"
            ],
            "gfs:level": 1,
            "gfs:typecode": "NSFAM",
            "rdfs:comment": "Grundfos NS pumps are centrifugal pumps designed for lifting water in domestic, industrial and agricultural installations. Available in two versions: Single-impeller pumps and twin-impeller pumps.",
            "skos:inScheme": "https://grundfos.com/concept/productFamily",
            "skos:narrower": [],
            "skos:prefLabel": "NS"
        },
        {
            "@id": "https://grundfos.com/concept/productFamily/SERCOMMI",
            "@type": [
                "gfs:ProductFamily",
                "skos:Concept"
            ],
            "gfs:level": 2,
            "gfs:typecode": "SERCOMMI",
            "rdfs:comment": "Maximise the performance and efficiency of your pump system with advanced commissioning services from industry experts.",
            "skos:inScheme": "https://grundfos.com/concept/productFamily",
            "skos:prefLabel": "Commissioning"
        },
        {
            "@id": "https://grundfos.com/concept/productFamily/INSPECT",
            "@type": [
                "gfs:ProductFamily",
                "skos:Concept"
            ],
            "gfs:level": 2,
            "gfs:typecode": "INSPECT",
            "rdfs:comment": "Minimise costs and ensure lifelong pump efficiency. An inspection gives you an overview of installed base conditions and recommendations for improvements.",
            "skos:inScheme": "https://grundfos.com/concept/productFamily",
            "skos:prefLabel": "Inspection"
        },
        {
            "@id": "https://grundfos.com/concept/productFamily/OPERINST",
            "@type": [
                "gfs:ProductFamily",
                "skos:Concept"
            ],
            "gfs:level": 2,
            "gfs:typecode": "OPERINST",
            "rdfs:comment": "Outsource installation tasks to Grundfos personnel to know that your pumps are in capable hands.",
            "skos:inScheme": "https://grundfos.com/concept/productFamily",
            "skos:prefLabel": "Installation"
        },
        {
            "@id": "https://grundfos.com/concept/productFamily/SERLAALI",
            "@type": [
                "gfs:ProductFamily",
                "skos:Concept"
            ],
            "gfs:level": 2,
            "gfs:typecode": "SERLAALI",
            "rdfs:comment": "Optimise efficiency and reliability and reduce energy consumption and operating costs with our pump laser alignment service.",
            "skos:inScheme": "https://grundfos.com/concept/productFamily",
            "skos:prefLabel": "Laser Alignment"
        },
        {
            "@id": "https://grundfos.com/concept/productFamily/OPERTHER",
            "@type": [
                "gfs:ProductFamily",
                "skos:Concept"
            ],
            "gfs:level": 2,
            "gfs:typecode": "OPERTHER",
            "rdfs:comment": "A Grundfos thermal scan helps you detect hazards in your control panel and thereby prevent accidents and avoid downtime.",
            "skos:inScheme": "https://grundfos.com/concept/productFamily",
            "skos:prefLabel": "Thermal scan"
        },
        {
            "@id": "https://grundfos.com/concept/productFamily/OPERVIBR",
            "@type": [
                "gfs:ProductFamily",
                "skos:Concept"
            ],
            "gfs:level": 2,
            "gfs:typecode": "OPERVIBR",
            "rdfs:comment": "Staying in the know about equipment status allows you to take the necessary measures to prevent expensive downtime.",
            "skos:inScheme": "https://grundfos.com/concept/productFamily",
            "skos:prefLabel": "Vibration measurement"
        },
        {
            "@id": "https://grundfos.com/concept/productFamily/OPERSERV",
            "@type": [
                "gfs:ProductFamily",
                "skos:Concept"
            ],
            "gfs:level": 1,
            "gfs:typecode": "OPERSERV",
            "rdfs:comment": "Keep your system running smoothly with our wide range of pump operation service offerings. We maximise the performance and efficiency of your system, allowing you all the time you need to focus on your business. And, we make sure you get the best performance out of every pump and pump system.",
            "skos:inScheme": "https://grundfos.com/concept/productFamily",
            "skos:narrower": [
                "https://grundfos.com/concept/productFamily/SERCOMMI",
                "https://grundfos.com/concept/productFamily/INSPECT",
                "https://grundfos.com/concept/productFamily/OPERINST",
                "https://grundfos.com/concept/productFamily/SERLAALI",
                "https://grundfos.com/concept/productFamily/OPERTHER",
                "https://grundfos.com/concept/productFamily/OPERVIBR"
            ],
            "skos:prefLabel": "Operation services"
        },
        {
            "@id": "https://grundfos.com/concept/productFamily/PUMPAUD",
            "@type": [
                "gfs:ProductFamily",
                "skos:Concept"
            ],
            "gfs:level": 2,
            "gfs:typecode": "PUMPAUD",
            "rdfs:comment": "A detailed, measurement-based analysis of your current pump performance with suggestions for future energy savings and improved performance.",
            "skos:inScheme": "https://grundfos.com/concept/productFamily",
            "skos:prefLabel": "Energy audit"
        },
        {
            "@id": "https://grundfos.com/concept/productFamily/SERECHCK",
            "@type": [
                "gfs:ProductFamily",
                "skos:Concept"
            ],
            "gfs:level": 2,
            "gfs:typecode": "SERECHCK",
            "rdfs:comment": "A free, non-binding analysis of your current pump performance that will help you find potential energy savings in your pumps.",
            "skos:inScheme": "https://grundfos.com/concept/productFamily",
            "skos:prefLabel": "Energy check"
        },
        {
            "@id": "https://grundfos.com/concept/productFamily/SEROPTC",
            "@type": [
                "gfs:ProductFamily",
                "skos:Concept"
            ],
            "gfs:level": 1,
            "gfs:typecode": "SEROPTC",
            "rdfs:comment": "Pumps help run the air-conditioning systems that keep us cool and ensure warm water in showers. But they can also waste enormous amounts of energy. And with 85 % of the total life-cycle cost of a pump spent on energy usage, ensuring pump efficiency makes good sense. Grundfos can help you reduce energy consumption, improve pump efficiency and find the hidden savings in your pumps.",
            "skos:inScheme": "https://grundfos.com/concept/productFamily",
            "skos:narrower": [
                "https://grundfos.com/concept/productFamily/PUMPAUD",
                "https://grundfos.com/concept/productFamily/SERECHCK"
            ],
            "skos:prefLabel": "Optimisation services"
        },
        {
            "@id": "https://grundfos.com/concept/productFamily/OTHMOT",
            "@type": [
                "gfs:ProductFamily",
                "skos:Concept"
            ],
            "gfs:level": 1,
            "gfs:typecode": "OTHMOT",
            "rdfs:comment": "Standard motors",
            "skos:inScheme": "https://grundfos.com/concept/productFamily",
            "skos:narrower": [],
            "skos:prefLabel": "Other standard motor"
        },
        {
            "@id": "https://grundfos.com/concept/productFamily/FRANKLIN",
            "@type": [
                "gfs:ProductFamily",
                "skos:Concept"
            ],
            "gfs:level": 2,
            "gfs:typecode": "FRANKLIN",
            "rdfs:comment": "Submersible motors",
            "skos:inScheme": "https://grundfos.com/concept/productFamily",
            "skos:prefLabel": "Franklin"
        },
        {
            "@id": "https://grundfos.com/concept/productFamily/OTHSMOT",
            "@type": [
                "gfs:ProductFamily",
                "skos:Concept"
            ],
            "gfs:level": 1,
            "gfs:typecode": "OTHSMOT",
            "rdfs:comment": "Submersible motors",
            "skos:inScheme": "https://grundfos.com/concept/productFamily",
            "skos:narrower": [
                "https://grundfos.com/concept/productFamily/FRANKLIN"
            ],
            "skos:prefLabel": "Other submersible motors"
        },
        {
            "@id": "https://grundfos.com/concept/productFamily/PF000",
            "@type": [
                "gfs:ProductFamily",
                "skos:Concept"
            ],
            "gfs:level": 1,
            "gfs:typecode": "PF000",
            "rdfs:comment": "Grundfos PF pumps are compact, peripheral pumps. PF can generate high heads suitable for applications such as water supply, light gardening, and light industrial applications.",
            "skos:inScheme": "https://grundfos.com/concept/productFamily",
            "skos:narrower": [],
            "skos:prefLabel": "PF"
        },
        {
            "@id": "https://grundfos.com/concept/productFamily/POMONA",
            "@type": [
                "gfs:ProductFamily",
                "skos:Concept"
            ],
            "gfs:level": 1,
            "gfs:typecode": "POMONA",
            "rdfs:comment": "Self priming drainage pump. Either with an electric motor or combustion engine. Special hydraulics for wear-resistance",
            "skos:inScheme": "https://grundfos.com/concept/productFamily",
            "skos:narrower": [],
            "skos:prefLabel": "POMONA"
        },
        {
            "@id": "https://grundfos.com/concept/productFamily/MOBDOS",
            "@type": [
                "gfs:ProductFamily",
                "skos:Concept"
            ],
            "gfs:level": 2,
            "gfs:typecode": "MOBDOS",
            "rdfs:comment": "Transportable dosing station for use with standard canisters",
            "skos:inScheme": "https://grundfos.com/concept/productFamily",
            "skos:prefLabel": "Mobile Dos"
        },
        {
            "@id": "https://grundfos.com/concept/productFamily/POLYDOS",
            "@type": [
                "gfs:ProductFamily",
                "skos:Concept"
            ],
            "gfs:level": 2,
            "gfs:typecode": "POLYDOS",
            "rdfs:comment": "Full automatic system for preparation of solutions from dry or concentrated liquid polymers",
            "skos:inScheme": "https://grundfos.com/concept/productFamily",
            "skos:prefLabel": "Polydos"
        },
        {
            "@id": "https://grundfos.com/concept/productFamily/DOSSYFAM",
            "@type": [
                "gfs:ProductFamily",
                "skos:Concept"
            ],
            "gfs:level": 1,
            "gfs:typecode": "DOSSYFAM",
            "rdfs:comment": "Complete dosing systems and installation sets",
            "skos:inScheme": "https://grundfos.com/concept/productFamily",
            "skos:narrower": [
                "https://grundfos.com/concept/productFamily/MOBDOS",
                "https://grundfos.com/concept/productFamily/POLYDOS"
            ],
            "skos:prefLabel": "Preparation and Dosing Systems"
        },
        {
            "@id": "https://grundfos.com/concept/productFamily/PM1",
            "@type": [
                "gfs:ProductFamily",
                "skos:Concept"
            ],
            "gfs:level": 2,
            "gfs:typecode": "PM1",
            "rdfs:comment": "Grundfos pressure managers PM 1 are designed for automatic start/stop control for Grundfos pumps and third-party water supply pumps.",
            "skos:inScheme": "https://grundfos.com/concept/productFamily",
            "skos:prefLabel": "PM 1"
        },
        {
            "@id": "https://grundfos.com/concept/productFamily/PM2",
            "@type": [
                "gfs:ProductFamily",
                "skos:Concept"
            ],
            "gfs:level": 2,
            "gfs:typecode": "PM2",
            "rdfs:comment": "Grundfos pressure managers PM 2 are designed for automatic start/stop control for Grundfos pumps and third-party water supply pumps.",
            "skos:inScheme": "https://grundfos.com/concept/productFamily",
            "skos:prefLabel": "PM 2"
        },
        {
            "@id": "https://grundfos.com/concept/productFamily/PMRFAM",
            "@type": [
                "gfs:ProductFamily",
                "skos:Concept"
            ],
            "gfs:level": 2,
            "gfs:typecode": "PMRFAM",
            "rdfs:comment": "Grundfos Pressure Manager Rain is an interconnect device that allows you to utilise harvested rainwater, with the added benefit of mains water back-up.",
            "skos:inScheme": "https://grundfos.com/concept/productFamily",
            "skos:prefLabel": "PM Rain"
        },
        {
            "@id": "https://grundfos.com/concept/productFamily/PMTWIN",
            "@type": [
                "gfs:ProductFamily",
                "skos:Concept"
            ],
            "gfs:level": 2,
            "gfs:typecode": "PMTWIN",
            "rdfs:comment": "All-in one Grundfos Pressure Manager Twin is an intelligent waterworks that controls two pump solutions with Duty/Standby Mode in accordance with consumption in domestic water supply",
            "skos:inScheme": "https://grundfos.com/concept/productFamily",
            "skos:prefLabel": "PM Twin"
        },
        {
            "@id": "https://grundfos.com/concept/productFamily/PRESSMAN",
            "@type": [
                "gfs:ProductFamily",
                "skos:Concept"
            ],
            "gfs:level": 1,
            "gfs:typecode": "PRESSMAN",
            "rdfs:comment": "The Pressure Managers are intelligent waterworks that control your pump in accordance with consumption in domestic water supply and booster systems.",
            "skos:inScheme": "https://grundfos.com/concept/productFamily",
            "skos:narrower": [
                "https://grundfos.com/concept/productFamily/PM1",
                "https://grundfos.com/concept/productFamily/PM2",
                "https://grundfos.com/concept/productFamily/PMRFAM",
                "https://grundfos.com/concept/productFamily/PMTWIN"
            ],
            "skos:prefLabel": "Pressure Manager"
        },
        {
            "@id": "https://grundfos.com/concept/productFamily/GTC",
            "@type": [
                "gfs:ProductFamily",
                "skos:Concept"
            ],
            "gfs:level": 2,
            "gfs:typecode": "GTC",
            "rdfs:comment": "The GT-C tanks are lightweight composite pressure tanks. The diaphragm is a chlorine-resistant 100 % butyl diaphragm with a precision-moulded copolymer polypropylene liner for superior air and water separation. Also available as FlowThru variant. Recommend application: Sea water and Drinking water.",
            "skos:inScheme": "https://grundfos.com/concept/productFamily",
            "skos:prefLabel": "GT-C"
        },
        {
            "@id": "https://grundfos.com/concept/productFamily/GTD",
            "@type": [
                "gfs:ProductFamily",
                "skos:Concept"
            ],
            "gfs:level": 2,
            "gfs:typecode": "GTD",
            "rdfs:comment": "The GT-D tanks are steel pressure tanks with double diaphragm. The diaphragm is a chlorine-resistant 100 % butyl diaphragm with a precision-moulded copolymer polypropylene liner for superior air and water separation. Also available as FlowThru variant. Recommend application: Drinking water.",
            "skos:inScheme": "https://grundfos.com/concept/productFamily",
            "skos:prefLabel": "GT-D"
        },
        {
            "@id": "https://grundfos.com/concept/productFamily/GTH",
            "@type": [
                "gfs:ProductFamily",
                "skos:Concept"
            ],
            "gfs:level": 2,
            "gfs:typecode": "GTH",
            "rdfs:comment": "The GT-H tanks are steel pressure tanks with a non-toxic butyl rubber diaphragm with a precision-moulded polypropylene liner for superior air and water separation. Recommend application: Drinking water.",
            "skos:inScheme": "https://grundfos.com/concept/productFamily",
            "skos:prefLabel": "GT-H"
        },
        {
            "@id": "https://grundfos.com/concept/productFamily/GTHR",
            "@type": [
                "gfs:ProductFamily",
                "skos:Concept"
            ],
            "gfs:level": 2,
            "gfs:typecode": "GTHR",
            "rdfs:comment": "The GT-HR tanks are steel pressure tank with a non-replaceable rubber diaphragm, pre-charged with nitrogen. Recommend application: Heating water.",
            "skos:inScheme": "https://grundfos.com/concept/productFamily",
            "skos:prefLabel": "GT-HR"
        },
        {
            "@id": "https://grundfos.com/concept/productFamily/GTU",
            "@type": [
                "gfs:ProductFamily",
                "skos:Concept"
            ],
            "gfs:level": 2,
            "gfs:typecode": "GTU",
            "rdfs:comment": "The GT-U tanks are steel pressure tanks with a replaceable, non-toxic butyl rubber bladder enclosed by compressed nitrogen. Recommend application: Grey water and Drinking water.",
            "skos:inScheme": "https://grundfos.com/concept/productFamily",
            "skos:prefLabel": "GT-U"
        },
        {
            "@id": "https://grundfos.com/concept/productFamily/GTUPLUS",
            "@type": [
                "gfs:ProductFamily",
                "skos:Concept"
            ],
            "gfs:level": 2,
            "gfs:typecode": "GTUPLUS",
            "rdfs:comment": "The GT-U+ tanks are steel pressure tanks with a replaceable, non-toxic butyl rubber bladder enclosed by compressed nitrogen, equipped with a Manometer and a connection for a pressure switch. Recommend application: Heating, Chilled water, Grey water and Drinking water.",
            "skos:inScheme": "https://grundfos.com/concept/productFamily",
            "skos:prefLabel": "GT-U+"
        },
        {
            "@id": "https://grundfos.com/concept/productFamily/TANK",
            "@type": [
                "gfs:ProductFamily",
                "skos:Concept"
            ],
            "gfs:level": 1,
            "gfs:typecode": "TANK",
            "rdfs:comment": "GT pressure tanks are long-life tanks suited for domestic, commercial and industrial applications in cold-water and heating systems.",
            "skos:inScheme": "https://grundfos.com/concept/productFamily",
            "skos:narrower": [
                "https://grundfos.com/concept/productFamily/GTC",
                "https://grundfos.com/concept/productFamily/GTD",
                "https://grundfos.com/concept/productFamily/GTH",
                "https://grundfos.com/concept/productFamily/GTHR",
                "https://grundfos.com/concept/productFamily/GTU",
                "https://grundfos.com/concept/productFamily/GTUPLUS"
            ],
            "skos:prefLabel": "Pressure tanks"
        },
        {
            "@id": "https://grundfos.com/concept/productFamily/PSG00",
            "@type": [
                "gfs:ProductFamily",
                "skos:Concept"
            ],
            "gfs:level": 2,
            "gfs:typecode": "PSG00",
            "rdfs:comment": "The PS.G is a range of prefabricated pumping stations molded in glass-fibre-reinforced polyester. This range is available with a sump diameter from 1200mm to 3000m, with a depth of up to 8m. On request up to 12m. The PS.G range can be equipped with wastewater pumps up to 85kW as standard.",
            "skos:inScheme": "https://grundfos.com/concept/productFamily",
            "skos:prefLabel": "PS.G"
        },
        {
            "@id": "https://grundfos.com/concept/productFamily/PSR00",
            "@type": [
                "gfs:ProductFamily",
                "skos:Concept"
            ],
            "gfs:level": 2,
            "gfs:typecode": "PSR00",
            "rdfs:comment": "The PS.R is a rotation molded range of prefabricated pumping stations in polyethylene. This range is available with a sump diameter from 500mm to 1700mm, with a depth of up to 6m. The PS.R range can be equipped with wastewater pumps up to 7,5kW.",
            "skos:inScheme": "https://grundfos.com/concept/productFamily",
            "skos:prefLabel": "PS.R"
        },
        {
            "@id": "https://grundfos.com/concept/productFamily/PSW00",
            "@type": [
                "gfs:ProductFamily",
                "skos:Concept"
            ],
            "gfs:level": 2,
            "gfs:typecode": "PSW00",
            "rdfs:comment": "The PS.W is a welded range of prefabricated pumping stations in either polyethylene or polypropylene. This range is an extension of the PS.R range with a sump diameter from 400mm to 2000mm, with a depth up to 6m. The PS.W range can be equipped with wastewater pumps up to 11kW.",
            "skos:inScheme": "https://grundfos.com/concept/productFamily",
            "skos:prefLabel": "PS.W"
        },
        {
            "@id": "https://grundfos.com/concept/productFamily/PS",
            "@type": [
                "gfs:ProductFamily",
                "skos:Concept"
            ],
            "gfs:level": 1,
            "gfs:typecode": "PS",
            "rdfs:comment": "Grundfos pumping stations are prefabricated pumping stations designed for collection and pumping of drainage water, rainwater or wastewater. The products available here only represent a fraction of our selection. Use the \"Pumping Station Creator\" found in Tools to size and configure a system fitting your requirements.",
            "skos:inScheme": "https://grundfos.com/concept/productFamily",
            "skos:narrower": [
                "https://grundfos.com/concept/productFamily/PSG00",
                "https://grundfos.com/concept/productFamily/PSR00",
                "https://grundfos.com/concept/productFamily/PSW00"
            ],
            "skos:prefLabel": "Pumping Stations"
        },
        {
            "@id": "https://grundfos.com/concept/productFamily/RCMEFAM",
            "@type": [
                "gfs:ProductFamily",
                "skos:Concept"
            ],
            "gfs:level": 1,
            "gfs:typecode": "RCMEFAM",
            "rdfs:comment": "The Grundfos rainwater pumping system is designed for the monitoring and control of rainwater utilisation systems",
            "skos:inScheme": "https://grundfos.com/concept/productFamily",
            "skos:narrower": [],
            "skos:prefLabel": "RCME"
        },
        {
            "@id": "https://grundfos.com/concept/productFamily/SEROSREP",
            "@type": [
                "gfs:ProductFamily",
                "skos:Concept"
            ],
            "gfs:level": 2,
            "gfs:typecode": "SEROSREP",
            "rdfs:comment": "Complete workshop repair services for all pump repair needs including delivery options",
            "skos:inScheme": "https://grundfos.com/concept/productFamily",
            "skos:prefLabel": "Onsite & Workshop Repair"
        },
        {
            "@id": "https://grundfos.com/concept/productFamily/REPLACE",
            "@type": [
                "gfs:ProductFamily",
                "skos:Concept"
            ],
            "gfs:level": 2,
            "gfs:typecode": "REPLACE",
            "rdfs:comment": "Find the pumps you need and build a business case for upgrading to pumps with some of the lowest power consumption available.",
            "skos:inScheme": "https://grundfos.com/concept/productFamily",
            "skos:prefLabel": "Replacement"
        },
        {
            "@id": "https://grundfos.com/concept/productFamily/SERVKITS",
            "@type": [
                "gfs:ProductFamily",
                "skos:Concept"
            ],
            "gfs:level": 2,
            "gfs:typecode": "SERVKITS",
            "rdfs:comment": "Get quick and easy access to the most commonly used spare parts for standard Grundfos pumps and systems.",
            "skos:inScheme": "https://grundfos.com/concept/productFamily",
            "skos:prefLabel": "Service kits"
        },
        {
            "@id": "https://grundfos.com/concept/productFamily/SPAREPAR",
            "@type": [
                "gfs:ProductFamily",
                "skos:Concept"
            ],
            "gfs:level": 2,
            "gfs:typecode": "SPAREPAR",
            "rdfs:comment": "Grundfos spare parts are high-quality components that enable you to optimise system performance and minimise downtime due to unforeseen breakdowns. Grundfos pump parts can be delivered as single parts or in bulk depending on your needs.",
            "skos:inScheme": "https://grundfos.com/concept/productFamily",
            "skos:prefLabel": "Spare parts"
        },
        {
            "@id": "https://grundfos.com/concept/productFamily/SERWSREP",
            "@type": [
                "gfs:ProductFamily",
                "skos:Concept"
            ],
            "gfs:level": 2,
            "gfs:typecode": "SERWSREP",
            "rdfs:comment": "Complete workshop repair services for all pump repair needs including delivery options",
            "skos:inScheme": "https://grundfos.com/concept/productFamily",
            "skos:prefLabel": "Workshop Repair"
        },
        {
            "@id": "https://grundfos.com/concept/productFamily/SERREPM",
            "@type": [
                "gfs:ProductFamily",
                "skos:Concept"
            ],
            "gfs:level": 1,
            "gfs:typecode": "SERREPM",
            "rdfs:comment": "Keep your system up and running with our wide range of pump repair services. Our team of highly skilled service technicians can resolve any kind of pump problem, while ensuring that you get the maximum performance from every pump and pump system.",
            "skos:inScheme": "https://grundfos.com/concept/productFamily",
            "skos:narrower": [
                "https://grundfos.com/concept/productFamily/SEROSREP",
                "https://grundfos.com/concept/productFamily/REPLACE",
                "https://grundfos.com/concept/productFamily/SERVKITS",
                "https://grundfos.com/concept/productFamily/SPAREPAR",
                "https://grundfos.com/concept/productFamily/SERWSREP"
            ],
            "skos:prefLabel": "Repair services"
        },
        {
            "@id": "https://grundfos.com/concept/productFamily/RMQFAM",
            "@type": [
                "gfs:ProductFamily",
                "skos:Concept"
            ],
            "gfs:level": 1,
            "gfs:typecode": "RMQFAM",
            "rdfs:comment": "Grundfos RMQ are rainwater units designed for monitoring and control of rainwater systems according to EN 1717.",
            "skos:inScheme": "https://grundfos.com/concept/productFamily",
            "skos:narrower": [],
            "skos:prefLabel": "RMQ"
        },
        {
            "@id": "https://grundfos.com/concept/productFamily/RSIFAM",
            "@type": [
                "gfs:ProductFamily",
                "skos:Concept"
            ],
            "gfs:level": 1,
            "gfs:typecode": "RSIFAM",
            "rdfs:comment": "Renewable Solar Inverter is an off-grid solar inverter to expand the solar pumping systems family. RSI work with submersible, multistage and singlestage pumps",
            "skos:inScheme": "https://grundfos.com/concept/productFamily",
            "skos:narrower": [],
            "skos:prefLabel": "RSI"
        },
        {
            "@id": "https://grundfos.com/concept/productFamily/SRANGE50",
            "@type": [
                "gfs:ProductFamily",
                "skos:Concept"
            ],
            "gfs:level": 2,
            "gfs:typecode": "SRANGE50",
            "rdfs:comment": "The S pumps are a range of free-flow channel impeller pumps specifically designed for pumping sewage and wastewater in a wide range of municipal and industrial applications",
            "skos:inScheme": "https://grundfos.com/concept/productFamily",
            "skos:prefLabel": "Range 50 => 13 kW"
        },
        {
            "@id": "https://grundfos.com/concept/productFamily/SRANGE54",
            "@type": [
                "gfs:ProductFamily",
                "skos:Concept"
            ],
            "gfs:level": 2,
            "gfs:typecode": "SRANGE54",
            "rdfs:comment": "The S pumps are a range of free-flow channel impeller pumps specifically designed for pumping sewage and wastewater in a wide range of municipal and industrial applications",
            "skos:inScheme": "https://grundfos.com/concept/productFamily",
            "skos:prefLabel": "Range 54 => 21 kW"
        },
        {
            "@id": "https://grundfos.com/concept/productFamily/SRANGE58",
            "@type": [
                "gfs:ProductFamily",
                "skos:Concept"
            ],
            "gfs:level": 2,
            "gfs:typecode": "SRANGE58",
            "rdfs:comment": "The S pumps are a range of free-flow channel impeller pumps specifically designed for pumping sewage and wastewater in a wide range of municipal and industrial applications",
            "skos:inScheme": "https://grundfos.com/concept/productFamily",
            "skos:prefLabel": "Range 58 => 29 kW"
        },
        {
            "@id": "https://grundfos.com/concept/productFamily/SRANGE62",
            "@type": [
                "gfs:ProductFamily",
                "skos:Concept"
            ],
            "gfs:level": 2,
            "gfs:typecode": "SRANGE62",
            "rdfs:comment": "The S pumps are a range of free-flow channel impeller pumps specifically designed for pumping sewage and wastewater in a wide range of municipal and industrial applications",
            "skos:inScheme": "https://grundfos.com/concept/productFamily",
            "skos:prefLabel": "Range 62 => 50 kW"
        },
        {
            "@id": "https://grundfos.com/concept/productFamily/SRANGE66",
            "@type": [
                "gfs:ProductFamily",
                "skos:Concept"
            ],
            "gfs:level": 2,
            "gfs:typecode": "SRANGE66",
            "rdfs:comment": "The S pumps are a range of free-flow channel impeller pumps specifically designed for pumping sewage and wastewater in a wide range of municipal and industrial applications",
            "skos:inScheme": "https://grundfos.com/concept/productFamily",
            "skos:prefLabel": "Range 66 => 68 kW"
        },
        {
            "@id": "https://grundfos.com/concept/productFamily/SRANGE70",
            "@type": [
                "gfs:ProductFamily",
                "skos:Concept"
            ],
            "gfs:level": 2,
            "gfs:typecode": "SRANGE70",
            "rdfs:comment": "The S pumps are a range of free-flow channel impeller pumps specifically designed for pumping sewage and wastewater in a wide range of municipal and industrial applications",
            "skos:inScheme": "https://grundfos.com/concept/productFamily",
            "skos:prefLabel": "Range 70 => 155 kW"
        },
        {
            "@id": "https://grundfos.com/concept/productFamily/SRANGE72",
            "@type": [
                "gfs:ProductFamily",
                "skos:Concept"
            ],
            "gfs:level": 2,
            "gfs:typecode": "SRANGE72",
            "rdfs:comment": "The S pumps are a range of free-flow channel impeller pumps specifically designed for pumping sewage and wastewater in a wide range of municipal and industrial applications",
            "skos:inScheme": "https://grundfos.com/concept/productFamily",
            "skos:prefLabel": "Range 72 => 225 kW"
        },
        {
            "@id": "https://grundfos.com/concept/productFamily/SRANGE74",
            "@type": [
                "gfs:ProductFamily",
                "skos:Concept"
            ],
            "gfs:level": 2,
            "gfs:typecode": "SRANGE74",
            "rdfs:comment": "The S pumps are a range of free-flow channel impeller pumps specifically designed for pumping sewage and wastewater in a wide range of municipal and industrial applications",
            "skos:inScheme": "https://grundfos.com/concept/productFamily",
            "skos:prefLabel": "Range 74 => 315 kW"
        },
        {
            "@id": "https://grundfos.com/concept/productFamily/SRANGE78",
            "@type": [
                "gfs:ProductFamily",
                "skos:Concept"
            ],
            "gfs:level": 2,
            "gfs:typecode": "SRANGE78",
            "rdfs:comment": "The S pumps are a range of free-flow channel impeller pumps specifically designed for pumping sewage and wastewater in a wide range of municipal and industrial applications",
            "skos:inScheme": "https://grundfos.com/concept/productFamily",
            "skos:prefLabel": "Range 78 => 520 kW"
        },
        {
            "@id": "https://grundfos.com/concept/productFamily/SFAM",
            "@type": [
                "gfs:ProductFamily",
                "skos:Concept"
            ],
            "gfs:level": 1,
            "gfs:typecode": "SFAM",
            "rdfs:comment": "The S pumps are a range of free-flow channel impeller pumps specifically designed for pumping sewage and wastewater in a wide range of municipal and industrial applications",
            "skos:inScheme": "https://grundfos.com/concept/productFamily",
            "skos:narrower": [
                "https://grundfos.com/concept/productFamily/SRANGE50",
                "https://grundfos.com/concept/productFamily/SRANGE54",
                "https://grundfos.com/concept/productFamily/SRANGE58",
                "https://grundfos.com/concept/productFamily/SRANGE62",
                "https://grundfos.com/concept/productFamily/SRANGE66",
                "https://grundfos.com/concept/productFamily/SRANGE70",
                "https://grundfos.com/concept/productFamily/SRANGE72",
                "https://grundfos.com/concept/productFamily/SRANGE74",
                "https://grundfos.com/concept/productFamily/SRANGE78"
            ],
            "skos:prefLabel": "S"
        },
        {
            "@id": "https://grundfos.com/concept/productFamily/SB000",
            "@type": [
                "gfs:ProductFamily",
                "skos:Concept"
            ],
            "gfs:level": 2,
            "gfs:typecode": "SB000",
            "rdfs:comment": "Grundfos SB pumps are submersible multistage pumps, designed to pump clean water for domestic tanks, shallow wells, and rainwater applications.",
            "skos:inScheme": "https://grundfos.com/concept/productFamily",
            "skos:prefLabel": "SB"
        },
        {
            "@id": "https://grundfos.com/concept/productFamily/SBHF0",
            "@type": [
                "gfs:ProductFamily",
                "skos:Concept"
            ],
            "gfs:level": 2,
            "gfs:typecode": "SBHF0",
            "rdfs:comment": "Grundfos SB HF pumps are stainless steel submersible multistage pumps, designed to pump clean water for domestic tanks, shallow wells, and rainwater applications.",
            "skos:inScheme": "https://grundfos.com/concept/productFamily",
            "skos:prefLabel": "SB HF"
        },
        {
            "@id": "https://grundfos.com/concept/productFamily/SBA00",
            "@type": [
                "gfs:ProductFamily",
                "skos:Concept"
            ],
            "gfs:level": 2,
            "gfs:typecode": "SBA00",
            "rdfs:comment": "Grundfos SBA submersible multistage boosters are complete all-in-one units, designed to pump clean water for break tanks, shallow wells, and rainwater applications. They come with an integrated control unit eliminating the need for an external pump controller.",
            "skos:inScheme": "https://grundfos.com/concept/productFamily",
            "skos:prefLabel": "SBA"
        },
        {
            "@id": "https://grundfos.com/concept/productFamily/SBFAM",
            "@type": [
                "gfs:ProductFamily",
                "skos:Concept"
            ],
            "gfs:level": 1,
            "gfs:typecode": "SBFAM",
            "rdfs:comment": "Submersible 5 inch pump for a wide range of domestic applications",
            "skos:inScheme": "https://grundfos.com/concept/productFamily",
            "skos:narrower": [
                "https://grundfos.com/concept/productFamily/SB000",
                "https://grundfos.com/concept/productFamily/SBHF0",
                "https://grundfos.com/concept/productFamily/SBA00"
            ],
            "skos:prefLabel": "SB, SBA"
        },
        {
            "@id": "https://grundfos.com/concept/productFamily/SCALAACC",
            "@type": [
                "gfs:ProductFamily",
                "skos:Concept"
            ],
            "gfs:level": 2,
            "gfs:typecode": "SCALAACC",
            "rdfs:comment": "Accessories",
            "skos:inScheme": "https://grundfos.com/concept/productFamily",
            "skos:prefLabel": "Accessories, SCALA"
        },
        {
            "@id": "https://grundfos.com/concept/productFamily/SCALA2",
            "@type": [
                "gfs:ProductFamily",
                "skos:Concept"
            ],
            "gfs:level": 2,
            "gfs:typecode": "SCALA2",
            "rdfs:comment": "The Grundfos SCALA2 is a fully integrated, self-priming, compact waterworks for pressure boosting in domestic applications, such as one and two-family houses and apartments. SCALA2 incorporates integrated speed control which allows maintaining a perfect pressure in the taps.",
            "skos:inScheme": "https://grundfos.com/concept/productFamily",
            "skos:prefLabel": "SCALA2"
        },
        {
            "@id": "https://grundfos.com/concept/productFamily/SCALA",
            "@type": [
                "gfs:ProductFamily",
                "skos:Concept"
            ],
            "gfs:level": 1,
            "gfs:typecode": "SCALA",
            "rdfs:comment": "The Grundfos SCALA pumps are all-in-one integrated self-priming pressure boosters designed for domestic use and ensure a constant supply of clean water to households, gardens and light commercial applications.",
            "skos:inScheme": "https://grundfos.com/concept/productFamily",
            "skos:narrower": [
                "https://grundfos.com/concept/productFamily/SCALAACC",
                "https://grundfos.com/concept/productFamily/SCALA2"
            ],
            "skos:prefLabel": "SCALA"
        },
        {
            "@id": "https://grundfos.com/concept/productFamily/SE100",
            "@type": [
                "gfs:ProductFamily",
                "skos:Concept"
            ],
            "gfs:level": 2,
            "gfs:typecode": "SE100",
            "rdfs:comment": "Submersible Grundfos SE sewage pumps (1.1-11 kW) are fitted with either S-tube\u00c3\u201a\u00c2\u00ae (SE1) or SuperVortex impeller (SEV). The free passage through the pump varies from 50-100 mm depending on size.",
            "skos:inScheme": "https://grundfos.com/concept/productFamily",
            "skos:prefLabel": "SE1"
        },
        {
            "@id": "https://grundfos.com/concept/productFamily/SEV00",
            "@type": [
                "gfs:ProductFamily",
                "skos:Concept"
            ],
            "gfs:level": 2,
            "gfs:typecode": "SEV00",
            "rdfs:comment": "Submersible Grundfos SEV sewage pumps (1.1-11 kW) are fitted with a SuperVortex impeller. The free passage through the pump varies from 50-100 mm depending on size.",
            "skos:inScheme": "https://grundfos.com/concept/productFamily",
            "skos:prefLabel": "SEV"
        },
        {
            "@id": "https://grundfos.com/concept/productFamily/SEFAM",
            "@type": [
                "gfs:ProductFamily",
                "skos:Concept"
            ],
            "gfs:level": 1,
            "gfs:typecode": "SEFAM",
            "rdfs:comment": "Submersible Grundfos SE sewage pumps (1.1-11 kW) are fitted with either S-tube\u00c3\u201a\u00c2\u00ae (SE1) or SuperVortex impeller (SEV). The free passage through the pump varies from 50-100 mm depending on size.",
            "skos:inScheme": "https://grundfos.com/concept/productFamily",
            "skos:narrower": [
                "https://grundfos.com/concept/productFamily/SE100",
                "https://grundfos.com/concept/productFamily/SEV00"
            ],
            "skos:prefLabel": "SE"
        },
        {
            "@id": "https://grundfos.com/concept/productFamily/SESLFAM",
            "@type": [
                "gfs:ProductFamily",
                "skos:Concept"
            ],
            "gfs:level": 1,
            "gfs:typecode": "SESLFAM",
            "rdfs:comment": "Submersible Grundfos SE/SL sewage pumps (9-30 kW) are fitted with either S-tube\u00c3\u201a\u00c2\u00ae or SuperVortex impeller (SLV). The free passage through the pump varies from 75-125 mm depending on size.",
            "skos:inScheme": "https://grundfos.com/concept/productFamily",
            "skos:narrower": [],
            "skos:prefLabel": "SE/SL 9-30 kW"
        },
        {
            "@id": "https://grundfos.com/concept/productFamily/SEGFAM",
            "@type": [
                "gfs:ProductFamily",
                "skos:Concept"
            ],
            "gfs:level": 1,
            "gfs:typecode": "SEGFAM",
            "rdfs:comment": "Submersible Grundfos SEG sewage grinder pumps (0.9-4 kW) are designed for pumping wastewater, sludge-containing water, and sewage. Fitted with a patented grinder system designed to grind the media.",
            "skos:inScheme": "https://grundfos.com/concept/productFamily",
            "skos:narrower": [],
            "skos:prefLabel": "SEG"
        },
        {
            "@id": "https://grundfos.com/concept/productFamily/ACCSEN",
            "@type": [
                "gfs:ProductFamily",
                "skos:Concept"
            ],
            "gfs:level": 2,
            "gfs:typecode": "ACCSEN",
            "rdfs:comment": "Accessories for sensor products",
            "skos:inScheme": "https://grundfos.com/concept/productFamily",
            "skos:prefLabel": "Accessories, Sensors"
        },
        {
            "@id": "https://grundfos.com/concept/productFamily/LEVEL000",
            "@type": [
                "gfs:ProductFamily",
                "skos:Concept"
            ],
            "gfs:level": 2,
            "gfs:typecode": "LEVEL000",
            "rdfs:comment": "Float switches for level control/monitoring in tanks, pumping stations or similar applications.",
            "skos:inScheme": "https://grundfos.com/concept/productFamily",
            "skos:prefLabel": "Float switches"
        },
        {
            "@id": "https://grundfos.com/concept/productFamily/LEVELS00",
            "@type": [
                "gfs:ProductFamily",
                "skos:Concept"
            ],
            "gfs:level": 2,
            "gfs:typecode": "LEVELS00",
            "rdfs:comment": "Group program of submersible sensors for hydrostatic level measurements.",
            "skos:inScheme": "https://grundfos.com/concept/productFamily",
            "skos:prefLabel": "Level sensors"
        },
        {
            "@id": "https://grundfos.com/concept/productFamily/TEMP000",
            "@type": [
                "gfs:ProductFamily",
                "skos:Concept"
            ],
            "gfs:level": 2,
            "gfs:typecode": "TEMP000",
            "rdfs:comment": "Pressure, flow and temperature products. Transducers, sensors, switches, meters, transmitters. Grundfos Direct Sensors and insourced products. For use across products, applications and solutions.",
            "skos:inScheme": "https://grundfos.com/concept/productFamily",
            "skos:prefLabel": "Temperature, Pressure, Flow Sensors, Transmitter"
        },
        {
            "@id": "https://grundfos.com/concept/productFamily/SENSOFAM",
            "@type": [
                "gfs:ProductFamily",
                "skos:Concept"
            ],
            "gfs:level": 1,
            "gfs:typecode": "SENSOFAM",
            "rdfs:comment": "Group program of measuring and switching products. Transducers, sensors, floats, switches, meters, transmitter, probes and associated controllers. For use across products, applications and solutions.",
            "skos:inScheme": "https://grundfos.com/concept/productFamily",
            "skos:narrower": [
                "https://grundfos.com/concept/productFamily/ACCSEN",
                "https://grundfos.com/concept/productFamily/LEVEL000",
                "https://grundfos.com/concept/productFamily/LEVELS00",
                "https://grundfos.com/concept/productFamily/TEMP000"
            ],
            "skos:prefLabel": "Sensor, Transmitter and Switches"
        },
        {
            "@id": "https://grundfos.com/concept/productFamily/SERCUSTO",
            "@type": [
                "gfs:ProductFamily",
                "skos:Concept"
            ],
            "gfs:level": 2,
            "gfs:typecode": "SERCUSTO",
            "rdfs:comment": "A customised service agreement from Grundfos provides you with the exact services you need to stay on top of equipment status at all times for a fixed price.",
            "skos:inScheme": "https://grundfos.com/concept/productFamily",
            "skos:prefLabel": "Customised Service Agreement"
        },
        {
            "@id": "https://grundfos.com/concept/productFamily/SERPERFO",
            "@type": [
                "gfs:ProductFamily",
                "skos:Concept"
            ],
            "gfs:level": 2,
            "gfs:typecode": "SERPERFO",
            "rdfs:comment": "Let Grundfos specialists take care of delivering on your goals, and free up your time and mind for other tasks.",
            "skos:inScheme": "https://grundfos.com/concept/productFamily",
            "skos:prefLabel": "Performance Agreement"
        },
        {
            "@id": "https://grundfos.com/concept/productFamily/SERSERCO",
            "@type": [
                "gfs:ProductFamily",
                "skos:Concept"
            ],
            "gfs:level": 2,
            "gfs:typecode": "SERSERCO",
            "rdfs:comment": "Let us take care of your pumping system, while you take care of your business.",
            "skos:inScheme": "https://grundfos.com/concept/productFamily",
            "skos:prefLabel": "Standard Service Agreement"
        },
        {
            "@id": "https://grundfos.com/concept/productFamily/SERIO",
            "@type": [
                "gfs:ProductFamily",
                "skos:Concept"
            ],
            "gfs:level": 1,
            "gfs:typecode": "SERIO",
            "rdfs:comment": "Keep your system running in top condition and experience reduced operating costs, predictable maintenance costs and increased system lifetime. With a Grundfos service agreement, you can leave your service, maintenance and analysis to experienced professionals.",
            "skos:inScheme": "https://grundfos.com/concept/productFamily",
            "skos:narrower": [
                "https://grundfos.com/concept/productFamily/SERCUSTO",
                "https://grundfos.com/concept/productFamily/SERPERFO",
                "https://grundfos.com/concept/productFamily/SERSERCO"
            ],
            "skos:prefLabel": "Service agreements"
        },
        {
            "@id": "https://grundfos.com/concept/productFamily/SHOWFAM",
            "@type": [
                "gfs:ProductFamily",
                "skos:Concept"
            ],
            "gfs:level": 1,
            "gfs:typecode": "SHOWFAM",
            "rdfs:comment": "Grundfos shower pumps are used for boosting hot and cold water to showers, bathrooms or whole households. Shower pumps allows customers to boost performance and have a more powerful showering experience.",
            "skos:inScheme": "https://grundfos.com/concept/productFamily",
            "skos:narrower": [],
            "skos:prefLabel": "Shower pumps"
        },
        {
            "@id": "https://grundfos.com/concept/productFamily/SL1000",
            "@type": [
                "gfs:ProductFamily",
                "skos:Concept"
            ],
            "gfs:level": 2,
            "gfs:typecode": "SL1000",
            "rdfs:comment": "Submersible Grundfos SL sewage pumps (1.1-11 kW) are fitted with an S-tube\u00c3\u201a\u00c2\u00ae impeller. The free passage through the pump varies from 50-100 mm depending on size.",
            "skos:inScheme": "https://grundfos.com/concept/productFamily",
            "skos:prefLabel": "SL1"
        },
        {
            "@id": "https://grundfos.com/concept/productFamily/SLV000",
            "@type": [
                "gfs:ProductFamily",
                "skos:Concept"
            ],
            "gfs:level": 2,
            "gfs:typecode": "SLV000",
            "rdfs:comment": "Submersible Grundfos SLV sewage pumps (1.1-11 kW) are fitted with a SuperVortex impeller. The free passage through the pump varies from 50-100 mm depending on size.",
            "skos:inScheme": "https://grundfos.com/concept/productFamily",
            "skos:prefLabel": "SLV"
        },
        {
            "@id": "https://grundfos.com/concept/productFamily/SLFAM",
            "@type": [
                "gfs:ProductFamily",
                "skos:Concept"
            ],
            "gfs:level": 1,
            "gfs:typecode": "SLFAM",
            "rdfs:comment": "Submersible Grundfos SL sewage pumps (1.1-11 kW) are fitted with either S-tube\u00c3\u201a\u00c2\u00ae (SL1) or SuperVortex impeller (SLV). The free passage through the pump varies from 50-100 mm depending on size.",
            "skos:inScheme": "https://grundfos.com/concept/productFamily",
            "skos:narrower": [
                "https://grundfos.com/concept/productFamily/SL1000",
                "https://grundfos.com/concept/productFamily/SLV000"
            ],
            "skos:prefLabel": "SL"
        },
        {
            "@id": "https://grundfos.com/concept/productFamily/GF5565C",
            "@type": [
                "gfs:ProductFamily",
                "skos:Concept"
            ],
            "gfs:level": 2,
            "gfs:typecode": "GF5565C",
            "rdfs:comment": "Solar modules generate photovoltaic power, and supply DC electricity from the solar irradiation to SQFlex, MGFlex and RSI inverters",
            "skos:inScheme": "https://grundfos.com/concept/productFamily",
            "skos:prefLabel": "GF 80, GF 100 TF, GF 100 C, GF 100 S"
        },
        {
            "@id": "https://grundfos.com/concept/productFamily/SOLMFAM",
            "@type": [
                "gfs:ProductFamily",
                "skos:Concept"
            ],
            "gfs:level": 1,
            "gfs:typecode": "SOLMFAM",
            "rdfs:comment": "Solar modules generate photovoltaic power, and supply DC electricity from the solar irradiation to SQFlex, MGFlex and RSI inverters",
            "skos:inScheme": "https://grundfos.com/concept/productFamily",
            "skos:narrower": [
                "https://grundfos.com/concept/productFamily/GF5565C"
            ],
            "skos:prefLabel": "Solar modules"
        },
        {
            "@id": "https://grundfos.com/concept/productFamily/SOLOLIF2",
            "@type": [
                "gfs:ProductFamily",
                "skos:Concept"
            ],
            "gfs:level": 1,
            "gfs:typecode": "SOLOLIF2",
            "rdfs:comment": "Grundfos SOLOLIFT2 are small, compact, ready-to-install automatic lifting stations with integrated powerful cutter systems. Suitable for pumping wastewater with feces from private dwellings. The unit is designed according to EN 12050-3.",
            "skos:inScheme": "https://grundfos.com/concept/productFamily",
            "skos:narrower": [],
            "skos:prefLabel": "Sololift2"
        },
        {
            "@id": "https://grundfos.com/concept/productFamily/SPFAM",
            "@type": [
                "gfs:ProductFamily",
                "skos:Concept"
            ],
            "gfs:level": 2,
            "gfs:typecode": "SPFAM",
            "rdfs:comment": "Grundfos SP are submersible borehole pumps, designed for pumping groundwater. Grundfos SP are all stainless-steel pumps, and they are available in 3 material grades. The pumps are suitable for boreholes in sizes ranging from 4\" over 6\" and 8\" to 10\". The motor sizes for the pumps are available in 0.37-250 kW.",
            "skos:inScheme": "https://grundfos.com/concept/productFamily",
            "skos:prefLabel": "SP"
        },
        {
            "@id": "https://grundfos.com/concept/productFamily/SPGFAM",
            "@type": [
                "gfs:ProductFamily",
                "skos:Concept"
            ],
            "gfs:level": 2,
            "gfs:typecode": "SPGFAM",
            "rdfs:comment": "Grundfos SP are submersible borehole pumps, designed for pumping groundwater. Grundfos SP-G are high capacity cast iron pumps. The pumps are suitable for boreholes in size 12\".",
            "skos:inScheme": "https://grundfos.com/concept/productFamily",
            "skos:prefLabel": "SP-G"
        },
        {
            "@id": "https://grundfos.com/concept/productFamily/SPRANGE",
            "@type": [
                "gfs:ProductFamily",
                "skos:Concept"
            ],
            "gfs:level": 1,
            "gfs:typecode": "SPRANGE",
            "rdfs:comment": "Grundfos SP are submersible borehole pumps, designed for pumping groundwater. Grundfos SP are all stainless-steel pumps, and they are available in 3 material grades. The pumps are suitable for boreholes in sizes ranging from 4\" over 6\" and 8\" to 10\". The motor sizes for the pumps are available in 0.37-250 kW.",
            "skos:inScheme": "https://grundfos.com/concept/productFamily",
            "skos:narrower": [
                "https://grundfos.com/concept/productFamily/SPFAM",
                "https://grundfos.com/concept/productFamily/SPGFAM"
            ],
            "skos:prefLabel": "SP, SP-G"
        },
        {
            "@id": "https://grundfos.com/concept/productFamily/SPNE03",
            "@type": [
                "gfs:ProductFamily",
                "skos:Concept"
            ],
            "gfs:level": 2,
            "gfs:typecode": "SPNE03",
            "rdfs:comment": "Grundfos SP are submersible borehole pumps, designed for pumping contaminated/polluted groundwater for leachate, sampling, and water quality monitoring. Grundfos SP-NE are all stainless-steel pumps, and they are suitable for boreholes in sizes 4\"and 6\".",
            "skos:inScheme": "https://grundfos.com/concept/productFamily",
            "skos:prefLabel": "SP 3A-NE"
        },
        {
            "@id": "https://grundfos.com/concept/productFamily/SPNE05",
            "@type": [
                "gfs:ProductFamily",
                "skos:Concept"
            ],
            "gfs:level": 2,
            "gfs:typecode": "SPNE05",
            "rdfs:comment": "Grundfos SP are submersible borehole pumps, designed for pumping contaminated/polluted groundwater for leachate, sampling, and water quality monitoring. Grundfos SP-NE are all stainless-steel pumps, and they are suitable for boreholes in sizes 4\"and 6\".",
            "skos:inScheme": "https://grundfos.com/concept/productFamily",
            "skos:prefLabel": "SP 5A-NE"
        },
        {
            "@id": "https://grundfos.com/concept/productFamily/SPNE09",
            "@type": [
                "gfs:ProductFamily",
                "skos:Concept"
            ],
            "gfs:level": 2,
            "gfs:typecode": "SPNE09",
            "rdfs:comment": "Grundfos SP are submersible borehole pumps, designed for pumping contaminated/polluted groundwater for leachate, sampling, and water quality monitoring. Grundfos SP-NE are all stainless-steel pumps, and they are suitable for boreholes in sizes 4\"and 6\".",
            "skos:inScheme": "https://grundfos.com/concept/productFamily",
            "skos:prefLabel": "SP 9-NE"
        },
        {
            "@id": "https://grundfos.com/concept/productFamily/SPNE17",
            "@type": [
                "gfs:ProductFamily",
                "skos:Concept"
            ],
            "gfs:level": 2,
            "gfs:typecode": "SPNE17",
            "rdfs:comment": "Grundfos SP are submersible borehole pumps, designed for pumping contaminated/polluted groundwater for leachate, sampling, and water quality monitoring. Grundfos SP-NE are all stainless-steel pumps, and they are suitable for boreholes in sizes 4\"and 6\".",
            "skos:inScheme": "https://grundfos.com/concept/productFamily",
            "skos:prefLabel": "SP 17-NE"
        },
        {
            "@id": "https://grundfos.com/concept/productFamily/SPNEFAM",
            "@type": [
                "gfs:ProductFamily",
                "skos:Concept"
            ],
            "gfs:level": 1,
            "gfs:typecode": "SPNEFAM",
            "rdfs:comment": "Grundfos SP are submersible borehole pumps, designed for pumping contaminated/polluted groundwater for leachate, sampling, and water quality monitoring. Grundfos SP-NE are all stainless-steel pumps, and they are suitable for boreholes in sizes 4\"and 6\".",
            "skos:inScheme": "https://grundfos.com/concept/productFamily",
            "skos:narrower": [
                "https://grundfos.com/concept/productFamily/SPNE03",
                "https://grundfos.com/concept/productFamily/SPNE05",
                "https://grundfos.com/concept/productFamily/SPNE09",
                "https://grundfos.com/concept/productFamily/SPNE17"
            ],
            "skos:prefLabel": "SP-NE"
        },
        {
            "@id": "https://grundfos.com/concept/productFamily/SQC01",
            "@type": [
                "gfs:ProductFamily",
                "skos:Concept"
            ],
            "gfs:level": 2,
            "gfs:typecode": "SQC01",
            "rdfs:comment": "Submersible pumps",
            "skos:inScheme": "https://grundfos.com/concept/productFamily",
            "skos:prefLabel": "SQ 1"
        },
        {
            "@id": "https://grundfos.com/concept/productFamily/SQC02",
            "@type": [
                "gfs:ProductFamily",
                "skos:Concept"
            ],
            "gfs:level": 2,
            "gfs:typecode": "SQC02",
            "rdfs:comment": "Submersible pumps",
            "skos:inScheme": "https://grundfos.com/concept/productFamily",
            "skos:prefLabel": "SQ 2"
        },
        {
            "@id": "https://grundfos.com/concept/productFamily/SQC03",
            "@type": [
                "gfs:ProductFamily",
                "skos:Concept"
            ],
            "gfs:level": 2,
            "gfs:typecode": "SQC03",
            "rdfs:comment": "Submersible pumps",
            "skos:inScheme": "https://grundfos.com/concept/productFamily",
            "skos:prefLabel": "SQ 3"
        },
        {
            "@id": "https://grundfos.com/concept/productFamily/SQC05",
            "@type": [
                "gfs:ProductFamily",
                "skos:Concept"
            ],
            "gfs:level": 2,
            "gfs:typecode": "SQC05",
            "rdfs:comment": "Submersible pumps",
            "skos:inScheme": "https://grundfos.com/concept/productFamily",
            "skos:prefLabel": "SQ 5"
        },
        {
            "@id": "https://grundfos.com/concept/productFamily/SQC07",
            "@type": [
                "gfs:ProductFamily",
                "skos:Concept"
            ],
            "gfs:level": 2,
            "gfs:typecode": "SQC07",
            "rdfs:comment": "Submersible pumps",
            "skos:inScheme": "https://grundfos.com/concept/productFamily",
            "skos:prefLabel": "SQ 7"
        },
        {
            "@id": "https://grundfos.com/concept/productFamily/SQCFAM",
            "@type": [
                "gfs:ProductFamily",
                "skos:Concept"
            ],
            "gfs:level": 1,
            "gfs:typecode": "SQCFAM",
            "rdfs:comment": "Grundfos SQ pumps are compact submersible pumps, designed for domestic groundwater supply for private housing, small waterworks, and small irrigation systems.",
            "skos:inScheme": "https://grundfos.com/concept/productFamily",
            "skos:narrower": [
                "https://grundfos.com/concept/productFamily/SQC01",
                "https://grundfos.com/concept/productFamily/SQC02",
                "https://grundfos.com/concept/productFamily/SQC03",
                "https://grundfos.com/concept/productFamily/SQC05",
                "https://grundfos.com/concept/productFamily/SQC07"
            ],
            "skos:prefLabel": "SQ"
        },
        {
            "@id": "https://grundfos.com/concept/productFamily/SQEC01",
            "@type": [
                "gfs:ProductFamily",
                "skos:Concept"
            ],
            "gfs:level": 2,
            "gfs:typecode": "SQEC01",
            "rdfs:comment": "Submersible pumps with variable speed motor",
            "skos:inScheme": "https://grundfos.com/concept/productFamily",
            "skos:prefLabel": "SQE 1"
        },
        {
            "@id": "https://grundfos.com/concept/productFamily/SQEC02",
            "@type": [
                "gfs:ProductFamily",
                "skos:Concept"
            ],
            "gfs:level": 2,
            "gfs:typecode": "SQEC02",
            "rdfs:comment": "Submersible pumps with variable speed motor",
            "skos:inScheme": "https://grundfos.com/concept/productFamily",
            "skos:prefLabel": "SQE 2"
        },
        {
            "@id": "https://grundfos.com/concept/productFamily/SQEC03",
            "@type": [
                "gfs:ProductFamily",
                "skos:Concept"
            ],
            "gfs:level": 2,
            "gfs:typecode": "SQEC03",
            "rdfs:comment": "Submersible pumps with variable speed motor",
            "skos:inScheme": "https://grundfos.com/concept/productFamily",
            "skos:prefLabel": "SQE 3"
        },
        {
            "@id": "https://grundfos.com/concept/productFamily/SQEC05",
            "@type": [
                "gfs:ProductFamily",
                "skos:Concept"
            ],
            "gfs:level": 2,
            "gfs:typecode": "SQEC05",
            "rdfs:comment": "Submersible pumps with variable speed motor",
            "skos:inScheme": "https://grundfos.com/concept/productFamily",
            "skos:prefLabel": "SQE 5"
        },
        {
            "@id": "https://grundfos.com/concept/productFamily/SQEC07",
            "@type": [
                "gfs:ProductFamily",
                "skos:Concept"
            ],
            "gfs:level": 2,
            "gfs:typecode": "SQEC07",
            "rdfs:comment": "Submersible pumps with variable speed motor",
            "skos:inScheme": "https://grundfos.com/concept/productFamily",
            "skos:prefLabel": "SQE 7"
        },
        {
            "@id": "https://grundfos.com/concept/productFamily/SQECFAM",
            "@type": [
                "gfs:ProductFamily",
                "skos:Concept"
            ],
            "gfs:level": 1,
            "gfs:typecode": "SQECFAM",
            "rdfs:comment": "Grundfos SQE pumps are compact submersible pumps, designed for constant pressure applications within domestic groundwater supply for private housing, small waterworks, and small irrigation systems.",
            "skos:inScheme": "https://grundfos.com/concept/productFamily",
            "skos:narrower": [
                "https://grundfos.com/concept/productFamily/SQEC01",
                "https://grundfos.com/concept/productFamily/SQEC02",
                "https://grundfos.com/concept/productFamily/SQEC03",
                "https://grundfos.com/concept/productFamily/SQEC05",
                "https://grundfos.com/concept/productFamily/SQEC07"
            ],
            "skos:prefLabel": "SQE"
        },
        {
            "@id": "https://grundfos.com/concept/productFamily/SQENEC",
            "@type": [
                "gfs:ProductFamily",
                "skos:Concept"
            ],
            "gfs:level": 1,
            "gfs:typecode": "SQENEC",
            "rdfs:comment": "Grundfos SQE-NE pumps are compact submersible pumps, designed for remedial pumping and liquid sampling from areas with contaminated groundwater.",
            "skos:inScheme": "https://grundfos.com/concept/productFamily",
            "skos:narrower": [],
            "skos:prefLabel": "SQE-NE"
        },
        {
            "@id": "https://grundfos.com/concept/productFamily/SQFFAM",
            "@type": [
                "gfs:ProductFamily",
                "skos:Concept"
            ],
            "gfs:level": 1,
            "gfs:typecode": "SQFFAM",
            "rdfs:comment": "Renewable energy submersible pumps with build in inverter for solar, wind and AC powersource. Runs on both AC and DC voltage",
            "skos:inScheme": "https://grundfos.com/concept/productFamily",
            "skos:narrower": [],
            "skos:prefLabel": "SQFlex"
        },
        {
            "@id": "https://grundfos.com/concept/productFamily/TP000",
            "@type": [
                "gfs:ProductFamily",
                "skos:Concept"
            ],
            "gfs:level": 2,
            "gfs:typecode": "TP000",
            "rdfs:comment": "Single-stage in-line pumps",
            "skos:inScheme": "https://grundfos.com/concept/productFamily",
            "skos:prefLabel": "TP"
        },
        {
            "@id": "https://grundfos.com/concept/productFamily/TPB00",
            "@type": [
                "gfs:ProductFamily",
                "skos:Concept"
            ],
            "gfs:level": 2,
            "gfs:typecode": "TPB00",
            "rdfs:comment": "Single-stage in-line pumps with pump housing in bronze or stainless steel",
            "skos:inScheme": "https://grundfos.com/concept/productFamily",
            "skos:prefLabel": "TP (B), (I)"
        },
        {
            "@id": "https://grundfos.com/concept/productFamily/TPD00",
            "@type": [
                "gfs:ProductFamily",
                "skos:Concept"
            ],
            "gfs:level": 2,
            "gfs:typecode": "TPD00",
            "rdfs:comment": "Twin-head single-stage in-line pumps",
            "skos:inScheme": "https://grundfos.com/concept/productFamily",
            "skos:prefLabel": "TPD"
        },
        {
            "@id": "https://grundfos.com/concept/productFamily/TPE00",
            "@type": [
                "gfs:ProductFamily",
                "skos:Concept"
            ],
            "gfs:level": 2,
            "gfs:typecode": "TPE00",
            "rdfs:comment": "Single-stage in-line pumps with frequency converters",
            "skos:inScheme": "https://grundfos.com/concept/productFamily",
            "skos:prefLabel": "TPE Series 1000, TPE2"
        },
        {
            "@id": "https://grundfos.com/concept/productFamily/TPE0S2",
            "@type": [
                "gfs:ProductFamily",
                "skos:Concept"
            ],
            "gfs:level": 2,
            "gfs:typecode": "TPE0S2",
            "rdfs:comment": "Single-stage in-line pumps with frequency converters",
            "skos:inScheme": "https://grundfos.com/concept/productFamily",
            "skos:prefLabel": "TPE Series 2000, TPE3"
        },
        {
            "@id": "https://grundfos.com/concept/productFamily/TPE3NI",
            "@type": [
                "gfs:ProductFamily",
                "skos:Concept"
            ],
            "gfs:level": 2,
            "gfs:typecode": "TPE3NI",
            "rdfs:comment": "Single-stage stainless steel in-line pumps with frequency converters",
            "skos:inScheme": "https://grundfos.com/concept/productFamily",
            "skos:prefLabel": "TPE2 (I)"
        },
        {
            "@id": "https://grundfos.com/concept/productFamily/TPE3SI",
            "@type": [
                "gfs:ProductFamily",
                "skos:Concept"
            ],
            "gfs:level": 2,
            "gfs:typecode": "TPE3SI",
            "rdfs:comment": "Single-stage stainless steel in-line pumps with frequency converters",
            "skos:inScheme": "https://grundfos.com/concept/productFamily",
            "skos:prefLabel": "TPE3  (I)"
        },
        {
            "@id": "https://grundfos.com/concept/productFamily/TPED0",
            "@type": [
                "gfs:ProductFamily",
                "skos:Concept"
            ],
            "gfs:level": 2,
            "gfs:typecode": "TPED0",
            "rdfs:comment": "Twin-head single-stage in-line pumps with frequency converters",
            "skos:inScheme": "https://grundfos.com/concept/productFamily",
            "skos:prefLabel": "TPED Series 1000, TPE2 D"
        },
        {
            "@id": "https://grundfos.com/concept/productFamily/TPEDS2",
            "@type": [
                "gfs:ProductFamily",
                "skos:Concept"
            ],
            "gfs:level": 2,
            "gfs:typecode": "TPEDS2",
            "rdfs:comment": "Twin-head single-stage in-line pumps with frequency converters",
            "skos:inScheme": "https://grundfos.com/concept/productFamily",
            "skos:prefLabel": "TPED Series 2000, TPE3 D"
        },
        {
            "@id": "https://grundfos.com/concept/productFamily/TPFAM",
            "@type": [
                "gfs:ProductFamily",
                "skos:Concept"
            ],
            "gfs:level": 1,
            "gfs:typecode": "TPFAM",
            "rdfs:comment": "Single-stage, in-line centrifugal pumps with mechanical shaft seal. The pumps are close-coupled, i.e. pump and motor are separate units",
            "skos:inScheme": "https://grundfos.com/concept/productFamily",
            "skos:narrower": [
                "https://grundfos.com/concept/productFamily/TP000",
                "https://grundfos.com/concept/productFamily/TPB00",
                "https://grundfos.com/concept/productFamily/TPD00",
                "https://grundfos.com/concept/productFamily/TPE00",
                "https://grundfos.com/concept/productFamily/TPE0S2",
                "https://grundfos.com/concept/productFamily/TPE3NI",
                "https://grundfos.com/concept/productFamily/TPE3SI",
                "https://grundfos.com/concept/productFamily/TPED0",
                "https://grundfos.com/concept/productFamily/TPEDS2"
            ],
            "skos:prefLabel": "TP, TPE"
        },
        {
            "@id": "https://grundfos.com/concept/productFamily/AP012",
            "@type": [
                "gfs:ProductFamily",
                "skos:Concept"
            ],
            "gfs:level": 2,
            "gfs:typecode": "AP012",
            "rdfs:comment": "Grundfos UNILIFT AP12 are stainless-steel submersible pumps designed for pumping non-aggressive water and grey wastewater such as drainage and domestic effluents with particles up to 12 mm. The pump can be used as a portable unit or stationary installation inside and outside buildings.",
            "skos:inScheme": "https://grundfos.com/concept/productFamily",
            "skos:prefLabel": "Unilift AP12"
        },
        {
            "@id": "https://grundfos.com/concept/productFamily/AP035",
            "@type": [
                "gfs:ProductFamily",
                "skos:Concept"
            ],
            "gfs:level": 2,
            "gfs:typecode": "AP035",
            "rdfs:comment": "Grundfos UNILIFT AP35 are stainless-steel submersible pumps designed for pumping non-aggressive water and grey wastewater such as drainage and domestic effluents with particles up to 35 mm. The pump can be used as a portable unit or stationary installation inside and outside buildings.",
            "skos:inScheme": "https://grundfos.com/concept/productFamily",
            "skos:prefLabel": "Unilift AP35"
        },
        {
            "@id": "https://grundfos.com/concept/productFamily/AP35B",
            "@type": [
                "gfs:ProductFamily",
                "skos:Concept"
            ],
            "gfs:level": 2,
            "gfs:typecode": "AP35B",
            "rdfs:comment": "Grundfos UNILIFT AP35B are stainless-steel submersible pumps designed for pumping effluents (excluding toilet discharge), with particles up to 35 mm. The pump is suitable for installation on auto coupling, allowing for easy access to the pump for maintenance and other purposes.",
            "skos:inScheme": "https://grundfos.com/concept/productFamily",
            "skos:prefLabel": "Unilift AP35B"
        },
        {
            "@id": "https://grundfos.com/concept/productFamily/AP050",
            "@type": [
                "gfs:ProductFamily",
                "skos:Concept"
            ],
            "gfs:level": 2,
            "gfs:typecode": "AP050",
            "rdfs:comment": "Grundfos UNILIFT AP50 are stainless-steel submersible pumps designed for pumping non-aggressive water and grey wastewater such as drainage and domestic effluents with particles up to 50 mm. The pump can be used as a portable unit or stationary installation inside and outside buildings.",
            "skos:inScheme": "https://grundfos.com/concept/productFamily",
            "skos:prefLabel": "Unilift AP50"
        },
        {
            "@id": "https://grundfos.com/concept/productFamily/AP50B",
            "@type": [
                "gfs:ProductFamily",
                "skos:Concept"
            ],
            "gfs:level": 2,
            "gfs:typecode": "AP50B",
            "rdfs:comment": "Grundfos UNILIFT AP50B are stainless-steel submersible pumps designed for pumping waste water, including toilet discharge (where allowed), with particles up to 50 mm. The pump is suitable for installation on auto coupling, allowing for easy access to the pump for maintenance and other purposes.",
            "skos:inScheme": "https://grundfos.com/concept/productFamily",
            "skos:prefLabel": "Unilift AP50B"
        },
        {
            "@id": "https://grundfos.com/concept/productFamily/APUFAM",
            "@type": [
                "gfs:ProductFamily",
                "skos:Concept"
            ],
            "gfs:level": 1,
            "gfs:typecode": "APUFAM",
            "rdfs:comment": "Drainage, effluent and domestic sewage pumps",
            "skos:inScheme": "https://grundfos.com/concept/productFamily",
            "skos:narrower": [
                "https://grundfos.com/concept/productFamily/AP012",
                "https://grundfos.com/concept/productFamily/AP035",
                "https://grundfos.com/concept/productFamily/AP35B",
                "https://grundfos.com/concept/productFamily/AP050",
                "https://grundfos.com/concept/productFamily/AP50B"
            ],
            "skos:prefLabel": "Unilift AP"
        },
        {
            "@id": "https://grundfos.com/concept/productFamily/CCFAM",
            "@type": [
                "gfs:ProductFamily",
                "skos:Concept"
            ],
            "gfs:level": 1,
            "gfs:typecode": "CCFAM",
            "rdfs:comment": "Grundfos UNILIFT CC pumps are single-stage submersible pumps designed for pumping clean, non-aggressive water and slightly dirty (grey) wastewater. Capable of pumping down to 3 mm water level. The pumps have both a top and a side outlet allowing easy adaptation to existing pipework.",
            "skos:inScheme": "https://grundfos.com/concept/productFamily",
            "skos:narrower": [],
            "skos:prefLabel": "Unilift CC"
        },
        {
            "@id": "https://grundfos.com/concept/productFamily/KP000",
            "@type": [
                "gfs:ProductFamily",
                "skos:Concept"
            ],
            "gfs:level": 1,
            "gfs:typecode": "KP000",
            "rdfs:comment": "Grundfos UNILIFT KP are stainless-steel submersible pumps designed for pumping non-aggressive water and grey wastewater such as drainage and domestic effluents with particles up to 10 mm. The pump can be used as a portable unit or stationary installation inside and outside buildings.",
            "skos:inScheme": "https://grundfos.com/concept/productFamily",
            "skos:narrower": [],
            "skos:prefLabel": "Unilift KP"
        },
        {
            "@id": "https://grundfos.com/concept/productFamily/LIFTCONT",
            "@type": [
                "gfs:ProductFamily",
                "skos:Concept"
            ],
            "gfs:level": 2,
            "gfs:typecode": "LIFTCONT",
            "rdfs:comment": "Accessories",
            "skos:inScheme": "https://grundfos.com/concept/productFamily",
            "skos:prefLabel": "Controllers"
        },
        {
            "@id": "https://grundfos.com/concept/productFamily/DUO000",
            "@type": [
                "gfs:ProductFamily",
                "skos:Concept"
            ],
            "gfs:level": 2,
            "gfs:typecode": "DUO000",
            "rdfs:comment": "Lifting stations for collecting and removing wastewater of inside buildings",
            "skos:inScheme": "https://grundfos.com/concept/productFamily",
            "skos:prefLabel": "Duolift systems"
        },
        {
            "@id": "https://grundfos.com/concept/productFamily/UNODUOTA",
            "@type": [
                "gfs:ProductFamily",
                "skos:Concept"
            ],
            "gfs:level": 2,
            "gfs:typecode": "UNODUOTA",
            "rdfs:comment": "Wastewater collecting tanks for lifting stations with a one or two pump system. Suitable for collecting and removing wastewater from inside buildings i.e. basements/cellars below sewer level (note: not designed for traffic loads).",
            "skos:inScheme": "https://grundfos.com/concept/productFamily",
            "skos:prefLabel": "Uno-/Duolift tanks"
        },
        {
            "@id": "https://grundfos.com/concept/productFamily/UNO000",
            "@type": [
                "gfs:ProductFamily",
                "skos:Concept"
            ],
            "gfs:level": 2,
            "gfs:typecode": "UNO000",
            "rdfs:comment": "Lifting stations for collecting and removing wastewater of inside buildings",
            "skos:inScheme": "https://grundfos.com/concept/productFamily",
            "skos:prefLabel": "Unolift systems"
        },
        {
            "@id": "https://grundfos.com/concept/productFamily/UNOFAM",
            "@type": [
                "gfs:ProductFamily",
                "skos:Concept"
            ],
            "gfs:level": 1,
            "gfs:typecode": "UNOFAM",
            "rdfs:comment": "One and two pump systems suitable for collection and pumping of wastewater from basements/cellars below sewer level (note: not designed for traffic loads)",
            "skos:inScheme": "https://grundfos.com/concept/productFamily",
            "skos:narrower": [
                "https://grundfos.com/concept/productFamily/LIFTCONT",
                "https://grundfos.com/concept/productFamily/DUO000",
                "https://grundfos.com/concept/productFamily/UNODUOTA",
                "https://grundfos.com/concept/productFamily/UNO000"
            ],
            "skos:prefLabel": "UNO-/DUOLIFT Lifting Stations"
        },
        {
            "@id": "https://grundfos.com/concept/productFamily/ALPHA11",
            "@type": [
                "gfs:ProductFamily",
                "skos:Concept"
            ],
            "gfs:level": 2,
            "gfs:typecode": "ALPHA11",
            "rdfs:comment": "Grundfos ALPHA1.1 are stand-alone circulators with basic control functions.",
            "skos:inScheme": "https://grundfos.com/concept/productFamily",
            "skos:prefLabel": "ALPHA1.1 OEM"
        },
        {
            "@id": "https://grundfos.com/concept/productFamily/ALPHA21",
            "@type": [
                "gfs:ProductFamily",
                "skos:Concept"
            ],
            "gfs:level": 2,
            "gfs:typecode": "ALPHA21",
            "rdfs:comment": "Grundfos ALPHA2.1 are stand-alone circulators with advanced control functions.",
            "skos:inScheme": "https://grundfos.com/concept/productFamily",
            "skos:prefLabel": "ALPHA2.1 OEM"
        },
        {
            "@id": "https://grundfos.com/concept/productFamily/ALPHA22",
            "@type": [
                "gfs:ProductFamily",
                "skos:Concept"
            ],
            "gfs:level": 2,
            "gfs:typecode": "ALPHA22",
            "rdfs:comment": "Grundfos ALPHA2.2 are stand-alone circulators with advanced control functions plus Go Balance",
            "skos:inScheme": "https://grundfos.com/concept/productFamily",
            "skos:prefLabel": "ALPHA2.2 OEM"
        },
        {
            "@id": "https://grundfos.com/concept/productFamily/UPSOLOEM",
            "@type": [
                "gfs:ProductFamily",
                "skos:Concept"
            ],
            "gfs:level": 2,
            "gfs:typecode": "UPSOLOEM",
            "rdfs:comment": "SOLAR PML is an OEM high efficiency circulator for thermal solar systems with extended performance",
            "skos:inScheme": "https://grundfos.com/concept/productFamily",
            "skos:prefLabel": "SOLAR PML"
        },
        {
            "@id": "https://grundfos.com/concept/productFamily/UPMGEO",
            "@type": [
                "gfs:ProductFamily",
                "skos:Concept"
            ],
            "gfs:level": 2,
            "gfs:typecode": "UPMGEO",
            "rdfs:comment": "UPM GEO is a integrated circulator externally controlled via a signal cable entry with extended performance.",
            "skos:inScheme": "https://grundfos.com/concept/productFamily",
            "skos:prefLabel": "UPM GEO OEM"
        },
        {
            "@id": "https://grundfos.com/concept/productFamily/UPM2",
            "@type": [
                "gfs:ProductFamily",
                "skos:Concept"
            ],
            "gfs:level": 2,
            "gfs:typecode": "UPM2",
            "rdfs:comment": "UPM2 is a boiler integrated circulator externally controlled via a signal cable entry.",
            "skos:inScheme": "https://grundfos.com/concept/productFamily",
            "skos:prefLabel": "UPM2 OEM"
        },
        {
            "@id": "https://grundfos.com/concept/productFamily/UPM3",
            "@type": [
                "gfs:ProductFamily",
                "skos:Concept"
            ],
            "gfs:level": 2,
            "gfs:typecode": "UPM3",
            "rdfs:comment": "UPM3 is a boiler integrated circulator externally controlled via a signal cable entry.",
            "skos:inScheme": "https://grundfos.com/concept/productFamily",
            "skos:prefLabel": "UPM3 OEM"
        },
        {
            "@id": "https://grundfos.com/concept/productFamily/UPML",
            "@type": [
                "gfs:ProductFamily",
                "skos:Concept"
            ],
            "gfs:level": 2,
            "gfs:typecode": "UPML",
            "rdfs:comment": "UPML is designed for integration in boilers and other heating appliances with large performance.",
            "skos:inScheme": "https://grundfos.com/concept/productFamily",
            "skos:prefLabel": "UPML OEM"
        },
        {
            "@id": "https://grundfos.com/concept/productFamily/UPMM",
            "@type": [
                "gfs:ProductFamily",
                "skos:Concept"
            ],
            "gfs:level": 2,
            "gfs:typecode": "UPMM",
            "rdfs:comment": "UPMM is designed for integration in boilers and other heating appliances with medium performance.",
            "skos:inScheme": "https://grundfos.com/concept/productFamily",
            "skos:prefLabel": "UPMM OEM"
        },
        {
            "@id": "https://grundfos.com/concept/productFamily/UPMO",
            "@type": [
                "gfs:ProductFamily",
                "skos:Concept"
            ],
            "gfs:level": 2,
            "gfs:typecode": "UPMO",
            "rdfs:comment": "UPMO is the right ErP replacement for UP integrated in heating appliances or stand alone.",
            "skos:inScheme": "https://grundfos.com/concept/productFamily",
            "skos:prefLabel": "UPMO OEM"
        },
        {
            "@id": "https://grundfos.com/concept/productFamily/UPMXL",
            "@type": [
                "gfs:ProductFamily",
                "skos:Concept"
            ],
            "gfs:level": 2,
            "gfs:typecode": "UPMXL",
            "rdfs:comment": "UPMXL is designed for integration in boilers and other heating appliances with extra large performance.",
            "skos:inScheme": "https://grundfos.com/concept/productFamily",
            "skos:prefLabel": "UPMXL OEM"
        },
        {
            "@id": "https://grundfos.com/concept/productFamily/UPOEM",
            "@type": [
                "gfs:ProductFamily",
                "skos:Concept"
            ],
            "gfs:level": 1,
            "gfs:typecode": "UPOEM",
            "rdfs:comment": "OEM high efficiency circulator pumps suitable for all HVAC applications, from boilers and heat pumps to HIU systems.",
            "skos:inScheme": "https://grundfos.com/concept/productFamily",
            "skos:narrower": [
                "https://grundfos.com/concept/productFamily/ALPHA11",
                "https://grundfos.com/concept/productFamily/ALPHA21",
                "https://grundfos.com/concept/productFamily/ALPHA22",
                "https://grundfos.com/concept/productFamily/UPSOLOEM",
                "https://grundfos.com/concept/productFamily/UPMGEO",
                "https://grundfos.com/concept/productFamily/UPM2",
                "https://grundfos.com/concept/productFamily/UPM3",
                "https://grundfos.com/concept/productFamily/UPML",
                "https://grundfos.com/concept/productFamily/UPMM",
                "https://grundfos.com/concept/productFamily/UPMO",
                "https://grundfos.com/concept/productFamily/UPMXL"
            ],
            "skos:prefLabel": "UP OEM"
        },
        {
            "@id": "https://grundfos.com/concept/productFamily/UPS01",
            "@type": [
                "gfs:ProductFamily",
                "skos:Concept"
            ],
            "gfs:level": 2,
            "gfs:typecode": "UPS01",
            "rdfs:comment": "Circulator pumps",
            "skos:inScheme": "https://grundfos.com/concept/productFamily",
            "skos:prefLabel": "UP, UPS"
        },
        {
            "@id": "https://grundfos.com/concept/productFamily/UPSB1",
            "@type": [
                "gfs:ProductFamily",
                "skos:Concept"
            ],
            "gfs:level": 2,
            "gfs:typecode": "UPSB1",
            "rdfs:comment": "Domestic hot water pumps",
            "skos:inScheme": "https://grundfos.com/concept/productFamily",
            "skos:prefLabel": "UP, UPS (N)"
        },
        {
            "@id": "https://grundfos.com/concept/productFamily/UPS200",
            "@type": [
                "gfs:ProductFamily",
                "skos:Concept"
            ],
            "gfs:level": 2,
            "gfs:typecode": "UPS200",
            "rdfs:comment": "Circulator pumps",
            "skos:inScheme": "https://grundfos.com/concept/productFamily",
            "skos:prefLabel": "UPS2"
        },
        {
            "@id": "https://grundfos.com/concept/productFamily/UPSD1",
            "@type": [
                "gfs:ProductFamily",
                "skos:Concept"
            ],
            "gfs:level": 2,
            "gfs:typecode": "UPSD1",
            "rdfs:comment": "Twin-head circulator pumps",
            "skos:inScheme": "https://grundfos.com/concept/productFamily",
            "skos:prefLabel": "UPSD"
        },
        {
            "@id": "https://grundfos.com/concept/productFamily/S100FAM",
            "@type": [
                "gfs:ProductFamily",
                "skos:Concept"
            ],
            "gfs:level": 1,
            "gfs:typecode": "S100FAM",
            "rdfs:comment": "Non-electronically controlled circulator pumps for domestic building with speedcontrol",
            "skos:inScheme": "https://grundfos.com/concept/productFamily",
            "skos:narrower": [
                "https://grundfos.com/concept/productFamily/UPS01",
                "https://grundfos.com/concept/productFamily/UPSB1",
                "https://grundfos.com/concept/productFamily/UPS200",
                "https://grundfos.com/concept/productFamily/UPSD1"
            ],
            "skos:prefLabel": "UP, UPS Series 100"
        },
        {
            "@id": "https://grundfos.com/concept/productFamily/UPA000",
            "@type": [
                "gfs:ProductFamily",
                "skos:Concept"
            ],
            "gfs:level": 1,
            "gfs:typecode": "UPA000",
            "rdfs:comment": "Domestic in-line boosting pumps",
            "skos:inScheme": "https://grundfos.com/concept/productFamily",
            "skos:narrower": [],
            "skos:prefLabel": "UPA, Home booster"
        },
        {
            "@id": "https://grundfos.com/concept/productFamily/UPS02",
            "@type": [
                "gfs:ProductFamily",
                "skos:Concept"
            ],
            "gfs:level": 2,
            "gfs:typecode": "UPS02",
            "rdfs:comment": "Circulator pumps",
            "skos:inScheme": "https://grundfos.com/concept/productFamily",
            "skos:prefLabel": "UPS"
        },
        {
            "@id": "https://grundfos.com/concept/productFamily/UPSB2",
            "@type": [
                "gfs:ProductFamily",
                "skos:Concept"
            ],
            "gfs:level": 2,
            "gfs:typecode": "UPSB2",
            "rdfs:comment": "Domestic hot water pumps",
            "skos:inScheme": "https://grundfos.com/concept/productFamily",
            "skos:prefLabel": "UPS (B)"
        },
        {
            "@id": "https://grundfos.com/concept/productFamily/UPSD2",
            "@type": [
                "gfs:ProductFamily",
                "skos:Concept"
            ],
            "gfs:level": 2,
            "gfs:typecode": "UPSD2",
            "rdfs:comment": "Twin-head circulator pumps",
            "skos:inScheme": "https://grundfos.com/concept/productFamily",
            "skos:prefLabel": "UPSD"
        },
        {
            "@id": "https://grundfos.com/concept/productFamily/S200FAM",
            "@type": [
                "gfs:ProductFamily",
                "skos:Concept"
            ],
            "gfs:level": 1,
            "gfs:typecode": "S200FAM",
            "rdfs:comment": "Non-electronically controlled circulator pumps for commercial building with speedcontrol",
            "skos:inScheme": "https://grundfos.com/concept/productFamily",
            "skos:narrower": [
                "https://grundfos.com/concept/productFamily/UPS02",
                "https://grundfos.com/concept/productFamily/UPSB2",
                "https://grundfos.com/concept/productFamily/UPSD2"
            ],
            "skos:prefLabel": "UPS Series 200"
        }
    ]
}